@prefix : <http://www.yso.fi/onto/metatietosanasto/> .
@prefix dc: <http://purl.org/dc/elements/1.1/> .
@prefix dct: <http://purl.org/dc/terms/> .
@prefix foaf: <http://xmlns.com/foaf/0.1/> .
@prefix isothes: <http://purl.org/iso25964/skos-thes#> .
@prefix mts: <http://metatietosanasto.fi/> .
@prefix owl: <http://www.w3.org/2002/07/owl#> .
@prefix rdaa: <http://rdaregistry.info/Elements/a/> .
@prefix rdac: <http://rdaregistry.info/Elements/c/> .
@prefix rdae: <http://rdaregistry.info/Elements/e/> .
@prefix rdai: <http://rdaregistry.info/Elements/i/> .
@prefix rdam: <http://rdaregistry.info/Elements/m/> .
@prefix rdau: <http://rdaregistry.info/Elements/u/> .
@prefix rdaw: <http://rdaregistry.info/Elements/w/> .
@prefix rdf: <http://www.w3.org/1999/02/22-rdf-syntax-ns#> .
@prefix rdfs: <http://www.w3.org/2000/01/rdf-schema#> .
@prefix reg: <http://metadataregistry.org/uri/profile/RegAp/> .
@prefix skos: <http://www.w3.org/2004/02/skos/core#> .
@prefix status: <http://metadataregistry.org/uri/RegStatus/> .
@prefix xml: <http://www.w3.org/XML/1998/namespace> .
@prefix xsd: <http://www.w3.org/2001/XMLSchema#> .

mts:C10001 a isothes:ConceptGroup,
        skos:Collection ;
    rdfs:seeAlso rdac:C10001 ;
    skos:definition "Itsenäinen tiedollinen tai taiteellinen sisältö."@fi ;
    skos:prefLabel "Teos"@fi .

mts:C10002 a isothes:ConceptGroup,
        skos:Collection ;
    rdfs:seeAlso rdac:C10002 ;
    skos:prefLabel "Toimija"@fi .

mts:C10003 a isothes:ConceptGroup,
        skos:Collection ;
    rdfs:seeAlso rdac:C10003 ;
    skos:definition "Yksittäinen manifestaation toteutuma (esim. yksittäinen CD-äänilevy, kirja kirjaston kokoelmissa)."@fi ;
    skos:prefLabel "Kappale"@fi .

mts:C10004 a isothes:ConceptGroup,
        skos:Collection ;
    rdfs:seeAlso rdac:C10004 ;
    skos:prefLabel "Henkilö"@fi .

mts:C10005 a isothes:ConceptGroup,
        skos:Collection ;
    rdfs:seeAlso rdac:C10005 ;
    skos:prefLabel "Yhteisö"@fi .

mts:C10006 a isothes:ConceptGroup,
        skos:Collection ;
    rdfs:seeAlso rdac:C10006 ;
    skos:definition "Teoksen tiedollinen tai taiteellinen toteutus, joka voi olla muodoltaan ääntä, kuvaa, liikettä, kirjaimista koostuva, musiikkinuotinnos jne."@fi ;
    skos:prefLabel "Ekspressio"@fi .

mts:C10008 a isothes:ConceptGroup,
        skos:Collection ;
    rdfs:seeAlso rdac:C10008 ;
    skos:prefLabel "Suku"@fi .

mts:P30001 a isothes:ConceptGroup,
        skos:Collection ;
    isothes:superGroup mts:C10007 ;
    rdfs:seeAlso rdam:P30001 ;
    skos:member <http://metatietosanasto.fi/069>,
        <http://metatietosanasto.fi/069_1>,
        <http://metatietosanasto.fi/070>,
        <http://metatietosanasto.fi/071>,
        <http://metatietosanasto.fi/072>,
        <http://metatietosanasto.fi/073>,
        <http://metatietosanasto.fi/074>,
        <http://metatietosanasto.fi/075>,
        <http://metatietosanasto.fi/076>,
        <http://metatietosanasto.fi/077>,
        <http://metatietosanasto.fi/078>,
        <http://metatietosanasto.fi/080>,
        <http://metatietosanasto.fi/081>,
        <http://metatietosanasto.fi/082>,
        <http://metatietosanasto.fi/083>,
        <http://metatietosanasto.fi/084>,
        <http://metatietosanasto.fi/085>,
        <http://metatietosanasto.fi/086>,
        <http://metatietosanasto.fi/087>,
        <http://metatietosanasto.fi/088>,
        <http://metatietosanasto.fi/089>,
        <http://metatietosanasto.fi/090>,
        <http://metatietosanasto.fi/091>,
        <http://metatietosanasto.fi/092>,
        <http://metatietosanasto.fi/093>,
        <http://metatietosanasto.fi/094>,
        <http://metatietosanasto.fi/095>,
        <http://metatietosanasto.fi/096>,
        <http://metatietosanasto.fi/097>,
        <http://metatietosanasto.fi/098>,
        <http://metatietosanasto.fi/099>,
        <http://metatietosanasto.fi/100>,
        <http://metatietosanasto.fi/101>,
        <http://metatietosanasto.fi/102>,
        <http://metatietosanasto.fi/103>,
        <http://metatietosanasto.fi/104>,
        <http://rdvocab.info/termList/RDACarrierType/1004>,
        <http://rdvocab.info/termList/RDACarrierType/1007>,
        <http://rdvocab.info/termList/RDACarrierType/1008>,
        <http://rdvocab.info/termList/RDACarrierType/1011>,
        <http://rdvocab.info/termList/RDACarrierType/1013>,
        <http://rdvocab.info/termList/RDACarrierType/1018>,
        <http://rdvocab.info/termList/RDACarrierType/1022>,
        <http://rdvocab.info/termList/RDACarrierType/1027>,
        <http://rdvocab.info/termList/RDACarrierType/1040>,
        <http://rdvocab.info/termList/RDACarrierType/1045>,
        <http://rdvocab.info/termList/RDACarrierType/1052>,
        <http://rdvocab.info/termList/RDACarrierType/1056>,
        <http://rdvocab.info/termList/RDACarrierType/1060> ;
    skos:prefLabel "tallennetyyppi"@fi .

mts:P30002 a isothes:ConceptGroup,
        skos:Collection ;
    isothes:superGroup mts:C10007 ;
    rdfs:seeAlso rdam:P30002 ;
    skos:member <http://iflastandards.info/ns/isbd/terms/mediatype/T1001>,
        <http://iflastandards.info/ns/isbd/terms/mediatype/T1002>,
        <http://iflastandards.info/ns/isbd/terms/mediatype/T1003>,
        <http://iflastandards.info/ns/isbd/terms/mediatype/T1004>,
        <http://iflastandards.info/ns/isbd/terms/mediatype/T1005>,
        <http://iflastandards.info/ns/isbd/terms/mediatype/T1006>,
        <http://iflastandards.info/ns/isbd/terms/mediatype/T1007>,
        <http://iflastandards.info/ns/isbd/terms/mediatype/T1008>,
        <http://iflastandards.info/ns/isbd/terms/mediatype/T1009>,
        <http://iflastandards.info/ns/isbd/terms/mediatype/T1010> ;
    skos:prefLabel "mediatyyppi"@fi .

mts:P30004 a isothes:ConceptGroup,
        skos:Collection ;
    isothes:superGroup mts:C10007 ;
    rdfs:comment """Manifestaation tunniste on merkkijono, joka liittyy manifestaatioon ja joka erottaa manifestaation toisesta manifestaatiosta.\r
Manifestaation tunnisteisiin kuuluvat rekisteröidyt tunnisteet, joiden skeemat ovat kansainvälisesti hyväksyttyjä (esim. ISBN, ISSN, URN), sekä tunnisteet, joita kustantajat, jakajat, julkishallinnolliset yhteisöt, dokumentaatiopalvelut, arkistot tms. antavat ja jotka noudattavat sisäiseen tarkoitukseen laadittuja skeemoja.\r
Manifestaation tunnisteisiin kuuluu myös musiikin kustantajien numerot ja musiikkiaineiston laatan numerot."""@fi ;
    rdfs:seeAlso rdam:P30004 ;
    skos:member <http://metatietosanasto.fi/165>,
        <http://metatietosanasto.fi/166>,
        <http://metatietosanasto.fi/167>,
        <http://metatietosanasto.fi/168>,
        <http://metatietosanasto.fi/169>,
        <http://metatietosanasto.fi/170>,
        <http://metatietosanasto.fi/171>,
        <http://metatietosanasto.fi/172>,
        <http://metatietosanasto.fi/173> ;
    skos:prefLabel "manifestaation tunniste"@fi .

mts:P30007 a isothes:ConceptGroup,
        skos:Collection ;
    rdfs:seeAlso rdam:P30007 ;
    skos:prefLabel "copyright-vuosi"@fi .

mts:P30018 a isothes:ConceptGroup,
        skos:Collection ;
    isothes:superGroup mts:C10007 ;
    rdfs:seeAlso rdam:P30007 ;
    skos:member <http://metatietosanasto.fi/136>,
        <http://metatietosanasto.fi/137>,
        <http://metatietosanasto.fi/138>,
        <http://metatietosanasto.fi/139>,
        <http://metatietosanasto.fi/140>,
        <http://metatietosanasto.fi/141>,
        <http://metatietosanasto.fi/142>,
        <http://metatietosanasto.fi/143>,
        <http://metatietosanasto.fi/144>,
        <http://metatietosanasto.fi/145>,
        <http://metatietosanasto.fi/146>,
        <http://metatietosanasto.fi/147>,
        <http://metatietosanasto.fi/148>,
        <http://metatietosanasto.fi/149>,
        <http://metatietosanasto.fi/150>,
        <http://metatietosanasto.fi/151>,
        <http://metatietosanasto.fi/152>,
        <http://metatietosanasto.fi/153>,
        <http://metatietosanasto.fi/154>,
        <http://metatietosanasto.fi/155>,
        <http://metatietosanasto.fi/156>,
        <http://rdvocab.info/termList/fileType/1001>,
        <http://rdvocab.info/termList/fileType/1002>,
        <http://rdvocab.info/termList/fileType/1004>,
        <http://rdvocab.info/termList/fileType/1006> ;
    skos:prefLabel "tiedostomuoto"@fi .

mts:P30052 a isothes:ConceptGroup,
        skos:Collection ;
    isothes:superGroup mts:C10007 ;
    rdfs:seeAlso rdam:P30052 ;
    skos:member <http://metatietosanasto.fi/162> ;
    skos:prefLabel "huomautus jakelutiedoista"@fi .

mts:P30053 a isothes:ConceptGroup,
        skos:Collection ;
    isothes:superGroup mts:C10007 ;
    rdfs:seeAlso rdam:P30053 ;
    skos:member <http://metatietosanasto.fi/163> ;
    skos:prefLabel "huomautus valmistustiedoista"@fi .

mts:P30055 a isothes:ConceptGroup,
        skos:Collection ;
    isothes:superGroup mts:C10007 ;
    rdfs:seeAlso rdam:P30055 ;
    skos:member <http://metatietosanasto.fi/161> ;
    skos:prefLabel "huomautus kustannustiedoista"@fi .

mts:P30059 a isothes:ConceptGroup,
        skos:Collection ;
    isothes:superGroup mts:C10007 ;
    rdfs:seeAlso rdam:P30059 ;
    skos:member <http://metatietosanasto.fi/164> ;
    skos:prefLabel "huomautus copyright-vuodesta"@fi .

mts:P30063 a isothes:ConceptGroup,
        skos:Collection ;
    isothes:superGroup mts:C10007 ;
    rdfs:seeAlso rdam:P30063 ;
    skos:member <http://metatietosanasto.fi/025>,
        <http://metatietosanasto.fi/026>,
        <http://metatietosanasto.fi/026_1>,
        <http://metatietosanasto.fi/027>,
        <http://metatietosanasto.fi/028>,
        <http://metatietosanasto.fi/029>,
        <http://metatietosanasto.fi/030>,
        <http://metatietosanasto.fi/031>,
        <http://metatietosanasto.fi/032>,
        <http://metatietosanasto.fi/033>,
        <http://metatietosanasto.fi/034>,
        <http://metatietosanasto.fi/035>,
        <http://metatietosanasto.fi/036>,
        <http://metatietosanasto.fi/037>,
        <http://metatietosanasto.fi/038>,
        <http://metatietosanasto.fi/039>,
        <http://metatietosanasto.fi/040>,
        <http://metatietosanasto.fi/041>,
        <http://metatietosanasto.fi/042>,
        <http://metatietosanasto.fi/043>,
        <http://metatietosanasto.fi/044>,
        <http://metatietosanasto.fi/045>,
        <http://metatietosanasto.fi/046>,
        <http://metatietosanasto.fi/047>,
        <http://metatietosanasto.fi/048>,
        <http://metatietosanasto.fi/049>,
        <http://metatietosanasto.fi/050>,
        <http://metatietosanasto.fi/051>,
        <http://metatietosanasto.fi/052>,
        <http://metatietosanasto.fi/053>,
        <http://metatietosanasto.fi/054>,
        <http://metatietosanasto.fi/055>,
        <http://metatietosanasto.fi/056>,
        <http://metatietosanasto.fi/057>,
        <http://metatietosanasto.fi/058>,
        <http://metatietosanasto.fi/059>,
        <http://metatietosanasto.fi/060>,
        <http://metatietosanasto.fi/061>,
        <http://metatietosanasto.fi/062>,
        <http://metatietosanasto.fi/063>,
        <http://metatietosanasto.fi/064>,
        <http://metatietosanasto.fi/065>,
        <http://metatietosanasto.fi/066>,
        <http://metatietosanasto.fi/067> ;
    skos:prefLabel "huomautus nimekkeestä"@fi .

mts:P30064 a isothes:ConceptGroup,
        skos:Collection ;
    isothes:superGroup mts:C10007 ;
    rdfs:seeAlso rdam:P30064 ;
    skos:member <http://metatietosanasto.fi/157>,
        <http://metatietosanasto.fi/158>,
        <http://metatietosanasto.fi/159>,
        <http://metatietosanasto.fi/160> ;
    skos:prefLabel "huomautus painostiedoista"@fi .

mts:P30080 a isothes:ConceptGroup,
        skos:Collection ;
    rdfs:seeAlso rdam:P30080 ;
    skos:prefLabel "jakaja"@fi .

mts:P30082 a isothes:ConceptGroup,
        skos:Collection ;
    rdfs:seeAlso rdam:P30082 ;
    skos:prefLabel "valmistaja"@fi .

mts:P30083 a isothes:ConceptGroup,
        skos:Collection ;
    rdfs:seeAlso rdam:P30083 ;
    skos:prefLabel "kustantaja"@fi .

mts:P30096 a isothes:ConceptGroup,
        skos:Collection ;
    rdfs:seeAlso rdam:P30096 ;
    skos:prefLabel "koodaamismuoto"@fi .

mts:P30107 a isothes:ConceptGroup,
        skos:Collection ;
    isothes:superGroup mts:C10007 ;
    rdfs:seeAlso rdam:P30107 ;
    skos:member <http://metatietosanasto.fi/157>,
        <http://metatietosanasto.fi/158>,
        <http://metatietosanasto.fi/159>,
        <http://metatietosanasto.fi/160> ;
    skos:prefLabel "painostiedot"@fi .

mts:P30108 a isothes:ConceptGroup,
        skos:Collection ;
    rdfs:seeAlso rdam:P30108 ;
    skos:prefLabel "jakajatiedot"@fi .

mts:P30109 a isothes:ConceptGroup,
        skos:Collection ;
    rdfs:seeAlso rdam:P30109 ;
    skos:prefLabel "valmistustiedot"@fi .

mts:P30110 a isothes:ConceptGroup,
        skos:Collection ;
    rdfs:seeAlso rdam:P30110 ;
    skos:prefLabel "tuotantotiedot"@fi .

mts:P30111 a isothes:ConceptGroup,
        skos:Collection ;
    rdfs:seeAlso rdam:P30111 ;
    skos:prefLabel "kustannustiedot"@fi .

mts:P30128 a isothes:ConceptGroup,
        skos:Collection ;
    rdfs:comment "Päänimekkeestä poikkeava nimekkeen muoto."@fi ;
    rdfs:seeAlso rdam:P30128 .

mts:P30134 a isothes:ConceptGroup,
        skos:Collection ;
    reg:hasSubproperty "alanimeke"@fi,
        "epäitsenäinen nimeke"@fi,
        "erottuva nimeke"@fi,
        "juokseva nimeke"@fi,
        "kansinimeke"@fi,
        "osan nimeke"@fi,
        "otsikkonimeke"@fi,
        "selkänimeke"@fi,
        "sepitetty nimeke"@fi,
        "vaihtoehtoinen nimeke"@fi,
        "yhteisnimeke"@fi,
        "ylänimeke"@fi ;
    rdfs:seeAlso rdam:P300134 ;
    skos:prefLabel "nimekkeet"@fi .

mts:P30142 a isothes:ConceptGroup,
        skos:Collection ;
    rdfs:comment "Sana, ilmaisu tai merkkiryhmä, joka esiintyy julkaisun päänimekkeen yhteydessä ja sille alisteisena. Muu nimeketieto määrittelee, selittää tai täydentää nimekettä, johon se kuuluu."@fi ;
    rdfs:seeAlso rdam:P30142 ;
    skos:prefLabel "muu nimeketieto"@fi .

mts:P30145 a isothes:ConceptGroup,
        skos:Collection ;
    isothes:superGroup mts:C10007 ;
    rdfs:seeAlso rdam:P30145 ;
    skos:member <http://metatietosanasto.fi/001>,
        <http://metatietosanasto.fi/002>,
        <http://metatietosanasto.fi/003>,
        <http://metatietosanasto.fi/004>,
        <http://metatietosanasto.fi/005>,
        <http://metatietosanasto.fi/006>,
        <http://metatietosanasto.fi/007>,
        <http://metatietosanasto.fi/008>,
        <http://metatietosanasto.fi/009>,
        <http://metatietosanasto.fi/010> ;
    skos:prefLabel "aineiston saatavuuden rajoitukset"@fi .

mts:P30146 a isothes:ConceptGroup,
        skos:Collection ;
    isothes:superGroup mts:C10007 ;
    rdfs:seeAlso rdam:P30146 ;
    skos:definition "Aineiston käyttöä, esim. kopiointia, julkaisemista tai esille asettamista, koskevia rajoituksia."@fi ;
    skos:member <http://metatietosanasto.fi/011> ;
    skos:prefLabel "aineiston käyttöehdot"@fi .

mts:P30156 a isothes:ConceptGroup,
        skos:Collection ;
    rdfs:seeAlso rdam:P30156 ;
    skos:prefLabel "päänimeke"@fi .

mts:P30162 a isothes:ConceptGroup,
        skos:Collection ;
    isothes:superGroup mts:C10007 ;
    rdfs:seeAlso rdam:P30162 ;
    skos:member <http://metatietosanasto.fi/012>,
        <http://metatietosanasto.fi/013>,
        <http://metatietosanasto.fi/014>,
        <http://metatietosanasto.fi/015>,
        <http://metatietosanasto.fi/016>,
        <http://metatietosanasto.fi/017>,
        <http://metatietosanasto.fi/018>,
        <http://metatietosanasto.fi/019>,
        <http://metatietosanasto.fi/020>,
        <http://metatietosanasto.fi/021>,
        <http://metatietosanasto.fi/022>,
        <http://metatietosanasto.fi/023>,
        <http://metatietosanasto.fi/024> ;
    skos:prefLabel "laitteisto- tai järjestelmävaatimukset"@fi .

mts:P30173 a isothes:ConceptGroup,
        skos:Collection ;
    rdfs:seeAlso rdam:P30173 ;
    skos:prefLabel "jakajan nimi"@fi .

mts:P30174 a isothes:ConceptGroup,
        skos:Collection ;
    rdfs:seeAlso rdam:P30174 ;
    skos:prefLabel "tuottajan nimi"@fi .

mts:P30175 a isothes:ConceptGroup,
        skos:Collection ;
    rdfs:seeAlso rdam:P30175 ;
    skos:prefLabel "valmistajan nimi"@fi .

mts:P30176 a isothes:ConceptGroup,
        skos:Collection ;
    rdfs:seeAlso rdam:P30176 ;
    skos:prefLabel "kustantajan nimi"@fi .

mts:P30199 a isothes:ConceptGroup,
        skos:Collection ;
    isothes:superGroup mts:C10007 ;
    rdfs:seeAlso rdam:P30199 ;
    skos:member <http://rdvocab.info/termList/fontSize/1001>,
        <http://rdvocab.info/termList/fontSize/1002> ;
    skos:prefLabel "kirjasinkoko"@fi .

mts:P30203 a isothes:ConceptGroup,
        skos:Collection ;
    rdfs:seeAlso rdam:P30203 ;
    skos:prefLabel "rinnakkaisnimeke"@fi .

mts:P30209 a isothes:ConceptGroup,
        skos:Collection ;
    rdfs:comment "Jatkuvan julkaisun ainutkertainen nimi, jonka määrittää ISSN-verkosto ja joka liittyy ISSN-tunnukseen erottamattomasti."@fi ;
    rdfs:seeAlso rdam:P30209 ;
    skos:prefLabel "avainnimeke"@fi .

mts:P30214 a isothes:ConceptGroup,
        skos:Collection ;
    isothes:superGroup mts:C10007 ;
    rdfs:seeAlso rdam:P30214 ;
    skos:member <http://metatietosanasto.fi/068>,
        <http://metatietosanasto.fi/106>,
        <http://metatietosanasto.fi/107>,
        <http://metatietosanasto.fi/108>,
        <http://metatietosanasto.fi/109>,
        <http://metatietosanasto.fi/110>,
        <http://metatietosanasto.fi/111>,
        <http://metatietosanasto.fi/112>,
        <http://metatietosanasto.fi/113>,
        <http://metatietosanasto.fi/114>,
        <http://metatietosanasto.fi/115>,
        <http://metatietosanasto.fi/116>,
        <http://metatietosanasto.fi/117>,
        <http://metatietosanasto.fi/118>,
        <http://metatietosanasto.fi/119>,
        <http://metatietosanasto.fi/120>,
        <http://metatietosanasto.fi/121>,
        <http://metatietosanasto.fi/122>,
        <http://metatietosanasto.fi/123>,
        <http://metatietosanasto.fi/124>,
        <http://metatietosanasto.fi/125>,
        <http://metatietosanasto.fi/126>,
        <http://metatietosanasto.fi/127>,
        <http://metatietosanasto.fi/128>,
        <http://metatietosanasto.fi/129>,
        <http://metatietosanasto.fi/130>,
        <http://metatietosanasto.fi/131>,
        <http://metatietosanasto.fi/132>,
        <http://metatietosanasto.fi/133>,
        <http://metatietosanasto.fi/134>,
        <http://metatietosanasto.fi/135> ;
    skos:prefLabel "Huomautus tallenteesta"@fi .

rdam:P30003 a skos:Concept ;
    reg:name "modeOfIssuance"@en ;
    reg:status <http://metadataregistry.org/uri/RegStatus/1001> ;
    rdfs:domain rdac:C10007 ;
    rdfs:isDefinedBy rdam: ;
    rdfs:subPropertyOf rdau:P60051 ;
    owl:sameAs rdam:modeOfIssuance ;
    skos:definition "Relates a manifestation to a categorization reflecting whether a resource is issued in one or more parts, the way it is updated, and its intended termination."@en ;
    skos:inScheme : ;
    skos:prefLabel "has mode of issuance"@en .

rdam:P30005 a skos:Concept ;
    reg:name "preferredCitation"@en ;
    reg:status <http://metadataregistry.org/uri/RegStatus/1001> ;
    rdfs:domain rdac:C10007 ;
    rdfs:isDefinedBy rdam: ;
    rdfs:subPropertyOf rdau:P60057 ;
    owl:sameAs rdam:preferredCitation ;
    skos:definition "Relates a manifestation to a citation for a resource in the form preferred by a creator, publisher, custodian, indexing or abstracting service, etc."@en ;
    skos:inScheme : ;
    skos:prefLabel "has preferred citation"@en .

rdam:P30008 a skos:Concept ;
    reg:name "dateOfDistribution"@en ;
    reg:status <http://metadataregistry.org/uri/RegStatus/1001> ;
    rdfs:domain rdac:C10007 ;
    rdfs:isDefinedBy rdam: ;
    rdfs:subPropertyOf rdau:P60070 ;
    owl:sameAs rdam:dateOfDistribution ;
    skos:definition "Relates a manifestation to a date associated with the distribution of a resource in a published form."@en ;
    skos:inScheme : ;
    skos:prefLabel "has date of distribution"@en .

rdam:P30009 a skos:Concept ;
    reg:name "dateOfProduction"@en ;
    reg:status <http://metadataregistry.org/uri/RegStatus/1001> ;
    rdfs:domain rdac:C10007 ;
    rdfs:isDefinedBy rdam: ;
    rdfs:subPropertyOf rdau:P60071 ;
    owl:sameAs rdam:dateOfProduction ;
    skos:definition "Relates a manifestation to a date associated with the inscription, fabrication, construction, etc., of a resource in an unpublished form."@en ;
    skos:inScheme : ;
    skos:prefLabel "has date of production"@en .

rdam:P30010 a skos:Concept ;
    reg:name "dateOfManufacture"@en ;
    reg:status <http://metadataregistry.org/uri/RegStatus/1001> ;
    rdfs:domain rdac:C10007 ;
    rdfs:isDefinedBy rdam: ;
    rdfs:subPropertyOf rdau:P60072 ;
    owl:sameAs rdam:dateOfManufacture ;
    skos:definition "Relates a manifestation to a date associated with the printing, duplicating, casting, etc., of a resource in a published form."@en ;
    skos:inScheme : ;
    skos:prefLabel "has date of manufacture"@en .

rdam:P30011 a skos:Concept ;
    reg:name "dateOfPublication"@en ;
    reg:status <http://metadataregistry.org/uri/RegStatus/1001> ;
    rdfs:domain rdac:C10007 ;
    rdfs:isDefinedBy rdam: ;
    rdfs:subPropertyOf rdau:P60073 ;
    owl:sameAs rdam:dateOfPublication ;
    skos:definition "Relates a manifestation to a date associated with the publication, release, or issuing of a resource."@en ;
    skos:inScheme : ;
    skos:prefLabel "has date of publication"@en .

rdam:P30012 a skos:Concept ;
    reg:name "parallelDesignationOfANamedRevisionOfAnEdition"@en ;
    reg:status <http://metadataregistry.org/uri/RegStatus/1001> ;
    rdfs:domain rdac:C10007 ;
    rdfs:isDefinedBy rdam: ;
    rdfs:subPropertyOf rdau:P60077 ;
    owl:sameAs rdam:parallelDesignationOfANamedRevisionOfAnEdition ;
    skos:definition "Relates a manifestation to a designation of a named revision of an edition in a language and/or script that differs from that recorded in the designation of a named revision of an edition element."@en ;
    skos:inScheme : ;
    skos:prefLabel "has parallel designation of a named revision of an edition"@en .

rdam:P30013 a skos:Concept ;
    reg:name "parallelDesignationOfEdition"@en ;
    reg:status <http://metadataregistry.org/uri/RegStatus/1001> ;
    rdfs:domain rdac:C10007 ;
    rdfs:isDefinedBy rdam: ;
    rdfs:subPropertyOf rdau:P60078 ;
    owl:sameAs rdam:parallelDesignationOfEdition ;
    skos:definition "Relates a manifestation to a designation of edition in a language and/or script that differs from that recorded in the designation of edition element."@en ;
    skos:inScheme : ;
    skos:prefLabel "has parallel designation of edition"@en .

rdam:P30014 a skos:Concept ;
    reg:name "numberingWithinSeries"@en ;
    reg:status <http://metadataregistry.org/uri/RegStatus/1001> ;
    rdfs:domain rdac:C10007 ;
    rdfs:isDefinedBy rdam: ;
    rdfs:subPropertyOf rdau:P60081 ;
    owl:sameAs rdam:numberingWithinSeries ;
    skos:definition "Relates a manifestation to a designation of the sequencing of a part or parts within a series. numbering within series may include a numeral, a letter, any other character, or the combination of these with or without an accompanying caption (volume, number, etc.) and/or a chronological designation."@en ;
    skos:inScheme : ;
    skos:prefLabel "has numbering within series"@en .

rdam:P30015 a skos:Concept ;
    reg:name "numberingWithinSubseries"@en ;
    reg:status <http://metadataregistry.org/uri/RegStatus/1001> ;
    rdfs:domain rdac:C10007 ;
    rdfs:isDefinedBy rdam: ;
    rdfs:subPropertyOf rdau:P60082 ;
    owl:sameAs rdam:numberingWithinSubseries ;
    skos:definition "Relates a manifestation to a designation of the sequencing of a part or parts within a subseries. numbering within subseries may include a numeral, a letter, any other character, or the combination of these with or without an accompanying caption (volume, number, etc.) and/or a chronological designation."@en ;
    skos:inScheme : ;
    skos:prefLabel "has numbering within subseries"@en .

rdam:P30017 a skos:Concept ;
    reg:name "parallelDistributorsName"@en ;
    reg:status <http://metadataregistry.org/uri/RegStatus/1001> ;
    rdfs:domain rdac:C10007 ;
    rdfs:isDefinedBy rdam: ;
    rdfs:subPropertyOf rdau:P60087 ;
    owl:sameAs rdam:parallelDistributorsName ;
    skos:definition "Relates a manifestation to a distributor’s name in a language and/or script that differs from that recorded in the distributor’s name element."@en ;
    skos:inScheme : ;
    skos:prefLabel "has parallel distributor's name"@en .

rdam:P30049 a skos:Concept ;
    reg:name "parallelManufacturersName"@en ;
    reg:status <http://metadataregistry.org/uri/RegStatus/1001> ;
    rdfs:domain rdac:C10007 ;
    rdfs:isDefinedBy rdam: ;
    rdfs:subPropertyOf rdau:P60108 ;
    owl:sameAs rdam:parallelManufacturersName ;
    skos:definition "Relates a manifestation to a manufacturer’s name in a language and/or script that differs from that recorded in the manufacturer’s name element."@en ;
    skos:inScheme : ;
    skos:prefLabel "has parallel manufacturer's name"@en .

rdam:P30060 a skos:Concept ;
    reg:name "noteOnDimensionsOfManifestation"@en ;
    reg:status <http://metadataregistry.org/uri/RegStatus/1001> ;
    rdfs:domain rdac:C10007 ;
    rdfs:isDefinedBy rdam: ;
    rdfs:subPropertyOf rdau:P60133 ;
    owl:sameAs rdam:noteOnDimensionsOfManifestation ;
    skos:definition "Relates a manifestation to a note providing information on the dimensions of a manifestation that is not recorded as part of the dimensions element."@en ;
    skos:inScheme : ;
    skos:prefLabel "has note on dimensions of manifestation"@en .

rdam:P30061 a skos:Concept ;
    reg:name "noteOnExtentOfManifestation"@en ;
    reg:status <http://metadataregistry.org/uri/RegStatus/1001> ;
    rdfs:domain rdac:C10007 ;
    rdfs:isDefinedBy rdam: ;
    rdfs:subPropertyOf rdau:P60134 ;
    owl:sameAs rdam:noteOnExtentOfManifestation ;
    skos:definition "Relates a manifestation to a note providing information on the extent of a manifestation that is not recorded as part of the extent element."@en ;
    skos:inScheme : ;
    skos:prefLabel "has note on extent of manifestation"@en .

rdam:P30079 a skos:Concept ;
    reg:name "otherPFCManifestation"@en ;
    reg:status <http://metadataregistry.org/uri/RegStatus/1001> ;
    rdfs:domain rdac:C10007 ;
    rdfs:isDefinedBy rdam: ;
    rdfs:range rdac:C10002 ;
    rdfs:subPropertyOf rdau:P60374 ;
    owl:inverseOf rdaa:P50181 ;
    owl:sameAs rdam:otherPFCManifestation ;
    skos:definition "Relates a manifestation to a person, family, or corporate body other than a producer, publisher, distributor or manufacturer associated with a manifestation."@en ;
    skos:inScheme : ;
    skos:prefLabel "has other person, family, or corporate body associated with a manifestation"@en ;
    skos:scopeNote "Includes book designers, platemakers, etc."@en .

rdam:P30081 a skos:Concept ;
    reg:name "producerOfAnUnpublishedResource"@en ;
    reg:status <http://metadataregistry.org/uri/RegStatus/1001> ;
    rdfs:domain rdac:C10007 ;
    rdfs:isDefinedBy rdam: ;
    rdfs:range rdac:C10002 ;
    rdfs:subPropertyOf rdau:P60440 ;
    owl:inverseOf rdaa:P50200 ;
    owl:sameAs rdam:producerOfAnUnpublishedResource ;
    skos:definition "Relates a manifestation to a person, family, or corporate body responsible for inscribing, fabricating, constructing, etc., a resource in an unpublished form."@en ;
    skos:inScheme : ;
    skos:prefLabel "has producer of an unpublished resource"@en .

rdam:P30085 a skos:Concept ;
    reg:name "placeOfDistribution"@en ;
    reg:status <http://metadataregistry.org/uri/RegStatus/1001> ;
    rdfs:domain rdac:C10007 ;
    rdfs:isDefinedBy rdam: ;
    rdfs:subPropertyOf rdau:P60160 ;
    owl:sameAs rdam:placeOfDistribution ;
    skos:definition "Relates a manifestation to a place associated with the distribution of a resource in a published form."@en ;
    skos:inScheme : ;
    skos:prefLabel "has place of distribution"@en .

rdam:P30086 a skos:Concept ;
    reg:name "placeOfProduction"@en ;
    reg:status <http://metadataregistry.org/uri/RegStatus/1001> ;
    rdfs:domain rdac:C10007 ;
    rdfs:isDefinedBy rdam: ;
    rdfs:subPropertyOf rdau:P60161 ;
    owl:sameAs rdam:placeOfProduction ;
    skos:definition "Relates a manifestation to a place associated with the inscription, fabrication, construction, etc., of a resource in an unpublished form."@en ;
    skos:inScheme : ;
    skos:prefLabel "has place of production"@en .

rdam:P30087 a skos:Concept ;
    reg:name "placeOfManufacture"@en ;
    reg:status <http://metadataregistry.org/uri/RegStatus/1001> ;
    rdfs:domain rdac:C10007 ;
    rdfs:isDefinedBy rdam: ;
    rdfs:subPropertyOf rdau:P60162 ;
    owl:sameAs rdam:placeOfManufacture ;
    skos:definition "Relates a manifestation to a place associated with the printing, duplicating, casting, etc., of a resource in a published form."@en ;
    skos:inScheme : ;
    skos:prefLabel "has place of manufacture"@en .

rdam:P30088 a skos:Concept ;
    reg:name "placeOfPublication"@en ;
    reg:status <http://metadataregistry.org/uri/RegStatus/1001> ;
    rdfs:domain rdac:C10007 ;
    rdfs:isDefinedBy rdam: ;
    rdfs:subPropertyOf rdau:P60163 ;
    owl:sameAs rdam:placeOfPublication ;
    skos:definition "Relates a manifestation to a place associated with the publication, release, or issuing of a resource."@en ;
    skos:inScheme : ;
    skos:prefLabel "has place of publication"@en .

rdam:P30089 a skos:Concept ;
    reg:name "parallelPlaceOfDistribution"@en ;
    reg:status <http://metadataregistry.org/uri/RegStatus/1001> ;
    rdfs:domain rdac:C10007 ;
    rdfs:isDefinedBy rdam: ;
    rdfs:subPropertyOf rdau:P60164 ;
    owl:sameAs rdam:parallelPlaceOfDistribution ;
    skos:definition "Relates a manifestation to a place of distribution in a language and/or script that differs from that recorded in the place of distribution element."@en ;
    skos:inScheme : ;
    skos:prefLabel "has parallel place of distribution"@en .

rdam:P30090 a skos:Concept ;
    reg:name "parallelPlaceOfManufacture"@en ;
    reg:status <http://metadataregistry.org/uri/RegStatus/1001> ;
    rdfs:domain rdac:C10007 ;
    rdfs:isDefinedBy rdam: ;
    rdfs:subPropertyOf rdau:P60165 ;
    owl:sameAs rdam:parallelPlaceOfManufacture ;
    skos:definition "Relates a manifestation to a place of manufacture in a language and/or script that differs from that recorded in the place of manufacture element."@en ;
    skos:inScheme : ;
    skos:prefLabel "has parallel place of manufacture"@en .

rdam:P30091 a skos:Concept ;
    reg:name "parallelPlaceOfProduction"@en ;
    reg:status <http://metadataregistry.org/uri/RegStatus/1001> ;
    rdfs:domain rdac:C10007 ;
    rdfs:isDefinedBy rdam: ;
    rdfs:subPropertyOf rdau:P60166 ;
    owl:sameAs rdam:parallelPlaceOfProduction ;
    skos:definition "Relates a manifestation to a place of production in a language and/or script that differs from that recorded in the place of production element."@en ;
    skos:inScheme : ;
    skos:prefLabel "has parallel place of production"@en .

rdam:P30092 a skos:Concept ;
    reg:name "parallelPlaceOfPublication"@en ;
    reg:status <http://metadataregistry.org/uri/RegStatus/1001> ;
    rdfs:domain rdac:C10007 ;
    rdfs:isDefinedBy rdam: ;
    rdfs:subPropertyOf rdau:P60167 ;
    owl:sameAs rdam:parallelPlaceOfPublication ;
    skos:definition "Relates a manifestation to a place of publication in a language and/or script that differs from that recorded in the place of publication element."@en ;
    skos:inScheme : ;
    skos:prefLabel "has parallel place of publication"@en .

rdam:P30094 a skos:Concept ;
    reg:name "parallelProducersName"@en ;
    reg:status <http://metadataregistry.org/uri/RegStatus/1001> ;
    rdfs:domain rdac:C10007 ;
    rdfs:isDefinedBy rdam: ;
    rdfs:subPropertyOf rdau:P60172 ;
    owl:sameAs rdam:parallelProducersName ;
    skos:definition "Relates a manifestation to a producer’s name in a language and/or script that differs from that recorded in the producer’s name element."@en ;
    skos:inScheme : ;
    skos:prefLabel "has parallel producer's name"@en .

rdam:P30095 a skos:Concept ;
    reg:name "parallelPublishersName"@en ;
    reg:status <http://metadataregistry.org/uri/RegStatus/1001> ;
    rdfs:domain rdac:C10007 ;
    rdfs:isDefinedBy rdam: ;
    rdfs:subPropertyOf rdau:P60173 ;
    owl:sameAs rdam:parallelPublishersName ;
    skos:definition "Relates a manifestation to a publisher’s name in a language and/or script that differs from that recorded in the publisher’s name element."@en ;
    skos:inScheme : ;
    skos:prefLabel "has parallel publisher's name"@en .

rdam:P30103 a skos:Concept ;
    reg:name "exemplarOfManifestation"@en ;
    reg:status <http://metadataregistry.org/uri/RegStatus/1001> ;
    rdfs:domain rdac:C10007 ;
    rdfs:isDefinedBy rdam: ;
    rdfs:range rdac:C10003 ;
    owl:inverseOf rdai:P40049 ;
    owl:sameAs rdam:exemplarOfManifestation ;
    skos:definition "Relates a manifestation to a single exemplar or instance of a manifestation."@en ;
    skos:inScheme : ;
    skos:prefLabel "has exemplar of manifestation"@en .

rdam:P30106 a skos:Concept ;
    reg:name "seriesStatement"@en ;
    reg:status <http://metadataregistry.org/uri/RegStatus/1001> ;
    rdfs:domain rdac:C10007 ;
    rdfs:isDefinedBy rdam: ;
    rdfs:subPropertyOf rdau:P60328 ;
    owl:sameAs rdam:seriesStatement ;
    skos:definition "Relates a manifestation to a statement identifying a series to which a resource belongs and the numbering of the resource within the series."@en ;
    skos:inScheme : ;
    skos:prefLabel "has series statement"@en ;
    skos:scopeNote "A series statement may also include information identifying one or more subseries to which the resource being described belongs."@en .

rdam:P30112 a skos:Concept ;
    reg:name "parallelStatementOfResponsibilityRelatingToANamedRevisionOfAnEdition"@en ;
    reg:status <http://metadataregistry.org/uri/RegStatus/1001> ;
    rdfs:domain rdac:C10007 ;
    rdfs:isDefinedBy rdam: ;
    rdfs:subPropertyOf rdau:P60334 ;
    owl:sameAs rdam:parallelStatementOfResponsibilityRelatingToANamedRevisionOfAnEdition ;
    skos:definition "Relates a manifestation to a statement of responsibility relating to a named revision of an edition in a language and/or script that differs from that recorded in the statement of responsibility relating to a named revision of an edition element."@en ;
    skos:inScheme : ;
    skos:prefLabel "has parallel statement of responsibility relating to a named revision of an edition"@en .

rdam:P30113 a skos:Concept ;
    reg:name "parallelStatementOfResponsibilityRelatingToSeries"@en ;
    reg:status <http://metadataregistry.org/uri/RegStatus/1001> ;
    rdfs:domain rdac:C10007 ;
    rdfs:isDefinedBy rdam: ;
    rdfs:subPropertyOf rdau:P60335 ;
    owl:sameAs rdam:parallelStatementOfResponsibilityRelatingToSeries ;
    skos:definition "Relates a manifestation to a statement of responsibility relating to series in a language and/or script that differs from that recorded in the statement of responsibility relating to series element."@en ;
    skos:inScheme : ;
    skos:prefLabel "has parallel statement of responsibility relating to series"@en .

rdam:P30114 a skos:Concept ;
    reg:name "parallelStatementOfResponsibilityRelatingToSubseries"@en ;
    reg:status <http://metadataregistry.org/uri/RegStatus/1001> ;
    rdfs:domain rdac:C10007 ;
    rdfs:isDefinedBy rdam: ;
    rdfs:subPropertyOf rdau:P60336 ;
    owl:sameAs rdam:parallelStatementOfResponsibilityRelatingToSubseries ;
    skos:definition "Relates a manifestation to a statement of responsibility relating to subseries in a language and/or script that differs from that recorded in the statement of responsibility relating to subseries element."@en ;
    skos:inScheme : ;
    skos:prefLabel "has parallel statement of responsibility relating to subseries"@en .

rdam:P30115 a skos:Concept ;
    reg:name "parallelStatementOfResponsibilityRelatingToTheEdition"@en ;
    reg:status <http://metadataregistry.org/uri/RegStatus/1001> ;
    rdfs:domain rdac:C10007 ;
    rdfs:isDefinedBy rdam: ;
    rdfs:subPropertyOf rdau:P60337 ;
    owl:sameAs rdam:parallelStatementOfResponsibilityRelatingToTheEdition ;
    skos:definition "Relates a manifestation to a statement of responsibility relating to the edition in a language and/or script that differs from that recorded in the statement of responsibility relating to the edition element."@en ;
    skos:inScheme : ;
    skos:prefLabel "has parallel statement of responsibility relating to the edition"@en .

rdam:P30118 a skos:Concept ;
    reg:name "statementOfResponsibilityRelatingToANamedRevisionOfAnEdition"@en ;
    reg:status <http://metadataregistry.org/uri/RegStatus/1001> ;
    rdfs:domain rdac:C10007 ;
    rdfs:isDefinedBy rdam: ;
    rdfs:subPropertyOf rdau:P60340 ;
    owl:sameAs rdam:statementOfResponsibilityRelatingToANamedRevisionOfAnEdition ;
    skos:definition "Relates a manifestation to a statement relating to the identification of any persons, families, or corporate bodies responsible for a named revision of an edition."@en ;
    skos:inScheme : ;
    skos:prefLabel "has statement of responsibility relating to a named revision of an edition"@en .

rdam:P30119 a skos:Concept ;
    reg:name "statementOfResponsibilityRelatingToSeries"@en ;
    reg:status <http://metadataregistry.org/uri/RegStatus/1001> ;
    rdfs:domain rdac:C10007 ;
    rdfs:isDefinedBy rdam: ;
    rdfs:subPropertyOf rdau:P60341 ;
    owl:sameAs rdam:statementOfResponsibilityRelatingToSeries ;
    skos:definition "Relates a manifestation to a statement relating to the identification of any persons, families, or corporate bodies responsible for a series."@en ;
    skos:inScheme : ;
    skos:prefLabel "has statement of responsibility relating to series"@en .

rdam:P30120 a skos:Concept ;
    reg:name "statementOfResponsibilityRelatingToSubseries"@en ;
    reg:status <http://metadataregistry.org/uri/RegStatus/1001> ;
    rdfs:domain rdac:C10007 ;
    rdfs:isDefinedBy rdam: ;
    rdfs:subPropertyOf rdau:P60342 ;
    owl:sameAs rdam:statementOfResponsibilityRelatingToSubseries ;
    skos:definition "Relates a manifestation to a statement relating to the identification of any persons, families, or corporate bodies responsible for a subseries."@en ;
    skos:inScheme : ;
    skos:prefLabel "has statement of responsibility relating to subseries"@en .

rdam:P30121 a skos:Concept ;
    reg:name "statementOfResponsibilityRelatingToTheEdition"@en ;
    reg:status <http://metadataregistry.org/uri/RegStatus/1001> ;
    rdfs:domain rdac:C10007 ;
    rdfs:isDefinedBy rdam: ;
    rdfs:subPropertyOf rdau:P60343 ;
    owl:sameAs rdam:statementOfResponsibilityRelatingToTheEdition ;
    skos:definition "Relates a manifestation to a statement relating to the identification of any persons, families, or corporate bodies responsible for the edition being described but not to all editions."@en ;
    skos:inScheme : ;
    skos:prefLabel "has statement of responsibility relating to the edition"@en .

rdam:P30132 a skos:Concept ;
    reg:name "designationOfANamedRevisionOfAnEdition"@en ;
    reg:status <http://metadataregistry.org/uri/RegStatus/1001> ;
    rdfs:domain rdac:C10007 ;
    rdfs:isDefinedBy rdam: ;
    rdfs:subPropertyOf rdau:P60364 ;
    owl:sameAs rdam:designationOfANamedRevisionOfAnEdition ;
    skos:definition "Relates a manifestation to a word, character or group of words and/or characters, identifying a particular revision of a named edition."@en ;
    skos:inScheme : ;
    skos:prefLabel "has designation of a named revision of an edition"@en .

rdam:P30133 a skos:Concept ;
    reg:name "designationOfEdition"@en ;
    reg:status <http://metadataregistry.org/uri/RegStatus/1001> ;
    rdfs:domain rdac:C10007 ;
    rdfs:isDefinedBy rdam: ;
    rdfs:subPropertyOf rdau:P60365 ;
    owl:sameAs rdam:designationOfEdition ;
    skos:definition "Relates a manifestation to a word, character or group of words and/or characters, identifying the edition to which a resource belongs."@en ;
    skos:inScheme : ;
    skos:prefLabel "has designation of edition"@en .

rdam:P30135 a skos:Concept ;
    reg:name "workManifested"@en ;
    reg:status <http://metadataregistry.org/uri/RegStatus/1001> ;
    rdfs:domain rdac:C10007 ;
    rdfs:isDefinedBy rdam: ;
    rdfs:range rdac:C10001 ;
    owl:inverseOf rdaw:P10072 ;
    owl:sameAs rdam:workManifested ;
    skos:definition "Relates a manifestation to a work embodied in a manifestation."@en ;
    skos:inScheme : ;
    skos:prefLabel "has work manifested"@en .

rdam:P30139 a skos:Concept ;
    reg:name "expressionManifested"@en ;
    reg:status <http://metadataregistry.org/uri/RegStatus/1001> ;
    rdfs:domain rdac:C10007 ;
    rdfs:isDefinedBy rdam: ;
    rdfs:range rdac:C10006 ;
    owl:inverseOf rdae:P20059 ;
    owl:sameAs rdam:expressionManifested ;
    skos:definition "Relates a manifestation to an expression embodied in a manifestation."@en ;
    skos:inScheme : ;
    skos:prefLabel "has expression manifested"@en .

rdam:P30140 a skos:Concept ;
    reg:name "relatedItem"@en ;
    reg:status <http://metadataregistry.org/uri/RegStatus/1001> ;
    rdfs:domain rdac:C10007 ;
    rdfs:isDefinedBy rdam: ;
    rdfs:range rdac:C10003 ;
    rdfs:subPropertyOf rdau:P60313 ;
    owl:sameAs rdam:relatedItem ;
    skos:definition "Relates a manifestation to an item, represented by an identifier or a description, that is related to the manifestation being described (e.g., an item used as the basis for a microform reproduction)."@en ;
    skos:inScheme : ;
    skos:prefLabel "has related item"@en .

rdam:P30141 a skos:Concept ;
    reg:name "contactInformation"@en ;
    reg:status <http://metadataregistry.org/uri/RegStatus/1001> ;
    rdfs:domain rdac:C10007 ;
    rdfs:isDefinedBy rdam: ;
    rdfs:subPropertyOf rdau:P60490 ;
    owl:sameAs rdam:contactInformation ;
    skos:definition "Relates a manifestation to information about an organization, etc., from which a resource may be obtained."@en ;
    skos:inScheme : ;
    skos:prefLabel "has contact information"@en .

rdam:P30143 a skos:Concept ;
    reg:name "otherTitleInformationOfSeries"@en ;
    reg:status <http://metadataregistry.org/uri/RegStatus/1001> ;
    rdfs:domain rdac:C10007 ;
    rdfs:isDefinedBy rdam: ;
    rdfs:subPropertyOf rdau:P60494 ;
    owl:sameAs rdam:otherTitleInformationOfSeries ;
    skos:definition "Relates a manifestation to information that appears in conjunction with, and is subordinate to, the title proper of a series."@en ;
    skos:inScheme : ;
    skos:prefLabel "has other title information of series"@en .

rdam:P30144 a skos:Concept ;
    reg:name "otherTitleInformationOfSubseries"@en ;
    reg:status <http://metadataregistry.org/uri/RegStatus/1001> ;
    rdfs:domain rdac:C10007 ;
    rdfs:isDefinedBy rdam: ;
    rdfs:subPropertyOf rdau:P60495 ;
    owl:sameAs rdam:otherTitleInformationOfSubseries ;
    skos:definition "Relates a manifestation to information that appears in conjunction with, and is subordinate to, the title proper of a subseries."@en ;
    skos:inScheme : ;
    skos:prefLabel "has other title information of subseries"@en .

rdam:P30152 a skos:Concept ;
    reg:name "parallelOtherTitleInformationOfSeries"@en ;
    reg:status <http://metadataregistry.org/uri/RegStatus/1001> ;
    rdfs:domain rdac:C10007 ;
    rdfs:isDefinedBy rdam: ;
    rdfs:subPropertyOf rdau:P60508 ;
    owl:sameAs rdam:parallelOtherTitleInformationOfSeries ;
    skos:definition "Relates a manifestation to other title information of a series in a language and/or script that differs from that recorded in the other title information of series element."@en ;
    skos:inScheme : ;
    skos:prefLabel "has parallel other title information of series"@en .

rdam:P30153 a skos:Concept ;
    reg:name "parallelOtherTitleInformationOfSubseries"@en ;
    reg:status <http://metadataregistry.org/uri/RegStatus/1001> ;
    rdfs:domain rdac:C10007 ;
    rdfs:isDefinedBy rdam: ;
    rdfs:subPropertyOf rdau:P60509 ;
    owl:sameAs rdam:parallelOtherTitleInformationOfSubseries ;
    skos:definition "Relates a manifestation to other title information of a subseries in a language and/or script that differs from that recorded in the other title information of subseries element."@en ;
    skos:inScheme : ;
    skos:prefLabel "has parallel other title information of subseries"@en .

rdam:P30154 a skos:Concept ;
    reg:name "uniformResourceLocator"@en ;
    reg:status <http://metadataregistry.org/uri/RegStatus/1001> ;
    rdfs:domain rdac:C10007 ;
    rdfs:isDefinedBy rdam: ;
    rdfs:subPropertyOf rdau:P60511 ;
    owl:sameAs rdam:uniformResourceLocator ;
    skos:definition "Relates a manifestation to the address of a remote access resource."@en ;
    skos:inScheme : ;
    skos:prefLabel "has uniform resource locator"@en .

rdam:P30155 a skos:Concept ;
    reg:name "layout"@en ;
    reg:status <http://metadataregistry.org/uri/RegStatus/1001> ;
    rdfs:domain rdac:C10007 ;
    rdfs:isDefinedBy rdam: ;
    rdfs:subPropertyOf rdau:P60513 ;
    owl:sameAs rdam:layout ;
    skos:definition "Relates a manifestation to the arrangement of text, images, tactile notation, etc., in a resource."@en ;
    skos:inScheme : ;
    skos:prefLabel "has layout"@en .

rdam:P30157 a skos:Concept ;
    reg:name "titleProperOfSeries"@en ;
    reg:status <http://metadataregistry.org/uri/RegStatus/1001> ;
    rdfs:domain rdac:C10007 ;
    rdfs:isDefinedBy rdam: ;
    rdfs:subPropertyOf rdau:P60516 ;
    owl:sameAs rdam:titleProperOfSeries ;
    skos:definition "Relates a manifestation to the chief name of a series (i.e., the title normally used when citing the series)."@en ;
    skos:inScheme : ;
    skos:prefLabel "has title proper of series"@en .

rdam:P30158 a skos:Concept ;
    reg:name "titleProperOfSubseries"@en ;
    reg:status <http://metadataregistry.org/uri/RegStatus/1001> ;
    rdfs:domain rdac:C10007 ;
    rdfs:isDefinedBy rdam: ;
    rdfs:subPropertyOf rdau:P60517 ;
    owl:sameAs rdam:titleProperOfSubseries ;
    skos:definition "Relates a manifestation to the chief name of a subseries (i.e., the title normally used when citing the subseries)."@en ;
    skos:inScheme : ;
    skos:prefLabel "has title proper of subseries"@en .

rdam:P30160 a skos:Concept ;
    reg:name "termsOfAvailability"@en ;
    reg:status <http://metadataregistry.org/uri/RegStatus/1001> ;
    rdfs:domain rdac:C10007 ;
    rdfs:isDefinedBy rdam: ;
    rdfs:subPropertyOf rdau:P60521 ;
    owl:sameAs rdam:termsOfAvailability ;
    skos:definition "Relates a manifestation to the conditions under which the publisher, distributor, etc., will normally supply a resource or the price of a resource."@en ;
    skos:inScheme : ;
    skos:prefLabel "has terms of availability"@en .

rdam:P30166 a skos:Concept ;
    reg:name "issnOfSeries"@en ;
    reg:status <http://metadataregistry.org/uri/RegStatus/1001> ;
    rdfs:domain rdac:C10007 ;
    rdfs:isDefinedBy rdam: ;
    rdfs:subPropertyOf rdau:P60534 ;
    owl:sameAs rdam:issnOfSeries ;
    skos:definition "Relates a manifestation to the identifier assigned to a series by an issn registration agency."@en ;
    skos:inScheme : ;
    skos:prefLabel "has issn of series"@en .

rdam:P30167 a skos:Concept ;
    reg:name "issnOfSubseries"@en ;
    reg:status <http://metadataregistry.org/uri/RegStatus/1001> ;
    rdfs:domain rdac:C10007 ;
    rdfs:isDefinedBy rdam: ;
    rdfs:subPropertyOf rdau:P60535 ;
    owl:sameAs rdam:issnOfSubseries ;
    skos:definition "Relates a manifestation to the identifier assigned to a subseries by an issn registration agency."@en ;
    skos:inScheme : ;
    skos:prefLabel "has issn of subseries"@en .

rdam:P30168 a skos:Concept ;
    reg:name "frequency"@en ;
    reg:status <http://metadataregistry.org/uri/RegStatus/1001> ;
    rdfs:domain rdac:C10007 ;
    rdfs:isDefinedBy rdam: ;
    rdfs:subPropertyOf rdau:P60538 ;
    owl:sameAs rdam:frequency ;
    skos:definition "Relates a manifestation to the intervals at which the issues or parts of a serial or the updates to an integrating resource are issued."@en ;
    skos:inScheme : ;
    skos:prefLabel "has frequency"@en .

rdam:P30186 a skos:Concept ;
    reg:name "mount"@en ;
    reg:status <http://metadataregistry.org/uri/RegStatus/1001> ;
    rdfs:domain rdac:C10007 ;
    rdfs:isDefinedBy rdam: ;
    rdfs:subPropertyOf rdau:P60554 ;
    owl:sameAs rdam:mount ;
    skos:definition "Relates a manifestation to the physical material used for the support or backing to which the base material of a resource has been attached."@en ;
    skos:inScheme : ;
    skos:prefLabel "has mount"@en .

rdam:P30196 a skos:Concept ;
    reg:name "polarity"@en ;
    reg:status <http://metadataregistry.org/uri/RegStatus/1001> ;
    rdfs:domain rdac:C10007 ;
    rdfs:isDefinedBy rdam: ;
    rdfs:subPropertyOf rdau:P60573 ;
    owl:sameAs rdam:polarity ;
    skos:definition "Relates a manifestation to the relationship of the colours and tones in an image to the colours and tones of the object reproduced (e.g., positive, negative)."@en ;
    skos:inScheme : ;
    skos:prefLabel "has polarity"@en .

rdam:P30197 a skos:Concept ;
    reg:name "bookFormat"@en ;
    reg:status <http://metadataregistry.org/uri/RegStatus/1001> ;
    rdfs:domain rdac:C10007 ;
    rdfs:isDefinedBy rdam: ;
    rdfs:subPropertyOf rdau:P60578 ;
    owl:sameAs rdam:bookFormat ;
    skos:definition "Relates a manifestation to the result of folding a printed sheet to form a gathering of leaves (e.g., a sheet folded once to form a folio, twice to form a quarto, three times to form an octavo, etc.)."@en ;
    skos:inScheme : ;
    skos:prefLabel "has book format"@en .

rdam:P30198 a skos:Concept ;
    reg:name "reductionRatio"@en ;
    reg:status <http://metadataregistry.org/uri/RegStatus/1001> ;
    rdfs:domain rdac:C10007 ;
    rdfs:isDefinedBy rdam: ;
    rdfs:subPropertyOf rdau:P60581 ;
    owl:sameAs rdam:reductionRatio ;
    skos:definition "Relates a manifestation to the size of a micro-image in relation to the original from which it was produced."@en ;
    skos:inScheme : ;
    skos:prefLabel "has reduction ratio"@en .

rdam:P30204 a skos:Concept ;
    reg:name "parallelTitleProperOfSeries"@en ;
    reg:status <http://metadataregistry.org/uri/RegStatus/1001> ;
    rdfs:domain rdac:C10007 ;
    rdfs:isDefinedBy rdam: ;
    rdfs:subPropertyOf rdau:P60590 ;
    owl:sameAs rdam:parallelTitleProperOfSeries ;
    skos:definition "Relates a manifestation to the title proper of a series in another language and/or script."@en ;
    skos:inScheme : ;
    skos:prefLabel "has parallel title proper of series"@en .

rdam:P30205 a skos:Concept ;
    reg:name "parallelTitleProperOfSubseries"@en ;
    reg:status <http://metadataregistry.org/uri/RegStatus/1001> ;
    rdfs:domain rdac:C10007 ;
    rdfs:isDefinedBy rdam: ;
    rdfs:subPropertyOf rdau:P60591 ;
    owl:sameAs rdam:parallelTitleProperOfSubseries ;
    skos:definition "Relates a manifestation to the title proper of a subseries in another language and/or script."@en ;
    skos:inScheme : ;
    skos:prefLabel "has parallel title proper of subseries"@en .

rdaw:P10217 rdfs:label "kohderyhmä"@fi ;
    skos:scopeNote "Kohderyhmä tarkoittaa käyttäjäryhmää, jolle aineiston sisältö on tarkoitettu tai jolle sisällön on katsottu sopivan, kuten tiettyä ikäryhmää (esim. lapset, nuoret, aikuiset), opiskelutasoa (esim. peruskoulu, lukio), esteellisyyttä (esim. näkörajoitteiset) tai muuta ryhmittelyä."@fi .

<http://rdvocab.info/termList/RDAMediaType/1002> skos:prefLabel "mikromuoto"@fi ;
    skos:scopeNote "Viestin sisältää pienennettyjä kuvia, jotka eivät ole silmin luettavissa ja se on suunniteltu käytettäväksi mikrofilmin tai mikrokortin lukulaitteen avulla. Käsittää sekä läpinäkyvän että läpinäkymättömän mikromuotoisen viestimen."@fi .

<http://rdvocab.info/termList/RDAMediaType/1003> skos:prefLabel "tietokonekäyttöinen"@fi ;
    skos:scopeNote "Viestin sisältää elektronisia tiedostoja ja on tarkoitettu käytettäväksi tietokoneella. Käsittää sekä tiedostopalvelimien kautta käytettävät etäkäyttöiset viestimet että suorakäyttöiset viestimet kuten tietokonenauhat ja -levyt."@fi .

<http://rdvocab.info/termList/RDAMediaType/1004> skos:prefLabel "mikroskooppinen"@fi ;
    skos:scopeNote "Viestin sisältää hyvin pieniä objekteja, ja se on suunniteltu käytettäväksi laitteella kuten mikroskoopilla, joka paljastaa yksityiskohtia joita ei voi nähdä paljaalla silmällä."@fi .

<http://rdvocab.info/termList/RDAMediaType/1005> skos:prefLabel "heijastettava"@fi ;
    skos:scopeNote "Viestin sisältää liikkuvaa kuvaa tai stillkuvia ja on tarkoitettu käytettäväksi projektorilla kuten filmiprojektorilla, diaprojektorilla tai piirtoheittimellä. Käsittää viestimet, jotka on tarkoitettu heijastamaan sekä kaksiulotteisia että kolmiulotteisia kuvia."@fi .

<http://rdvocab.info/termList/RDAMediaType/1006> skos:prefLabel "stereografinen"@fi ;
    skos:scopeNote "Viestin sisältää stillkuvapareja ja on tarkoitettu käytettäväksi stereoskooppisella tai stereografisella laitteella kolmiulotteisen vaikutelman saamiseksi."@fi .

<http://rdvocab.info/termList/RDAMediaType/1007> skos:prefLabel "käytettävissä ilman laitetta"@fi ;
    skos:scopeNote "Viestimen sisältö havaitaan ihmisaistein ilman välittävää laitetta. Käsittää viestimet, jotka sisältävät visuaalista ja/tai pistekirjoitukseen perustuvaa sisältöä ja jotka on tuotettu menetelmillä kuten painamalla, kaivertamalla, kivipainolla, jne. kohotyönä, kutomalla jne., tai käsin kirjoittamalla, piirtämällä, maalamalla jne. Käsittää myös kolmiulotteisia muotoja ilmaisevat viestimet, kuten veistokset, pienoismallit jne."@fi .

<http://rdvocab.info/termList/RDAMediaType/1008> skos:prefLabel "video"@fi ;
    skos:scopeNote "Viestin sisältää liikkuvaa kuvaa tai stillkuvia ja on suunniteltu käytettäväksi toistolaitteen, kuten videokasettinauhurin tai DVD-soittimen avulla. Käsittää sekä digitaalisesti koodattua että analogista kuvaa sisältävät viestimet."@fi .

:vakioidutFraasit a owl:AnnotationProperty ;
    skos:prefLabel "vakioidutFraasit"@fi .

:vakioidutTermit a owl:AnnotationProperty ;
    skos:prefLabel "vakioidutTermit"@fi .

<http://iflastandards.info/ns/isbd/terms/mediatype/T1001> skos:prefLabel "audio"@fi ;
    skos:scopeNote """Kuuntelemiseen tarkoitetulla välineellä käytettävät aineistot.\r
\r
Tallenteessa olevan äänen kuunteleminen soittovälineillä kuten levysoittimella, kasettisoittimella, CD-soittimella, MP3-soittimella tai muulla mediatoistimella. Audio sisältää sekä digitaalisesti että analogisesti tallennetun äänen."""@fi .

<http://iflastandards.info/ns/isbd/terms/mediatype/T1002> skos:prefLabel "elektroninen"@fi ;
    skos:scopeNote """Termi elektroninen liittyy sekä etä- että suorakäyttöisiin aineistoihin kuten tietokonenauhoihin ja -levyihin.\r
Tietokoneella käytettävät aineistot. Tietokoneella käytettävät tiedostot."""@fi .

<http://iflastandards.info/ns/isbd/terms/mediatype/T1003> skos:prefLabel "mikromuoto"@fi ;
    skos:scopeNote """Pienennetyt kuvat, jotka eivät ole silmin luettavissa vaan käytettävissä mikrofilmin tai mikrokortin lukulaitteen avulla. Mikromuotoinen aineisto voi olla joko läpinäkyvää tai läpinäkymätöntä.\r
Mikrolukulaitteella käytettävät aineistot."""@fi .

<http://iflastandards.info/ns/isbd/terms/mediatype/T1004> skos:prefLabel "mikroskooppinen"@fi ;
    skos:scopeNote """Hyvin pienet kohteet, joiden yksityiskohtia voi tarkastella mikroskooppilaitteella, ei paljaalla silmällä.\r
Mikroskooppilaitteella käytettävät aineistot."""@fi .

<http://iflastandards.info/ns/isbd/terms/mediatype/T1005> skos:prefLabel "heijastettava"@fi ;
    skos:scopeNote """Termi heijastettava liittyy sekä kaksiulotteisiin että kolmiulotteisiin kuviin.\r
Projektorilla käytettävät aineistot. Liikkuva kuva tai stillkuvat, joita katsotaan filmiprojektorin, diaprojektorin tai piirtoheittimen avulla."""@fi .

<http://iflastandards.info/ns/isbd/terms/mediatype/T1006> skos:prefLabel "stereografinen"@fi ;
    skos:scopeNote """Stillkuvaparit, joita voi katsoa kolmiulotteisesti stereokooppisella tai stereografisella laitteella.\r
Stereografisella laitteella käytettävät aineistot."""@fi .

<http://iflastandards.info/ns/isbd/terms/mediatype/T1007> skos:prefLabel "video"@fi ;
    skos:scopeNote """Liikkuva kuva tai stillkuvat, joita katsotaan kuvaa toistavan laitteen, kuten videokasettinauhurin tai DVD-soittimen, avulla. Termi video liittyy sekä digitaaliseen että analogiseen aineistoon.\r
Videolaitteella käytettävät aineistot."""@fi .

<http://iflastandards.info/ns/isbd/terms/mediatype/T1008> skos:prefLabel "useita välittäviä laitteita"@fi ;
    skos:scopeNote "Aineistot, joihin liittyy vähintään kolme eri mediatyyppiä."@fi .

<http://iflastandards.info/ns/isbd/terms/mediatype/T1009> skos:prefLabel "määrittelemätön välittävä laite"@fi ;
    skos:scopeNote "Jos mikään mediatyypeistä ei sovellu, tehdään merkintö ”määrittelemätön välittävä laite”."@fi .

<http://iflastandards.info/ns/isbd/terms/mediatype/T1010> skos:prefLabel "ei välittävää laitetta"@fi ;
    skos:scopeNote "Aineiston käyttöön ei tarvita välinettä."@fi .

<http://metatietosanasto.fi/001> a skos:Concept ;
    skos:inScheme : ;
    skos:prefLabel "Lukuoikeus painetun version tilaajalla."@fi .

<http://metatietosanasto.fi/002> a skos:Concept ;
    skos:inScheme : ;
    skos:prefLabel "Maksullinen tietokanta; sopimus ja käyttäjätunnus pakollinen."@fi .

<http://metatietosanasto.fi/003> a skos:Concept ;
    skos:inScheme : ;
    skos:prefLabel "Saatavana maksullisena myös verkossa."@fi ;
    skos:scopeNote "Painetun julkaisun kuvailun yhteydessä annetaan tieto saatavuudesta verkossa, mutta saatavuus verkon kautta on  maksullista."@fi .

<http://metatietosanasto.fi/004> a skos:Concept ;
    skos:inScheme : ;
    skos:prefLabel "Salassa pidettävä vuoden 20XX loppuun (JulkL 621/1999 24 §)."@fi .

<http://metatietosanasto.fi/005> a skos:Concept ;
    skos:inScheme : ;
    skos:prefLabel "Edellyttää käyttäjätunnuksen."@fi .

<http://metatietosanasto.fi/006> a skos:Concept ;
    skos:inScheme : ;
    skos:prefLabel "Lainataan käyttöoikeuden hankkineiden kirjastojen asiakkaille."@fi .

<http://metatietosanasto.fi/007> a skos:Concept ;
    skos:inScheme : ;
    skos:prefLabel "Käytettävissä lisenssin hankkineiden organisaatioiden verkossa."@fi .

<http://metatietosanasto.fi/008> a skos:Concept ;
    skos:inScheme : ;
    skos:prefLabel "Access limited to [aineiston nimi] affiliated library networks."@en .

<http://metatietosanasto.fi/009> a skos:Concept ;
    skos:inScheme : ;
    skos:prefLabel "Access restricted to subscribers via a username and password or IP address authentication."@en .

<http://metatietosanasto.fi/010> a skos:Concept ;
    skos:inScheme : ;
    skos:prefLabel "Restricted to institutions with a subscription."@en .

<http://metatietosanasto.fi/011> a skos:Concept ;
    skos:inScheme : ;
    skos:prefLabel "Käyttöön ja kopiointiin liittyy rajoituksia."@fi .

<http://metatietosanasto.fi/012> a skos:Concept ;
    skos:inScheme : ;
    skos:prefLabel "Laitteisto-, järjestelmävaatimukset:"@fi .

<http://metatietosanasto.fi/013> a skos:Concept ;
    skos:inScheme : ;
    skos:prefLabel "Laitteistovaatimukset:"@fi .

<http://metatietosanasto.fi/014> a skos:Concept ;
    skos:inScheme : ;
    skos:prefLabel "Järjestelmävaatimukset:"@fi .

<http://metatietosanasto.fi/015> a skos:Concept ;
    skos:inScheme : ;
    skos:prefLabel "Blu-ray-asema"@fi .

<http://metatietosanasto.fi/016> a skos:Concept ;
    skos:inScheme : ;
    skos:prefLabel "DVD-asema"@fi .

<http://metatietosanasto.fi/017> a skos:Concept ;
    skos:inScheme : ;
    skos:prefLabel "Internet-yhteys"@fi .

<http://metatietosanasto.fi/022> a skos:Concept ;
    skos:inScheme : ;
    skos:prefLabel "mobiililaite"@fi ;
    skos:scopeNote "Mobiililaitteiksi kutsutaan laitteita, jotka on suunniteltu mukana kannettaviksi ja jotka soveltuvat tiedon käsittelyyn tai langattomaan tiedonsiirtoon (lähettämiseen ja vastaanottamiseen). Mobiililaitteita ovat esimerkiksi taskutietokoneet, matkapuhelimet, langattoman tiedonsiirron mahdollistavat kannettavat tietokoneet ja sykemittarit, joihin on integroitu tietokone. Lähde: Tietotekniikan termitalkoot, 2005-05-20"@fi .

<http://metatietosanasto.fi/023> a skos:Concept ;
    skos:inScheme : ;
    skos:prefLabel "MP3-tiedostoja toistava laite"@fi .

<http://metatietosanasto.fi/024> a skos:Concept ;
    skos:inScheme : ;
    skos:prefLabel "USB-portti"@fi ;
    skos:scopeNote "USB-muistille"@fi .

<http://metatietosanasto.fi/025> a skos:Concept ;
    skos:inScheme : ;
    skos:prefLabel "avainnimeke"@fi ;
    skos:scopeNote "Jatkuvan julkaisun ainutkertainen nimi, jonka määrittää ISSN-verkosto ja joka liittyy ISSN-tunnukseen erottamattomasti."@fi .

<http://metatietosanasto.fi/026> a skos:Concept ;
    skos:inScheme : ;
    skos:prefLabel "epäitsenäinen nimeke"@fi ;
    skos:scopeNote "Nimeke, joka itsessään on riittämätön julkaisun tunnistamiseen ja joka vaatii lisäkseen yhteisnimekkeen tai pääjulkaisun tai pääsarjan nimekkeen. Tällaisia nimekkeitä voivat olla esim. moniosaisen teoksen osamerkinnöt, lohkosarjan nimekkeet sekä eräät suplementtien ja alasarjojen nimekkeet. (engl. dependent title)"@fi .

<http://metatietosanasto.fi/026_1> a skos:Concept ;
    skos:inScheme : ;
    skos:prefLabel "erottuva nimeke"@fi ;
    skos:scopeNote "Erottuva nimeke näkyy tavallisen nimekkeen lisäksi yksittäisissä numeroissa ja numero voi olla tunnettu sen perusteella."@fi .

<http://metatietosanasto.fi/027> a skos:Concept ;
    skos:inScheme : ;
    skos:prefLabel "juokseva nimeke"@fi ;
    skos:scopeNote "Nimeke on painettu jokaisen sivun ylä- tai alamarginaaliin."@fi .

<http://metatietosanasto.fi/028> a skos:Concept ;
    skos:inScheme : ;
    skos:prefLabel "kansinimeke"@fi .

<http://metatietosanasto.fi/032> a skos:Concept ;
    skos:inScheme : ;
    skos:prefLabel "osan nimeke"@fi .

<http://metatietosanasto.fi/033> a skos:Concept ;
    skos:inScheme : ;
    skos:prefLabel "otsikkonimeke"@fi ;
    skos:scopeNote "Nimeke, joka esiintyy julkaisussa tekstin ensimmäisen sivun alussa. (engl. caption title)"@fi .

<http://metatietosanasto.fi/034> a skos:Concept ;
    skos:inScheme : ;
    skos:prefLabel "päänimeke"@fi .

<http://metatietosanasto.fi/035> a skos:Concept ;
    skos:inScheme : ;
    skos:prefLabel "rinnakkaisnimeke"@fi .

<http://metatietosanasto.fi/036> a skos:Concept ;
    skos:inScheme : ;
    skos:prefLabel "selkänimeke"@fi .

<http://metatietosanasto.fi/037> a skos:Concept ;
    skos:inScheme : ;
    skos:prefLabel "vaihtoehtoinen nimeke"@fi .

<http://metatietosanasto.fi/038> a skos:Concept ;
    skos:inScheme : ;
    skos:prefLabel "varianttinimeke"@fi ;
    skos:scopeNote "Päänimekkeestä poikkeava nimekkeen muoto. (engl. variant title)"@fi .

<http://metatietosanasto.fi/039> a skos:Concept ;
    skos:inScheme : ;
    skos:prefLabel "yhteisnimeke"@fi ;
    skos:scopeNote "Se osa nimekettä, joka ryhmällä yhteenkuuluvia julkaisuja on yhteinen niiden omien nimekkeiden lisäksi. Yhteisnimeke osoittaa tämän yhteenkuuluvuuden. Sen ja osan nimekkeen avulla julakisu tunnistetaan. Yhteisnimeke voi merkitä myös pääjulkaisun ja sen suplementin sekä pääsarjan ja sen alasarjojen nimekkeiden yhteistä osaa, kun suplementilla tai alasarjoilla on epäitsenäinen nimeke. (engl. common title)"@fi .

<http://metatietosanasto.fi/040> a skos:Concept ;
    skos:inScheme : ;
    skos:prefLabel "alanimeke kannessa:"@fi .

<http://metatietosanasto.fi/041> a skos:Concept ;
    skos:inScheme : ;
    skos:prefLabel "alanimeke selässä:"@fi .

<http://metatietosanasto.fi/042> a skos:Concept ;
    skos:inScheme : ;
    skos:prefLabel "alanimeke esiössä:"@fi .

<http://metatietosanasto.fi/043> a skos:Concept ;
    skos:inScheme : ;
    skos:prefLabel "ylänimeke kannessa:"@fi .

<http://metatietosanasto.fi/044> a skos:Concept ;
    skos:inScheme : ;
    skos:prefLabel "ylänimeke selässä:"@fi .

<http://metatietosanasto.fi/045> a skos:Concept ;
    skos:inScheme : ;
    skos:prefLabel "ylänimeke esiössä:"@fi .

<http://metatietosanasto.fi/046> a skos:Concept ;
    skos:inScheme : ;
    skos:prefLabel "lyhenne avattuna kannessa:"@fi .

<http://metatietosanasto.fi/047> a skos:Concept ;
    skos:inScheme : ;
    skos:prefLabel "nimekkeen lähde:"@fi .

<http://metatietosanasto.fi/048> a skos:Concept ;
    skos:inScheme : ;
    skos:prefLabel "nimeke ensimmäiseltä nuottisivulta"@fi .

<http://metatietosanasto.fi/049> a skos:Concept ;
    skos:inScheme : ;
    skos:prefLabel "nimeke etusivulta"@fi .

<http://metatietosanasto.fi/050> a skos:Concept ;
    skos:inScheme : ;
    skos:prefLabel "nimeke esiöstä"@fi .

<http://metatietosanasto.fi/051> a skos:Concept ;
    skos:inScheme : ;
    skos:prefLabel "nimeke irtopäällyksestä"@fi .

<http://metatietosanasto.fi/052> a skos:Concept ;
    skos:inScheme : ;
    skos:prefLabel "nimeke kannesta"@fi .

<http://metatietosanasto.fi/053> a skos:Concept ;
    skos:inScheme : ;
    skos:prefLabel "nimeke kannen kääntöpuolelta"@fi .

<http://metatietosanasto.fi/054> a skos:Concept ;
    skos:inScheme : ;
    skos:prefLabel "nimeke kotelosta"@fi .

<http://metatietosanasto.fi/055> a skos:Concept ;
    skos:inScheme : ;
    skos:prefLabel "nimeke kuvailulehdeltä"@fi .

<http://metatietosanasto.fi/056> a skos:Concept ;
    skos:inScheme : ;
    skos:prefLabel "nimeke levystä"@fi .

<http://metatietosanasto.fi/057> a skos:Concept ;
    skos:inScheme : ;
    skos:prefLabel "nimeke alkuteksteistä"@fi .

<http://metatietosanasto.fi/058> a skos:Concept ;
    skos:inScheme : ;
    skos:prefLabel "nimeke lopputeksteistä"@fi .

<http://metatietosanasto.fi/059> a skos:Concept ;
    skos:inScheme : ;
    skos:prefLabel "nimeke nimiönäytöltä"@fi .

<http://metatietosanasto.fi/060> a skos:Concept ;
    skos:inScheme : ;
    skos:prefLabel "nimeke nimiösivun kääntöpuolelta"@fi .

<http://metatietosanasto.fi/061> a skos:Concept ;
    skos:inScheme : ;
    skos:prefLabel "nimeke ohjekirjasta"@fi .

<http://metatietosanasto.fi/062> a skos:Concept ;
    skos:inScheme : ;
    skos:prefLabel "nimeke pakkauksesta"@fi .

<http://metatietosanasto.fi/063> a skos:Concept ;
    skos:inScheme : ;
    skos:prefLabel "nimeke selästä"@fi .

<http://metatietosanasto.fi/064> a skos:Concept ;
    skos:inScheme : ;
    skos:prefLabel "nimeke sähköpostin aiheriviltä"@fi .

<http://metatietosanasto.fi/065> a skos:Concept ;
    skos:inScheme : ;
    skos:prefLabel "nimeke  tekstin alusta"@fi .

<http://metatietosanasto.fi/066> a skos:Concept ;
    skos:inScheme : ;
    skos:prefLabel "nimeke  tekstiliitteestä"@fi .

<http://metatietosanasto.fi/067> a skos:Concept ;
    skos:inScheme : ;
    skos:prefLabel "nimeke  toimitustiedoista/ toimitustietolaatikosta"@fi .

<http://metatietosanasto.fi/068> a skos:Concept ;
    skos:inScheme : ;
    skos:prefLabel "aukkokirja"@fi .

<http://metatietosanasto.fi/069> a skos:Concept ;
    skos:inScheme : ;
    skos:prefLabel "juliste"@fi ;
    skos:scopeNote "Jstak tiedottava, jtak mainostava t. propagoiva (suurikokoinen) tav. kuvallinen painotuote; seinällä pidettävä suuri painokuva (Kielitoimiston sanakirja) (engl. poster)"@fi .

<http://metatietosanasto.fi/069_1> a skos:Concept ;
    skos:inScheme : ;
    skos:prefLabel "karttalehti"@fi .

<http://metatietosanasto.fi/070> a skos:Concept ;
    skos:inScheme : ;
    skos:prefLabel "karttaliite"@fi .

<http://metatietosanasto.fi/075> a skos:Concept ;
    skos:inScheme : ;
    skos:prefLabel "kuvasalkku"@fi ;
    skos:scopeNote "Kotelo, joka sisältää esim. grafiikanlehtiä, kuvakortteja tms. (Kuvailusäännöt)"@fi .

<http://metatietosanasto.fi/076> a skos:Concept ;
    skos:inScheme : ;
    skos:prefLabel "kuvataulu"@fi .

<http://metatietosanasto.fi/077> a skos:Concept ;
    skos:inScheme : ;
    skos:prefLabel "lelu"@fi .

<http://metatietosanasto.fi/078> a skos:Concept ;
    skos:inScheme : ;
    skos:prefLabel "levy"@fi .

<http://metatietosanasto.fi/093> a skos:Concept ;
    skos:inScheme : ;
    skos:prefLabel "opetuskuva"@fi .

<http://metatietosanasto.fi/094> a skos:Concept ;
    skos:inScheme : ;
    skos:prefLabel "opetustaulu"@fi .

<http://metatietosanasto.fi/095> a skos:Concept ;
    skos:inScheme : ;
    skos:prefLabel "painokuva"@fi .

<http://metatietosanasto.fi/099> a skos:Concept ;
    skos:inScheme : ;
    skos:prefLabel "piirtoheitinkalvo"@fi .

<http://metatietosanasto.fi/100> a skos:Concept ;
    skos:inScheme : ;
    skos:prefLabel "piirtoheitinkalvopohja"@fi .

<http://metatietosanasto.fi/101> a skos:Concept ;
    skos:inScheme : ;
    skos:prefLabel "USB-muisti"@fi .

<http://metatietosanasto.fi/106> a skos:Concept ;
    skos:inScheme : ;
    skos:prefLabel "haitarikirja"@fi ;
    skos:scopeNote "Kirja, jonka sivut on taitettu haitarimuotoon.Onix-termi. (engl. fold-out book or chart)"@fi .

<http://metatietosanasto.fi/107> a skos:Concept ;
    skos:inScheme : ;
    skos:prefLabel "kangaskirja"@fi ;
    skos:scopeNote "Kirja, jonka kaikki sivut on painettu tekstiilille. Onix-termi. (engl. rag book)"@fi .

<http://metatietosanasto.fi/108> a skos:Concept ;
    skos:inScheme : ;
    skos:prefLabel "katselukirja"@fi ;
    skos:scopeNote "Usein tekstitön lastenkirja jossa pääpaino on kuvituksella.Onix-termi. (engl. picture book)"@fi .

<http://metatietosanasto.fi/109> a skos:Concept ;
    skos:inScheme : ;
    skos:prefLabel "koskettelukirja"@fi ;
    skos:scopeNote "Värikkäitä, tunnusteltavia kuvia sisältävä kuvakirja, joka on tarkoitettu sokealle tai heikkonäköiselle lapselle. Kirjan teksti voi olla pistekirjoituksella, isokirjoituksella tai tavallisin kirjaimin. Kirjassa voi olla mukana myös äänite. Tarinat ovat tekijöiden sepittämiä tai sovituksia tutuista saduista, loruista tai runoista. Wikipedia, 23.1.2013."@fi .

<http://metatietosanasto.fi/110> a skos:Concept ;
    skos:inScheme : ;
    skos:prefLabel "kurkistuskirja"@fi ;
    skos:scopeNote "Kirja, jonka sivuilla on avattavia luukkuja.Onix-termi. (engl. lift-the-flap book)"@fi .

<http://metatietosanasto.fi/111> a skos:Concept ;
    skos:inScheme : ;
    skos:prefLabel "kuvatehostekirja"@fi ;
    skos:scopeNote "Kirja, jossa on erilaisia kuvatehosteita, esim. hologrammikuvia tai liikuteltavia kuvia. Kaunokki-termi"@fi .

<http://metatietosanasto.fi/112> a skos:Concept ;
    skos:inScheme : ;
    skos:prefLabel "kääntökirja"@fi ;
    skos:scopeNote "Julkaisu, jonka teksti ja sivunumerointi alkavat vastakkaisilta puolilta. Yleensä kyseessä on kaksikielinen julkaisu. Onix-termi. (engl. turn-around book)"@fi .

<http://metatietosanasto.fi/113> a skos:Concept ;
    skos:inScheme : ;
    skos:prefLabel "lelukirja"@fi ;
    skos:scopeNote "Kirja, joka toimii myös leluna, tai kirja, jonka osana on lelu. Onix-termi. (engl. book-as-toy)"@fi .

<http://metatietosanasto.fi/114> a skos:Concept ;
    skos:inScheme : ;
    skos:prefLabel "lippakirja"@fi ;
    skos:scopeNote "Minitaskukirja (8 x 12 cm), jonka teksti on painettu horisontaalisesti. Onix-termi.(eng. flipback)"@fi .

<http://metatietosanasto.fi/115> a skos:Concept ;
    skos:inScheme : ;
    skos:prefLabel "liuskakirja"@fi ;
    skos:scopeNote "Kirja, jossa sivut on leikattu liuskoiksi niin, että liuskoja yhdistelemällä voidaan vaihtaa esim. hahmojen osat toisiksi. Kaunokki-termi.(engl. flap book)"@fi .

<http://metatietosanasto.fi/116> a skos:Concept ;
    skos:inScheme : ;
    skos:prefLabel "magneettikirja"@fi ;
    skos:scopeNote "Kirja, joka voidaan siinä olevan magneetin avulla kiinnittää metallialustaan. Kaunokki-termi. (engl. magnet book)"@fi .

<http://metatietosanasto.fi/117> a skos:Concept ;
    skos:inScheme : ;
    skos:prefLabel "muotoonleikattu kirja"@fi ;
    skos:scopeNote "KMuuhun kuin perinteiseen nelikulmaiseen muotoon leikattu kirja. Onix-termi. (engl. die-cut book)"@fi .

<http://metatietosanasto.fi/118> a skos:Concept ;
    skos:inScheme : ;
    skos:prefLabel "paksulehtinen kirja"@fi ;
    skos:scopeNote "Kirja, jonka sivut ovat paksut niihin tarttumisen helpottamiseksi. Julkaisun kaikki sivut on painettu esimerkiksi pahville. Kaunokki-termi."@fi .

<http://metatietosanasto.fi/119> a skos:Concept ;
    skos:inScheme : ;
    skos:prefLabel "palapelikirja"@fi ;
    skos:scopeNote "Kirja, jossa on mukana palapelin palasia. Kaunokki-termi.   (engl. puzzle / jigsaw book)"@fi .

<http://metatietosanasto.fi/120> a skos:Concept ;
    skos:inScheme : ;
    skos:prefLabel "pienoiskokoinen kirja"@fi ;
    skos:scopeNote "Pienikokoinen, esimerkiksi korkeudeltaan alle 12 cm oleva kirja. Onix-termi. (engl. miniature book)"@fi .

<http://metatietosanasto.fi/121> a skos:Concept ;
    skos:inScheme : ;
    skos:prefLabel "pop-up-kirja"@fi ;
    skos:scopeNote "Näyttämö- tai ponnahduskirja, jonka sivuilla on esiin taittuvia kuvia. Onix-termi. (engl. pop-up book)"@fi .

<http://metatietosanasto.fi/122> a skos:Concept ;
    skos:inScheme : ;
    skos:prefLabel "siirtotarrakirja"@fi ;
    skos:scopeNote "Kirja, jossa on mukana sen sivuille liimattaviksi tarkoitettuja tarroja. Tarrat materiaalista, joita voi liimata useaan kertaan. (engl. transfer sticker book)"@fi .

<http://metatietosanasto.fi/123> a skos:Concept ;
    skos:inScheme : ;
    skos:prefLabel "tarrakirja"@fi ;
    skos:scopeNote "Kirja, jossa on mukana sen sivuille pysyvästi liimattaviksi tarkoitettuja tarroja.Onix-termi. (engl. sticker-book)"@fi .

<http://metatietosanasto.fi/124> a skos:Concept ;
    skos:inScheme : ;
    skos:prefLabel "tunnustelukirja"@fi ;
    skos:scopeNote "Kirja, jossa on erilaisia koskettelupintoja eri materiaaleista. Onix-termi. (engl touch-and-feel book )"@fi .

<http://metatietosanasto.fi/125> a skos:Concept ;
    skos:inScheme : ;
    skos:prefLabel "äänitehostekirja"@fi ;
    skos:scopeNote "Kirja, joka sisältää ääniefektejä tai musiikkia. Onix-termi. (engl. Sound story / 'noisy' book )"@fi .

<http://metatietosanasto.fi/126> a skos:Concept ;
    skos:inScheme : ;
    skos:prefLabel "Julkaisussa rengaskierteen peittävä selkä."@fi .

<http://metatietosanasto.fi/127> a skos:Concept ;
    skos:inScheme : ;
    skos:prefLabel "Julkaisussa irrotettavia paloja."@fi .

<http://metatietosanasto.fi/128> a skos:Concept ;
    skos:inScheme : ;
    skos:prefLabel "Julkaisussa liikuteltavia/irrotettavia/vaihtuvia kuvia."@fi .

<http://metatietosanasto.fi/129> a skos:Concept ;
    skos:inScheme : ;
    skos:prefLabel "Julkaisussa pyöritettäviä kiekkoja."@fi .

<http://metatietosanasto.fi/130> a skos:Concept ;
    skos:inScheme : ;
    skos:prefLabel "Julkaisussa sapluunoita."@fi .

<http://metatietosanasto.fi/131> a skos:Concept ;
    skos:inScheme : ;
    skos:prefLabel "Julkaisussa avattavia luukkuja."@fi .

<http://metatietosanasto.fi/132> a skos:Concept ;
    skos:inScheme : ;
    skos:prefLabel "Takakannen/etukannen sisäpuolelle kiinnitetyssä kotelossa/taskussa xxx. (esim. kynä)"@fi .

<http://metatietosanasto.fi/133> a skos:Concept ;
    skos:inScheme : ;
    skos:prefLabel "Varustettu kantokahvalla."@fi .

<http://metatietosanasto.fi/134> a skos:Concept ;
    skos:inScheme : ;
    skos:prefLabel "Varustettu lukolla."@fi .

<http://metatietosanasto.fi/135> a skos:Concept ;
    skos:inScheme : ;
    skos:prefLabel "Varustettu reunahakemistolla."@fi .

<http://metatietosanasto.fi/161> a skos:Concept ;
    skos:inScheme : ;
    skos:prefLabel "kustantajan nimi"@fi ;
    skos:scopeNote "aineiston kustantamisesta, julkaisemisesta tai ilmestymisestä vastuussa olevan henkilön, suvun tai yhteisön nimi. Vanhojen painettujen aineistojen kirjanpainajia ja kirjakauppiaita pidetään kustantajina"@fi .

<http://metatietosanasto.fi/162> a skos:Concept ;
    skos:inScheme : ;
    skos:prefLabel "Jakajan  nimi"@fi ;
    skos:scopeNote "julkaistun aineiston jakelemisesta vastuussa olevan henkilön, suvun tai yhteisön nimi."@fi .

<http://metatietosanasto.fi/163> a skos:Concept ;
    skos:inScheme : ;
    skos:prefLabel "Valmistajan  nimi"@fi ;
    skos:scopeNote "julkaistun aineiston painamisesta, monistamisesta, kirjasinten valamisesta jne. vastuussa olevan henkilön, suvun tai yhteisön nimi."@fi .

<http://metatietosanasto.fi/164> a skos:Concept ;
    skos:inScheme : ;
    skos:prefLabel "copyright-vuosi"@fi ;
    skos:scopeNote "aika, joka liittyy copyright-säädösten tai vastaavien säädösten alaiseen copyright-suojaukseen. Copyright-vuosiin sisältyvät P-ajat (phonogram) (äänitteiden copyright-suojaukseen liittyvät ajat)."@fi .

<http://metatietosanasto.fi/165> a skos:Concept ;
    skos:inScheme : ;
    skos:prefLabel "sid."@fi ;
    skos:scopeNote "manifestaation tunnisteen lisäys kovakantiselle kirjalle"@fi .

<http://metatietosanasto.fi/166> a skos:Concept ;
    skos:inScheme : ;
    skos:prefLabel "nid."@fi ;
    skos:scopeNote "manifestaation tunnisteen lisäys pehmeäkantiselle kirjalle"@fi .

<http://metatietosanasto.fi/167> a skos:Concept ;
    skos:inScheme : ;
    skos:prefLabel "rengaskirja"@fi ;
    skos:scopeNote "manifestaation tunnisteen lisäys"@fi .

<http://metatietosanasto.fi/168> a skos:Concept ;
    skos:inScheme : ;
    skos:prefLabel "kansio"@fi ;
    skos:scopeNote "manifestaation tunnisteen lisäys"@fi .

<http://metatietosanasto.fi/169> a skos:Concept ;
    skos:inScheme : ;
    skos:prefLabel "irtolehtiä"@fi ;
    skos:scopeNote "manifestaation tunnisteen lisäys"@fi .

<http://metatietosanasto.fi/170> a skos:Concept ;
    skos:inScheme : ;
    skos:prefLabel "kotelo"@fi ;
    skos:scopeNote "manifestaation tunnisteen lisäys"@fi .

<http://metatietosanasto.fi/171> a skos:Concept ;
    skos:inScheme : ;
    skos:prefLabel "virh."@fi ;
    skos:scopeNote "manifestaation tunnisteen lisäys"@fi .

<http://metatietosanasto.fi/172> a skos:Concept ;
    skos:inScheme : ;
    skos:prefLabel "korj."@fi ;
    skos:scopeNote "manifestaation tunnisteen lisäys"@fi .

<http://metatietosanasto.fi/173> a skos:Concept ;
    skos:inScheme : ;
    skos:prefLabel "GTIN-koodista"@fi ;
    skos:scopeNote "manifestaation tunnisteen lisäys"@fi .

rdam:P30001 a skos:Concept ;
    reg:name "carrierType"@en ;
    reg:status <http://metadataregistry.org/uri/RegStatus/1001> ;
    rdfs:domain rdac:C10007 ;
    rdfs:isDefinedBy rdam: ;
    rdfs:subPropertyOf rdau:P60048 ;
    owl:sameAs rdam:carrierType ;
    skos:definition "Relates a manifestation to a categorization reflecting the format of the storage medium and housing of a carrier in combination with the type of intermediation device required to view, play, run, etc., the content of a resource."@en ;
    skos:inScheme : ;
    skos:prefLabel "has carrier type"@en .

rdam:P30002 a skos:Concept ;
    reg:name "mediaType"@en ;
    reg:status <http://metadataregistry.org/uri/RegStatus/1001> ;
    rdfs:domain rdac:C10007 ;
    rdfs:isDefinedBy rdam: ;
    rdfs:subPropertyOf rdau:P60050 ;
    owl:sameAs rdam:mediaType ;
    skos:definition "Relates a manifestation to a categorization reflecting the general type of intermediation device required to view, play, run, etc., the content of a resource."@en ;
    skos:inScheme : ;
    skos:prefLabel "has media type"@en .

rdam:P30006 a skos:Concept ;
    reg:name "regionalEncoding"@en ;
    reg:status <http://metadataregistry.org/uri/RegStatus/1001> ;
    rdfs:domain rdac:C10007 ;
    rdfs:isDefinedBy rdam: ;
    rdfs:subPropertyOf rdam:P30124,
        rdau:P60059 ;
    owl:sameAs rdam:regionalEncoding ;
    skos:definition "Relates a manifestation to a code identifying the region of the world for which a videodisc has been encoded and preventing the disc from being played on a player sold in a different region."@en ;
    skos:inScheme : ;
    skos:prefLabel "has regional encoding"@en .

rdam:P30018 a skos:Concept ;
    reg:name "fileType"@en ;
    reg:status <http://metadataregistry.org/uri/RegStatus/1001> ;
    rdfs:domain rdac:C10007 ;
    rdfs:isDefinedBy rdam: ;
    rdfs:subPropertyOf rdam:P30124,
        rdau:P60093 ;
    owl:sameAs rdam:fileType ;
    skos:definition "Relates a manifestation to a general type of data content encoded in a computer file."@en ;
    skos:inScheme : ;
    skos:prefLabel "has file type"@en .

rdam:P30032 a skos:Concept ;
    reg:name "analysisOfManifestation"@en ;
    reg:status <http://metadataregistry.org/uri/RegStatus/1001> ;
    rdfs:domain rdac:C10007 ;
    rdfs:isDefinedBy rdam: ;
    rdfs:range rdac:C10007 ;
    rdfs:subPropertyOf rdam:P30023,
        rdau:P60239 ;
    owl:sameAs rdam:analysisOfManifestation ;
    skos:definition "Relates a manifestation to a manifestation that has been examined to identify its components and their relations."@en ;
    skos:inScheme : ;
    skos:prefLabel "is analysis of (manifestation)"@en .

rdam:P30034 a skos:Concept ;
    reg:name "evaluationOfManifestation"@en ;
    reg:status <http://metadataregistry.org/uri/RegStatus/1001> ;
    rdfs:domain rdac:C10007 ;
    rdfs:isDefinedBy rdam: ;
    rdfs:range rdac:C10007 ;
    rdfs:subPropertyOf rdam:P30023,
        rdau:P60255 ;
    owl:sameAs rdam:evaluationOfManifestation ;
    skos:definition "Relates a manifestation to a manifestation that is examined or judged."@en ;
    skos:inScheme : ;
    skos:prefLabel "is evaluation of (manifestation)"@en .

rdam:P30041 a skos:Concept ;
    reg:name "reviewOfManifestation"@en ;
    reg:status <http://metadataregistry.org/uri/RegStatus/1001> ;
    rdfs:domain rdac:C10007 ;
    rdfs:isDefinedBy rdam: ;
    rdfs:range rdac:C10007 ;
    rdfs:subPropertyOf rdam:P30023,
        rdau:P60288 ;
    owl:sameAs rdam:reviewOfManifestation ;
    skos:definition "Relates a manifestation to a manifestation used as the basis for a brief evaluation."@en ;
    skos:inScheme : ;
    skos:prefLabel "is review of (manifestation)"@en .

rdam:P30042 a skos:Concept ;
    reg:name "critiqueOfManifestation"@en ;
    reg:status <http://metadataregistry.org/uri/RegStatus/1001> ;
    rdfs:domain rdac:C10007 ;
    rdfs:isDefinedBy rdam: ;
    rdfs:range rdac:C10007 ;
    rdfs:subPropertyOf rdam:P30023,
        rdau:P60292 ;
    owl:sameAs rdam:critiqueOfManifestation ;
    skos:definition "Relates a manifestation to a manifestation used as the basis for a critical evaluation."@en ;
    skos:inScheme : ;
    skos:prefLabel "is critique of (manifestation)"@en .

rdam:P30044 a skos:Concept ;
    reg:name "commentaryOnManifestation"@en ;
    reg:status <http://metadataregistry.org/uri/RegStatus/1001> ;
    rdfs:domain rdac:C10007 ;
    rdfs:isDefinedBy rdam: ;
    rdfs:range rdac:C10007 ;
    rdfs:subPropertyOf rdam:P30023,
        rdau:P60298 ;
    owl:sameAs rdam:commentaryOnManifestation ;
    skos:definition "Relates a manifestation to a manifestation used as the basis for a set of explanatory or critical notes."@en ;
    skos:inScheme : ;
    skos:prefLabel "is commentary on (manifestation)"@en .

rdam:P30050 a skos:Concept ;
    reg:name "noteOnIssuePartOrIterationUsedAsTheBasisForIdentificationOfTheResource"@en ;
    reg:status <http://metadataregistry.org/uri/RegStatus/1001> ;
    rdfs:domain rdac:C10007 ;
    rdfs:isDefinedBy rdam: ;
    rdfs:subPropertyOf rdam:P30137,
        rdau:P60122 ;
    owl:sameAs rdam:noteOnIssuePartOrIterationUsedAsTheBasisForIdentificationOfTheResource ;
    skos:definition "Relates a manifestation to a note identifying the issue or part of a multipart monograph or serial, or the iteration of an integrating resource that has been used as the basis for the identification of a resource."@en ;
    skos:inScheme : ;
    skos:prefLabel "has note on issue, part, or iteration used as the basis for identification of the resource"@en .

rdam:P30051 a skos:Concept ;
    reg:name "noteOnChangesInCarrierCharacteristics"@en ;
    reg:status <http://metadataregistry.org/uri/RegStatus/1001> ;
    rdfs:domain rdac:C10007 ;
    rdfs:isDefinedBy rdam: ;
    rdfs:subPropertyOf rdam:P30137,
        rdau:P60124 ;
    owl:sameAs rdam:noteOnChangesInCarrierCharacteristics ;
    skos:definition "Relates a manifestation to a note on changes in the characteristics of the carrier that occur in subsequent issues or parts of a resource issued in successive parts or between iterations of an integrating resource."@en ;
    skos:inScheme : ;
    skos:prefLabel "has note on changes in carrier characteristics"@en .

rdam:P30054 a skos:Concept ;
    reg:name "noteOnProductionStatement"@en ;
    reg:status <http://metadataregistry.org/uri/RegStatus/1001> ;
    rdfs:domain rdac:C10007 ;
    rdfs:isDefinedBy rdam: ;
    rdfs:subPropertyOf rdam:P30137,
        rdau:P60127 ;
    owl:sameAs rdam:noteOnProductionStatement ;
    skos:definition "Relates a manifestation to a note providing details on place of production, producer, or date of production, or information on changes in the place of production, producer, or producer’s name."@en ;
    skos:inScheme : ;
    skos:prefLabel "has note on production statement"@en .

rdam:P30056 a skos:Concept ;
    reg:name "noteOnFrequency"@en ;
    reg:status <http://metadataregistry.org/uri/RegStatus/1001> ;
    rdfs:domain rdac:C10007 ;
    rdfs:isDefinedBy rdam: ;
    rdfs:subPropertyOf rdam:P30137,
        rdau:P60129 ;
    owl:sameAs rdam:noteOnFrequency ;
    skos:definition "Relates a manifestation to a note providing details on the currency of the contents, on the frequency of release of issues or parts of a serial or the frequency of updates to an integrating resource, or on changes in frequency."@en ;
    skos:inScheme : ;
    skos:prefLabel "has note on frequency"@en .

rdam:P30057 a skos:Concept ;
    reg:name "noteOnStatementOfResponsibility"@en ;
    reg:status <http://metadataregistry.org/uri/RegStatus/1001> ;
    rdfs:domain rdac:C10007 ;
    rdfs:isDefinedBy rdam: ;
    rdfs:subPropertyOf rdam:P30137,
        rdau:P60130 ;
    owl:sameAs rdam:noteOnStatementOfResponsibility ;
    skos:definition "Relates a manifestation to a note providing information on a person, family, or corporate body not named in a statement of responsibility to whom responsibility for the intellectual or artistic content of the resource has been attributed, on variant forms of names appearing in the resource, on changes in statements of responsibility, or on other details relating to a statement of responsibility."@en ;
    skos:inScheme : ;
    skos:prefLabel "has note on statement of responsibility"@en .

rdam:P30058 a skos:Concept ;
    reg:name "noteOnSeriesStatement"@en ;
    reg:status <http://metadataregistry.org/uri/RegStatus/1001> ;
    rdfs:domain rdac:C10007 ;
    rdfs:isDefinedBy rdam: ;
    rdfs:subPropertyOf rdam:P30137,
        rdau:P60131 ;
    owl:sameAs rdam:noteOnSeriesStatement ;
    skos:definition "Relates a manifestation to a note providing information on complex series statements, incorrect numbering within series, or changes in series statements."@en ;
    skos:inScheme : ;
    skos:prefLabel "has note on series statement"@en .

rdam:P30062 a skos:Concept ;
    reg:name "noteOnNumberingOfSerials"@en ;
    reg:status <http://metadataregistry.org/uri/RegStatus/1001> ;
    rdfs:domain rdac:C10007 ;
    rdfs:isDefinedBy rdam: ;
    rdfs:subPropertyOf rdam:P30137,
        rdau:P60135 ;
    owl:sameAs rdam:noteOnNumberingOfSerials ;
    skos:definition "Relates a manifestation to a note providing information on the numbering of the first and/or last issue or part, on complex or irregular numbering (including numbering errors), or on the period covered by a volume, issue, part, etc."@en ;
    skos:inScheme : ;
    skos:prefLabel "has note on numbering of serials"@en .

rdam:P30065 a skos:Concept ;
    reg:name "publishersNumberForMusic"@en ;
    reg:status <http://metadataregistry.org/uri/RegStatus/1001> ;
    rdfs:domain rdac:C10007 ;
    rdfs:isDefinedBy rdam: ;
    rdfs:subPropertyOf rdam:P30004,
        rdau:P60139 ;
    owl:sameAs rdam:publishersNumberForMusic ;
    skos:definition "Relates a manifestation to a numbering designation assigned to a resource by a music publisher, appearing normally only on the title page, the cover, and/or the first page of music."@en ;
    skos:inScheme : ;
    skos:prefLabel "has publisher's number for music"@en .

rdam:P30066 a skos:Concept ;
    reg:name "plateNumberForMusic"@en ;
    reg:status <http://metadataregistry.org/uri/RegStatus/1001> ;
    rdfs:domain rdac:C10007 ;
    rdfs:isDefinedBy rdam: ;
    rdfs:subPropertyOf rdam:P30004,
        rdau:P60140 ;
    owl:sameAs rdam:plateNumberForMusic ;
    skos:definition "Relates a manifestation to a numbering designation assigned to a resource by a music publisher."@en ;
    skos:inScheme : ;
    skos:prefLabel "has plate number for music"@en ;
    skos:scopeNote "The number is usually printed at the bottom of each page, and sometimes also appears on the title page."@en .

rdam:P30067 a skos:Concept ;
    reg:name "broadcaster"@en ;
    reg:status <http://metadataregistry.org/uri/RegStatus/1001> ;
    rdfs:domain rdac:C10007 ;
    rdfs:isDefinedBy rdam: ;
    rdfs:range rdac:C10002 ;
    rdfs:subPropertyOf rdam:P30083,
        rdau:P60407 ;
    owl:inverseOf rdaa:P50168 ;
    owl:sameAs rdam:broadcaster ;
    skos:definition "Relates a manifestation to a person, family, or corporate body involved in broadcasting a manifestation to an audience via radio, television, webcast, etc."@en ;
    skos:inScheme : ;
    skos:prefLabel "has broadcaster"@en .

rdam:P30068 a skos:Concept ;
    reg:name "filmDistributor"@en ;
    reg:status <http://metadataregistry.org/uri/RegStatus/1001> ;
    rdfs:domain rdac:C10007 ;
    rdfs:isDefinedBy rdam: ;
    rdfs:range rdac:C10002 ;
    rdfs:subPropertyOf rdam:P30080,
        rdau:P60408 ;
    owl:inverseOf rdaa:P50169 ;
    owl:sameAs rdam:filmDistributor ;
    skos:definition "Relates a manifestation to a person, family, or corporate body involved in distributing a moving image manifestation to theatres or other distribution channels."@en ;
    skos:inScheme : ;
    skos:prefLabel "has film distributor"@en .

rdam:P30069 a skos:Concept ;
    reg:name "bookDesigner"@en ;
    reg:status <http://metadataregistry.org/uri/RegStatus/1001> ;
    rdfs:domain rdac:C10007 ;
    rdfs:isDefinedBy rdam: ;
    rdfs:range rdac:C10002 ;
    rdfs:subPropertyOf rdam:P30082,
        rdau:P60409 ;
    owl:inverseOf rdaa:P50170 ;
    owl:sameAs rdam:bookDesigner ;
    skos:definition "Relates a manifestation to a person, family, or corporate body involved in manufacturing a manifestation by being responsible for the entire graphic design of a book, including arrangement of type and illustration, choice of materials, and process used."@en ;
    skos:inScheme : ;
    skos:prefLabel "has book designer"@en .

rdam:P30070 a skos:Concept ;
    reg:name "engraver"@en ;
    reg:status <http://metadataregistry.org/uri/RegStatus/1001> ;
    rdfs:domain rdac:C10007 ;
    rdfs:isDefinedBy rdam: ;
    rdfs:range rdac:C10002 ;
    rdfs:subPropertyOf rdam:P30082,
        rdau:P60410 ;
    owl:inverseOf rdaa:P50171 ;
    owl:sameAs rdam:engraver ;
    skos:definition "Relates a manifestation to a person, family, or corporate body involved in manufacturing a manifestation by cutting letters, figures, etc., on a surface such as a wooden or metal plate used for printing."@en ;
    skos:inScheme : ;
    skos:prefLabel "has engraver"@en .

rdam:P30071 a skos:Concept ;
    reg:name "brailleEmbosser"@en ;
    reg:status <http://metadataregistry.org/uri/RegStatus/1001> ;
    rdfs:domain rdac:C10007 ;
    rdfs:isDefinedBy rdam: ;
    rdfs:range rdac:C10002 ;
    rdfs:subPropertyOf rdam:P30082,
        rdau:P60411 ;
    owl:inverseOf rdaa:P50172 ;
    owl:sameAs rdam:brailleEmbosser ;
    skos:definition "Relates a manifestation to a person, family, or corporate body involved in manufacturing a manifestation by embossing braille cells using a stylus, special embossing printer, or other device."@en ;
    skos:inScheme : ;
    skos:prefLabel "has braille embosser"@en .

rdam:P30072 a skos:Concept ;
    reg:name "printmaker"@en ;
    reg:status <http://metadataregistry.org/uri/RegStatus/1001> ;
    rdfs:domain rdac:C10007 ;
    rdfs:isDefinedBy rdam: ;
    rdfs:range rdac:C10002 ;
    rdfs:subPropertyOf rdam:P30082,
        rdau:P60412 ;
    owl:inverseOf rdaa:P50173 ;
    owl:sameAs rdam:printmaker ;
    skos:definition "Relates a manifestation to a person, family, or corporate body involved in manufacturing a manifestation by making a relief, intaglio, or planographic printing surface."@en ;
    skos:inScheme : ;
    skos:prefLabel "has printmaker"@en .

rdam:P30073 a skos:Concept ;
    reg:name "caster"@en ;
    reg:status <http://metadataregistry.org/uri/RegStatus/1001> ;
    rdfs:domain rdac:C10007 ;
    rdfs:isDefinedBy rdam: ;
    rdfs:range rdac:C10002 ;
    rdfs:subPropertyOf rdam:P30082,
        rdau:P60413 ;
    owl:inverseOf rdaa:P50174 ;
    owl:sameAs rdam:caster ;
    skos:definition "Relates a manifestation to a person, family, or corporate body involved in manufacturing a manifestation by pouring a liquid or molten substance into a mold and leaving it to solidify to take the shape of the mold."@en ;
    skos:inScheme : ;
    skos:prefLabel "has caster"@en .

rdam:P30074 a skos:Concept ;
    reg:name "lithographer"@en ;
    reg:status <http://metadataregistry.org/uri/RegStatus/1001> ;
    rdfs:domain rdac:C10007 ;
    rdfs:isDefinedBy rdam: ;
    rdfs:range rdac:C10002 ;
    rdfs:subPropertyOf rdam:P30082,
        rdau:P60414 ;
    owl:inverseOf rdaa:P50175 ;
    owl:sameAs rdam:lithographer ;
    skos:definition "Relates a manifestation to a person, family, or corporate body involved in manufacturing a manifestation by preparing a stone or plate for lithographic printing, including a graphic artist creating a design directly on the surface from which printing will be done."@en ;
    skos:inScheme : ;
    skos:prefLabel "has lithographer"@en .

rdam:P30075 a skos:Concept ;
    reg:name "platemaker"@en ;
    reg:status <http://metadataregistry.org/uri/RegStatus/1001> ;
    rdfs:domain rdac:C10007 ;
    rdfs:isDefinedBy rdam: ;
    rdfs:range rdac:C10002 ;
    rdfs:subPropertyOf rdam:P30082,
        rdau:P60415 ;
    owl:inverseOf rdaa:P50176 ;
    owl:sameAs rdam:platemaker ;
    skos:definition "Relates a manifestation to a person, family, or corporate body involved in manufacturing a manifestation by preparing plates used in the production of printed images and/or text."@en ;
    skos:inScheme : ;
    skos:prefLabel "has platemaker"@en .

rdam:P30076 a skos:Concept ;
    reg:name "etcher"@en ;
    reg:status <http://metadataregistry.org/uri/RegStatus/1001> ;
    rdfs:domain rdac:C10007 ;
    rdfs:isDefinedBy rdam: ;
    rdfs:range rdac:C10002 ;
    rdfs:subPropertyOf rdam:P30082,
        rdau:P60416 ;
    owl:inverseOf rdaa:P50177 ;
    owl:sameAs rdam:etcher ;
    skos:definition "Relates a manifestation to a person, family, or corporate body involved in manufacturing a manifestation by subjecting metal, glass, or some other surface used for printing, to acid or another corrosive substance."@en ;
    skos:inScheme : ;
    skos:prefLabel "has etcher"@en .

rdam:P30077 a skos:Concept ;
    reg:name "collotyper"@en ;
    reg:status <http://metadataregistry.org/uri/RegStatus/1001> ;
    rdfs:domain rdac:C10007 ;
    rdfs:isDefinedBy rdam: ;
    rdfs:range rdac:C10002 ;
    rdfs:subPropertyOf rdam:P30082,
        rdau:P60417 ;
    owl:inverseOf rdaa:P50178 ;
    owl:sameAs rdam:collotyper ;
    skos:definition "Relates a manifestation to a person, family, or corporate body involved in manufacturing a manifestation of photographic prints from film or other colloid that has ink-receptive and ink-repellent surfaces."@en ;
    skos:inScheme : ;
    skos:prefLabel "has collotyper"@en .

rdam:P30078 a skos:Concept ;
    reg:name "printer"@en ;
    reg:status <http://metadataregistry.org/uri/RegStatus/1001> ;
    rdfs:domain rdac:C10007 ;
    rdfs:isDefinedBy rdam: ;
    rdfs:range rdac:C10002 ;
    rdfs:subPropertyOf rdam:P30082,
        rdau:P60418 ;
    owl:inverseOf rdaa:P50179 ;
    owl:sameAs rdam:printer ;
    skos:definition "Relates a manifestation to a person, family, or corporate body involved in manufacturing a manifestation of printed text, notated music, etc., from type or plates, such as a book, newspaper, magazine, broadside, score, etc."@en ;
    skos:inScheme : ;
    skos:prefLabel "has printer"@en .

rdam:P30084 a skos:Concept ;
    reg:hasSubproperty rdam:P30122 ;
    reg:name "appliedMaterial"@en ;
    reg:status <http://metadataregistry.org/uri/RegStatus/1001> ;
    rdfs:domain rdac:C10007 ;
    rdfs:isDefinedBy rdam: ;
    rdfs:subPropertyOf rdau:P60159 ;
    owl:sameAs rdam:appliedMaterial ;
    skos:definition "Relates a manifestation to a physical or chemical substance applied to a base material of a resource."@en ;
    skos:inScheme : ;
    skos:prefLabel "has applied material"@en .

rdam:P30097 a skos:Concept ;
    reg:name "alternativeNumericAndOrAlphabeticDesignationOfFirstIssueOrPartOfSequence"@en ;
    reg:status <http://metadataregistry.org/uri/RegStatus/1001> ;
    rdfs:domain rdac:C10007 ;
    rdfs:isDefinedBy rdam: ;
    rdfs:subPropertyOf rdam:P30165,
        rdau:P60499 ;
    owl:sameAs rdam:alternativeNumericAndOrAlphabeticDesignationOfFirstIssueOrPartOfSequence ;
    skos:definition "Relates a manifestation to a second or subsequent system of numbering presented in numeric and/or alphabetic form on the first issue or part of a sequence of numbering for a serial."@en ;
    skos:inScheme : ;
    skos:prefLabel "has alternative numeric and/or alphabetic designation of first issue or part of sequence"@en .

rdam:P30098 a skos:Concept ;
    reg:name "alternativeNumericAndOrAlphabeticDesignationOfLastIssueOrPartOfSequence"@en ;
    reg:status <http://metadataregistry.org/uri/RegStatus/1001> ;
    rdfs:domain rdac:C10007 ;
    rdfs:isDefinedBy rdam: ;
    rdfs:subPropertyOf rdam:P30165,
        rdau:P60500 ;
    owl:sameAs rdam:alternativeNumericAndOrAlphabeticDesignationOfLastIssueOrPartOfSequence ;
    skos:definition "Relates a manifestation to a second or subsequent system of numbering presented in numeric and/or alphabetic form on the last issue or part of a sequence of numbering for a serial."@en ;
    skos:inScheme : ;
    skos:prefLabel "has alternative numeric and/or alphabetic designation of last issue or part of sequence"@en .

rdam:P30099 a skos:Concept ;
    reg:name "alternativeChronologicalDesignationOfFirstIssueOrPartOfSequence"@en ;
    reg:status <http://metadataregistry.org/uri/RegStatus/1001> ;
    rdfs:domain rdac:C10007 ;
    rdfs:isDefinedBy rdam: ;
    rdfs:subPropertyOf rdam:P30165,
        rdau:P60501 ;
    owl:sameAs rdam:alternativeChronologicalDesignationOfFirstIssueOrPartOfSequence ;
    skos:definition "Relates a manifestation to a second or subsequent system of numbering presented in the form of a date (e.g., a year; year and month; month, day, and year) on the first issue or part of a sequence of numbering for a serial."@en ;
    skos:inScheme : ;
    skos:prefLabel "has alternative chronological designation of first issue or part of sequence"@en .

rdam:P30100 a skos:Concept ;
    reg:name "alternativeChronologicalDesignationOfLastIssueOrPartOfSequence"@en ;
    reg:status <http://metadataregistry.org/uri/RegStatus/1001> ;
    rdfs:domain rdac:C10007 ;
    rdfs:isDefinedBy rdam: ;
    rdfs:subPropertyOf rdam:P30165,
        rdau:P60502 ;
    owl:sameAs rdam:alternativeChronologicalDesignationOfLastIssueOrPartOfSequence ;
    skos:definition "Relates a manifestation to a second or subsequent system of numbering presented in the form of a date (e.g., a year; year and month; month, day, and year) on the last issue or part of a sequence of numbering for a serial."@en ;
    skos:inScheme : ;
    skos:prefLabel "has alternative chronological designation of last issue or part of sequence"@en .

rdam:P30102 a skos:Concept ;
    reg:name "digitalRepresentationOfCartographicContent"@en ;
    reg:status <http://metadataregistry.org/uri/RegStatus/1001> ;
    rdfs:domain rdac:C10007 ;
    rdfs:isDefinedBy rdam: ;
    rdfs:subPropertyOf rdam:P30124,
        rdau:P60323 ;
    owl:sameAs rdam:digitalRepresentationOfCartographicContent ;
    skos:definition "Relates a manifestation to a set of technical details relating to the encoding of geospatial information in a cartographic resource."@en ;
    skos:inScheme : ;
    skos:prefLabel "has digital representation of cartographic content"@en .

rdam:P30104 a skos:Concept ;
    reg:name "videoFormat"@en ;
    reg:status <http://metadataregistry.org/uri/RegStatus/1001> ;
    rdfs:domain rdac:C10007 ;
    rdfs:isDefinedBy rdam: ;
    rdfs:subPropertyOf rdam:P30126,
        rdau:P60326 ;
    owl:sameAs rdam:videoFormat ;
    skos:definition "Relates a manifestation to a standard, etc., used to encode the analog video content of a resource."@en ;
    skos:inScheme : ;
    skos:prefLabel "has video format"@en .

rdam:P30105 a skos:Concept ;
    reg:name "statementOfResponsibilityRelatingToTitleProper"@en ;
    reg:status <http://metadataregistry.org/uri/RegStatus/1001> ;
    rdfs:domain rdac:C10007 ;
    rdfs:isDefinedBy rdam: ;
    rdfs:subPropertyOf rdam:P30117,
        rdau:P60327 ;
    owl:sameAs rdam:statementOfResponsibilityRelatingToTitleProper ;
    skos:definition "Relates a manifestation to a statement associated with the title proper of a resource that relates to the identification and/or function of any persons, families, or corporate bodies responsible for the creation of, or contributing to the realization of, the intellectual or artistic content of the resource."@en ;
    skos:inScheme : ;
    skos:prefLabel "has statement of responsibility relating to title proper"@en .

rdam:P30107 a skos:Concept ;
    reg:name "editionStatement"@en ;
    reg:status <http://metadataregistry.org/uri/RegStatus/1001> ;
    rdfs:domain rdac:C10007 ;
    rdfs:isDefinedBy rdam: ;
    rdfs:subPropertyOf rdau:P60329 ;
    owl:sameAs rdam:editionStatement ;
    skos:definition "Relates a manifestation to a statement identifying the edition to which a resource belongs."@en ;
    skos:inScheme : ;
    skos:prefLabel "has edition statement"@en .

rdam:P30108 a skos:Concept ;
    reg:name "distributionStatement"@en ;
    reg:status <http://metadataregistry.org/uri/RegStatus/1001> ;
    rdfs:domain rdac:C10007 ;
    rdfs:isDefinedBy rdam: ;
    rdfs:subPropertyOf rdau:P60330 ;
    owl:sameAs rdam:distributionStatement ;
    skos:definition "Relates a manifestation to a statement identifying the place or places of distribution, distributor or distributors, and date or dates of distribution of a resource in a published form."@en ;
    skos:inScheme : ;
    skos:prefLabel "has distribution statement"@en .

rdam:P30109 a skos:Concept ;
    reg:name "manufactureStatement"@en ;
    reg:status <http://metadataregistry.org/uri/RegStatus/1001> ;
    rdfs:domain rdac:C10007 ;
    rdfs:isDefinedBy rdam: ;
    rdfs:subPropertyOf rdau:P60331 ;
    owl:sameAs rdam:manufactureStatement ;
    skos:definition "Relates a manifestation to a statement identifying the place or places of manufacture, manufacturer or manufacturers, and date or dates of manufacture of a resource in a published form."@en ;
    skos:inScheme : ;
    skos:prefLabel "has manufacture statement"@en .

rdam:P30110 a skos:Concept ;
    reg:name "productionStatement"@en ;
    reg:status <http://metadataregistry.org/uri/RegStatus/1001> ;
    rdfs:domain rdac:C10007 ;
    rdfs:isDefinedBy rdam: ;
    rdfs:subPropertyOf rdau:P60332 ;
    owl:sameAs rdam:productionStatement ;
    skos:definition "Relates a manifestation to a statement identifying the place or places of production, producer or producers, and date or dates of production of a resource in an unpublished form."@en ;
    skos:inScheme : ;
    skos:prefLabel "has production statement"@en .

rdam:P30111 a skos:Concept ;
    reg:name "publicationStatement"@en ;
    reg:status <http://metadataregistry.org/uri/RegStatus/1001> ;
    rdfs:domain rdac:C10007 ;
    rdfs:isDefinedBy rdam: ;
    rdfs:subPropertyOf rdau:P60333 ;
    owl:sameAs rdam:publicationStatement ;
    skos:definition "Relates a manifestation to a statement identifying the place or places of publication, publisher or publishers, and date or dates of publication of a resource."@en ;
    skos:inScheme : ;
    skos:prefLabel "has publication statement"@en .

rdam:P30116 a skos:Concept ;
    reg:name "parallelStatementOfResponsibilityRelatingToTitleProper"@en ;
    reg:status <http://metadataregistry.org/uri/RegStatus/1001> ;
    rdfs:domain rdac:C10007 ;
    rdfs:isDefinedBy rdam: ;
    rdfs:subPropertyOf rdam:P30117,
        rdau:P60338 ;
    owl:sameAs rdam:parallelStatementOfResponsibilityRelatingToTitleProper ;
    skos:definition "Relates a manifestation to a statement of responsibility relating to title proper in a language and/or script that differs from that recorded in the statement of responsibility relating to title proper element."@en ;
    skos:inScheme : ;
    skos:prefLabel "has parallel statement of responsibility relating to title proper"@en .

rdam:P30122 a skos:Concept ;
    reg:name "emulsionOnMicrofilmAndMicrofiche"@en ;
    reg:status <http://metadataregistry.org/uri/RegStatus/1001> ;
    rdfs:domain rdac:C10007 ;
    rdfs:isDefinedBy rdam: ;
    rdfs:subPropertyOf rdam:P30084,
        rdau:P60344 ;
    owl:sameAs rdam:emulsionOnMicrofilmAndMicrofiche ;
    skos:definition "Relates a manifestation to a suspension of light-sensitive chemicals used as a coating on a microfilm or microfiche (e.g., silver halide)."@en ;
    skos:inScheme : ;
    skos:prefLabel "has emulsion on microfilm and microfiche"@en .

rdam:P30123 a skos:Concept ;
    reg:name "broadcastStandard"@en ;
    reg:status <http://metadataregistry.org/uri/RegStatus/1001> ;
    rdfs:domain rdac:C10007 ;
    rdfs:isDefinedBy rdam: ;
    rdfs:subPropertyOf rdam:P30126,
        rdau:P60349 ;
    owl:sameAs rdam:broadcastStandard ;
    skos:definition "Relates a manifestation to a system used to format a video resource for television broadcast."@en ;
    skos:inScheme : ;
    skos:prefLabel "has broadcast standard"@en .

rdam:P30129 a skos:Concept ;
    reg:name "laterTitleProper"@en ;
    reg:status <http://metadataregistry.org/uri/RegStatus/1001> ;
    rdfs:domain rdac:C10007 ;
    rdfs:isDefinedBy rdam: ;
    rdfs:subPropertyOf rdam:P30134,
        rdau:P60357 ;
    owl:sameAs rdam:laterTitleProper ;
    skos:definition "Relates a manifestation to a title proper appearing on a later issue or part of a multipart monograph or serial that differs from that on the first or earliest issue or part."@en ;
    skos:inScheme : ;
    skos:prefLabel "has later title proper"@en .

rdam:P30130 a skos:Concept ;
    reg:name "earlierTitleProper"@en ;
    reg:status <http://metadataregistry.org/uri/RegStatus/1001> ;
    rdfs:domain rdac:C10007 ;
    rdfs:isDefinedBy rdam: ;
    rdfs:subPropertyOf rdam:P30134,
        rdau:P60358 ;
    owl:sameAs rdam:earlierTitleProper ;
    skos:definition "Relates a manifestation to a title proper appearing on an earlier iteration of an integrating resource that differs from that on the current iteration."@en ;
    skos:inScheme : ;
    skos:prefLabel "has earlier title proper"@en .

rdam:P30131 a skos:Concept ;
    reg:name "abbreviatedTitle"@en ;
    reg:status <http://metadataregistry.org/uri/RegStatus/1001> ;
    rdfs:domain rdac:C10007 ;
    rdfs:isDefinedBy rdam: ;
    rdfs:subPropertyOf rdam:P30134,
        rdau:P60359 ;
    owl:sameAs rdam:abbreviatedTitle ;
    skos:definition "Relates a manifestation to a title that has been abbreviated for purposes of indexing or identification."@en ;
    skos:inScheme : ;
    skos:prefLabel "has abbreviated title"@en .

rdam:P30138 a skos:Concept ;
    reg:name "specialPlaybackCharacteristic"@en ;
    reg:status <http://metadataregistry.org/uri/RegStatus/1001> ;
    rdfs:domain rdac:C10007 ;
    rdfs:isDefinedBy rdam: ;
    rdfs:subPropertyOf rdam:P30125,
        rdau:P60481 ;
    owl:sameAs rdam:specialPlaybackCharacteristic ;
    skos:definition "Relates a manifestation to an equalization system, noise reduction system, etc., used in making an audio recording."@en ;
    skos:inScheme : ;
    skos:prefLabel "has special playback characteristic"@en .

rdam:P30145 a skos:Concept ;
    reg:name "restrictionsOnAccess"@en ;
    reg:status <http://metadataregistry.org/uri/RegStatus/1001> ;
    rdfs:domain rdac:C10007 ;
    rdfs:isDefinedBy rdam: ;
    rdfs:subPropertyOf rdau:P60496 ;
    owl:sameAs rdam:restrictionsOnAccess ;
    skos:definition "Relates a manifestation to limitations placed on access to a resource."@en ;
    skos:inScheme : ;
    skos:prefLabel "has restrictions on access"@en .

rdam:P30146 a skos:Concept ;
    reg:name "restrictionsOnUse"@en ;
    reg:status <http://metadataregistry.org/uri/RegStatus/1001> ;
    rdfs:domain rdac:C10007 ;
    rdfs:isDefinedBy rdam: ;
    rdfs:subPropertyOf rdau:P60497 ;
    owl:sameAs rdam:restrictionsOnUse ;
    skos:definition "Relates a manifestation to limitations placed on uses such as reproduction, publication, exhibition, etc."@en ;
    skos:inScheme : ;
    skos:prefLabel "has restrictions on use"@en .

rdam:P30147 a skos:Concept ;
    reg:name "numericAndOrAlphabeticDesignationOfFirstIssueOrPartOfSequence"@en ;
    reg:status <http://metadataregistry.org/uri/RegStatus/1001> ;
    rdfs:domain rdac:C10007 ;
    rdfs:isDefinedBy rdam: ;
    rdfs:subPropertyOf rdam:P30165,
        rdau:P60499 ;
    owl:sameAs rdam:numericAndOrAlphabeticDesignationOfFirstIssueOrPartOfSequence ;
    skos:definition "Relates a manifestation to numbering presented in numeric and/or alphabetic form on the first issue or part of a sequence of numbering for a serial."@en ;
    skos:inScheme : ;
    skos:prefLabel "has numeric and/or alphabetic designation of first issue or part of sequence"@en .

rdam:P30148 a skos:Concept ;
    reg:name "numericAndOrAlphabeticDesignationOfLastIssueOrPartOfSequence"@en ;
    reg:status <http://metadataregistry.org/uri/RegStatus/1001> ;
    rdfs:domain rdac:C10007 ;
    rdfs:isDefinedBy rdam: ;
    rdfs:subPropertyOf rdam:P30165,
        rdau:P60500 ;
    owl:sameAs rdam:numericAndOrAlphabeticDesignationOfLastIssueOrPartOfSequence ;
    skos:definition "Relates a manifestation to numbering presented in numeric and/or alphabetic form on the last issue or part of a sequence of numbering for a serial."@en ;
    skos:inScheme : ;
    skos:prefLabel "has numeric and/or alphabetic designation of last issue or part of sequence"@en .

rdam:P30149 a skos:Concept ;
    reg:name "chronologicalDesignationOfFirstIssueOrPartOfSequence"@en ;
    reg:status <http://metadataregistry.org/uri/RegStatus/1001> ;
    rdfs:domain rdac:C10007 ;
    rdfs:isDefinedBy rdam: ;
    rdfs:subPropertyOf rdam:P30165,
        rdau:P60501 ;
    owl:sameAs rdam:chronologicalDesignationOfFirstIssueOrPartOfSequence ;
    skos:definition "Relates a manifestation to numbering presented in the form of a date (e.g., a year; year and month; month, day, and year) on the first issue or part of a sequence of numbering for a serial."@en ;
    skos:inScheme : ;
    skos:prefLabel "has chronological designation of first issue or part of sequence"@en .

rdam:P30150 a skos:Concept ;
    reg:name "chronologicalDesignationOfLastIssueOrPartOfSequence"@en ;
    reg:status <http://metadataregistry.org/uri/RegStatus/1001> ;
    rdfs:domain rdac:C10007 ;
    rdfs:isDefinedBy rdam: ;
    rdfs:subPropertyOf rdam:P30165,
        rdau:P60502 ;
    owl:sameAs rdam:chronologicalDesignationOfLastIssueOrPartOfSequence ;
    skos:definition "Relates a manifestation to numbering presented in the form of a date (e.g., a year; year and month; month, day, and year) on the last issue or part of a sequence of numbering for a serial."@en ;
    skos:inScheme : ;
    skos:prefLabel "has chronological designation of last issue or part of sequence"@en .

rdam:P30151 a skos:Concept ;
    reg:name "parallelOtherTitleInformation"@en ;
    reg:status <http://metadataregistry.org/uri/RegStatus/1001> ;
    rdfs:domain rdac:C10007 ;
    rdfs:isDefinedBy rdam: ;
    rdfs:subPropertyOf rdam:P30134,
        rdau:P60507 ;
    owl:sameAs rdam:parallelOtherTitleInformation ;
    skos:definition "Relates a manifestation to other title information in a language and/or script that differs from that recorded in the other title information element."@en ;
    skos:inScheme : ;
    skos:prefLabel "has parallel other title information"@en .

rdam:P30159 a skos:Concept ;
    reg:name "resolution"@en ;
    reg:status <http://metadataregistry.org/uri/RegStatus/1001> ;
    rdfs:domain rdac:C10007 ;
    rdfs:isDefinedBy rdam: ;
    rdfs:subPropertyOf rdam:P30124,
        rdau:P60519 ;
    owl:sameAs rdam:resolution ;
    skos:definition "Relates a manifestation to the clarity or fineness of detail in a digital image, expressed by the measurement of the image in pixels, etc."@en ;
    skos:inScheme : ;
    skos:prefLabel "has resolution"@en .

rdam:P30161 a skos:Concept ;
    reg:name "trackConfiguration"@en ;
    reg:status <http://metadataregistry.org/uri/RegStatus/1001> ;
    rdfs:domain rdac:C10007 ;
    rdfs:isDefinedBy rdam: ;
    rdfs:subPropertyOf rdam:P30125,
        rdau:P60522 ;
    owl:sameAs rdam:trackConfiguration ;
    skos:definition "Relates a manifestation to the configuration of the audio track on a sound-track film (e.g., centre track)."@en ;
    skos:inScheme : ;
    skos:prefLabel "has track configuration"@en .

rdam:P30162 a skos:Concept ;
    reg:name "equipmentOrSystemRequirement"@en ;
    reg:status <http://metadataregistry.org/uri/RegStatus/1001> ;
    rdfs:domain rdac:C10007 ;
    rdfs:isDefinedBy rdam: ;
    rdfs:subPropertyOf rdau:P60528 ;
    owl:sameAs rdam:equipmentOrSystemRequirement ;
    skos:definition "Relates a manifestation to the equipment or system required for use, playback, etc., of an analog, digital, etc., resource."@en ;
    skos:inScheme : ;
    skos:prefLabel "has equipment or system requirement"@en .

rdam:P30163 a skos:Concept ;
    reg:name "presentationFormat"@en ;
    reg:status <http://metadataregistry.org/uri/RegStatus/1001> ;
    rdfs:domain rdac:C10007 ;
    rdfs:isDefinedBy rdam: ;
    rdfs:subPropertyOf rdam:P30127,
        rdau:P60529 ;
    owl:sameAs rdam:presentationFormat ;
    skos:definition "Relates a manifestation to the format used in the production of a projected image (e.g., cinerama, imax)."@en ;
    skos:inScheme : ;
    skos:prefLabel "has presentation format"@en .

rdam:P30164 a skos:Concept ;
    reg:name "grooveCharacteristic"@en ;
    reg:status <http://metadataregistry.org/uri/RegStatus/1001> ;
    rdfs:domain rdac:C10007 ;
    rdfs:isDefinedBy rdam: ;
    rdfs:subPropertyOf rdam:P30125,
        rdau:P60532 ;
    owl:sameAs rdam:grooveCharacteristic ;
    skos:definition "Relates a manifestation to the groove width of an analog disc or the groove pitch of an analog cylinder."@en ;
    skos:inScheme : ;
    skos:prefLabel "has groove characteristic"@en .

rdam:P30170 a skos:Concept ;
    reg:name "dimensionsOfMapEtc"@en ;
    reg:status <http://metadataregistry.org/uri/RegStatus/1001> ;
    rdfs:domain rdac:C10007 ;
    rdfs:isDefinedBy rdam: ;
    rdfs:subPropertyOf rdam:P30169,
        rdau:P60540 ;
    owl:sameAs rdam:dimensionsOfMapEtc ;
    skos:definition "Relates a manifestation to the measurements of the face of a map, etc."@en ;
    skos:inScheme : ;
    skos:prefLabel "has dimensions of map, etc."@en .

rdam:P30171 a skos:Concept ;
    reg:name "dimensionsOfStillImage"@en ;
    reg:status <http://metadataregistry.org/uri/RegStatus/1001> ;
    rdfs:domain rdac:C10007 ;
    rdfs:isDefinedBy rdam: ;
    rdfs:subPropertyOf rdam:P30169,
        rdau:P60541 ;
    owl:sameAs rdam:dimensionsOfStillImage ;
    skos:definition "Relates a manifestation to the measurements of the pictorial area of a still image."@en ;
    skos:inScheme : ;
    skos:prefLabel "has dimensions of still image"@en .

rdam:P30172 a skos:Concept ;
    reg:name "typeOfRecording"@en ;
    reg:status <http://metadataregistry.org/uri/RegStatus/1001> ;
    rdfs:domain rdac:C10007 ;
    rdfs:isDefinedBy rdam: ;
    rdfs:subPropertyOf rdam:P30125,
        rdau:P60543 ;
    owl:sameAs rdam:typeOfRecording ;
    skos:definition "Relates a manifestation to the method used to encode audio content for playback (e.g., analog or digital)."@en ;
    skos:inScheme : ;
    skos:prefLabel "has type of recording"@en .

rdam:P30173 a skos:Concept ;
    reg:name "distributorsName"@en ;
    reg:status <http://metadataregistry.org/uri/RegStatus/1001> ;
    rdfs:domain rdac:C10007 ;
    rdfs:isDefinedBy rdam: ;
    rdfs:subPropertyOf rdau:P60544 ;
    owl:sameAs rdam:distributorsName ;
    skos:definition "Relates a manifestation to the name of a person, family, or corporate body responsible for distributing a resource in a published form."@en ;
    skos:inScheme : ;
    skos:prefLabel "has distributor's name"@en .

rdam:P30174 a skos:Concept ;
    reg:name "producersName"@en ;
    reg:status <http://metadataregistry.org/uri/RegStatus/1001> ;
    rdfs:domain rdac:C10007 ;
    rdfs:isDefinedBy rdam: ;
    rdfs:subPropertyOf rdau:P60545 ;
    owl:sameAs rdam:producersName ;
    skos:definition "Relates a manifestation to the name of a person, family, or corporate body responsible for inscribing, fabricating, constructing, etc., a resource in an unpublished form."@en ;
    skos:inScheme : ;
    skos:prefLabel "has producer's name"@en .

rdam:P30175 a skos:Concept ;
    reg:name "manufacturersName"@en ;
    reg:status <http://metadataregistry.org/uri/RegStatus/1001> ;
    rdfs:domain rdac:C10007 ;
    rdfs:isDefinedBy rdam: ;
    rdfs:subPropertyOf rdau:P60546 ;
    owl:sameAs rdam:manufacturersName ;
    skos:definition "Relates a manifestation to the name of a person, family, or corporate body responsible for printing, duplicating, casting, etc., a resource in a published form."@en ;
    skos:inScheme : ;
    skos:prefLabel "has manufacturer's name"@en .

rdam:P30176 a skos:Concept ;
    reg:name "publishersName"@en ;
    reg:status <http://metadataregistry.org/uri/RegStatus/1001> ;
    rdfs:domain rdac:C10007 ;
    rdfs:isDefinedBy rdam: ;
    rdfs:subPropertyOf rdau:P60547 ;
    owl:sameAs rdam:publishersName ;
    skos:definition "Relates a manifestation to the name of a person, family, or corporate body responsible for publishing, releasing, or issuing a resource."@en ;
    skos:inScheme : ;
    skos:prefLabel "has publisher's name"@en .

rdam:P30177 a skos:Concept ;
    reg:name "extentOfCartographicResource"@en ;
    reg:status <http://metadataregistry.org/uri/RegStatus/1001> ;
    rdfs:domain rdac:C10007 ;
    rdfs:isDefinedBy rdam: ;
    rdfs:subPropertyOf rdam:P30182,
        rdau:P60550 ;
    owl:sameAs rdam:extentOfCartographicResource ;
    skos:definition "Relates a manifestation to the number and type of units and/or subunits making up a cartographic resource."@en ;
    skos:inScheme : ;
    skos:prefLabel "has extent of cartographic resource"@en .

rdam:P30178 a skos:Concept ;
    reg:name "extentOfNotatedMusic"@en ;
    reg:status <http://metadataregistry.org/uri/RegStatus/1001> ;
    rdfs:domain rdac:C10007 ;
    rdfs:isDefinedBy rdam: ;
    rdfs:subPropertyOf rdam:P30182,
        rdau:P60550 ;
    owl:sameAs rdam:extentOfNotatedMusic ;
    skos:definition "Relates a manifestation to the number and type of units and/or subunits making up a resource consisting of notated music, with or without accompanying text and/or illustrations."@en ;
    skos:inScheme : ;
    skos:prefLabel "has extent of notated music"@en .

rdam:P30179 a skos:Concept ;
    reg:name "extentOfStillImage"@en ;
    reg:status <http://metadataregistry.org/uri/RegStatus/1001> ;
    rdfs:domain rdac:C10007 ;
    rdfs:isDefinedBy rdam: ;
    rdfs:subPropertyOf rdam:P30182,
        rdau:P60550 ;
    owl:sameAs rdam:extentOfStillImage ;
    skos:definition "Relates a manifestation to the number and type of units and/or subunits making up a resource consisting of one or more still images."@en ;
    skos:inScheme : ;
    skos:prefLabel "has extent of still image"@en .

rdam:P30180 a skos:Concept ;
    reg:name "extentOfThreeDimensionalForm"@en ;
    reg:status <http://metadataregistry.org/uri/RegStatus/1001> ;
    rdfs:domain rdac:C10007 ;
    rdfs:isDefinedBy rdam: ;
    rdfs:subPropertyOf rdam:P30182,
        rdau:P60550 ;
    owl:sameAs rdam:extentOfThreeDimensionalForm ;
    skos:definition "Relates a manifestation to the number and type of units and/or subunits making up a resource consisting of one or more three-dimensional forms."@en ;
    skos:inScheme : ;
    skos:prefLabel "has extent of three-dimensional form"@en .

rdam:P30181 a skos:Concept ;
    reg:name "extentOfText"@en ;
    reg:status <http://metadataregistry.org/uri/RegStatus/1001> ;
    rdfs:domain rdac:C10007 ;
    rdfs:isDefinedBy rdam: ;
    rdfs:subPropertyOf rdam:P30182,
        rdau:P60550 ;
    owl:sameAs rdam:extentOfText ;
    skos:definition "Relates a manifestation to the number and type of units and/or subunits making up a resource consisting of text, with or without accompanying illustrations."@en ;
    skos:inScheme : ;
    skos:prefLabel "has extent of text"@en .

rdam:P30183 a skos:Concept ;
    reg:name "fileSize"@en ;
    reg:status <http://metadataregistry.org/uri/RegStatus/1001> ;
    rdfs:domain rdac:C10007 ;
    rdfs:isDefinedBy rdam: ;
    rdfs:subPropertyOf rdam:P30124,
        rdau:P60551 ;
    owl:sameAs rdam:fileSize ;
    skos:definition "Relates a manifestation to the number of bytes in a digital file."@en ;
    skos:inScheme : ;
    skos:prefLabel "has file size"@en .

rdam:P30184 a skos:Concept ;
    reg:name "configurationOfPlaybackChannels"@en ;
    reg:status <http://metadataregistry.org/uri/RegStatus/1001> ;
    rdfs:domain rdac:C10007 ;
    rdfs:isDefinedBy rdam: ;
    rdfs:subPropertyOf rdam:P30125,
        rdau:P60552 ;
    owl:sameAs rdam:configurationOfPlaybackChannels ;
    skos:definition "Relates a manifestation to the number of sound channels used to make a recording (e.g., one channel for a monophonic recording, two channels for a stereophonic recording)."@en ;
    skos:inScheme : ;
    skos:prefLabel "has configuration of playback channels"@en .

rdam:P30185 a skos:Concept ;
    reg:name "tapeConfiguration"@en ;
    reg:status <http://metadataregistry.org/uri/RegStatus/1001> ;
    rdfs:domain rdac:C10007 ;
    rdfs:isDefinedBy rdam: ;
    rdfs:subPropertyOf rdam:P30125,
        rdau:P60553 ;
    owl:sameAs rdam:tapeConfiguration ;
    skos:definition "Relates a manifestation to the number of tracks on an audiotape."@en ;
    skos:inScheme : ;
    skos:prefLabel "has tape configuration"@en .

rdam:P30188 a skos:Concept ;
    reg:name "productionMethodForTactileResource"@en ;
    reg:status <http://metadataregistry.org/uri/RegStatus/1001> ;
    rdfs:domain rdac:C10007 ;
    rdfs:isDefinedBy rdam: ;
    rdfs:subPropertyOf rdam:P30187,
        rdau:P60561 ;
    owl:sameAs rdam:productionMethodForTactileResource ;
    skos:definition "Relates a manifestation to the process used to produce a tactile resource (e.g., embossing, thermoform)."@en ;
    skos:inScheme : ;
    skos:prefLabel "has production method for tactile resource"@en .

rdam:P30189 a skos:Concept ;
    reg:name "productionMethodForManuscript"@en ;
    reg:status <http://metadataregistry.org/uri/RegStatus/1001> ;
    rdfs:domain rdac:C10007 ;
    rdfs:isDefinedBy rdam: ;
    rdfs:subPropertyOf rdam:P30187 ;
    owl:sameAs rdam:productionMethodForManuscript ;
    skos:definition "Relates a manifestation to the process used to produce an original manuscript or a copy."@en ;
    skos:inScheme : ;
    skos:prefLabel "has production method for manuscript"@en .

rdam:P30190 a skos:Concept ;
    reg:name "generationOfAudioRecording"@en ;
    reg:status <http://metadataregistry.org/uri/RegStatus/1001> ;
    rdfs:domain rdac:C10007 ;
    rdfs:isDefinedBy rdam: ;
    rdfs:subPropertyOf rdam:P30191,
        rdau:P60567 ;
    owl:sameAs rdam:generationOfAudioRecording ;
    skos:definition "Relates a manifestation to the relationship between an original audio carrier and the carrier of a reproduction made from the original (e.g., a tape duplication master, a test pressing)."@en ;
    skos:inScheme : ;
    skos:prefLabel "has generation of audio recording"@en .

rdam:P30192 a skos:Concept ;
    reg:name "generationOfDigitalResource"@en ;
    reg:status <http://metadataregistry.org/uri/RegStatus/1001> ;
    rdfs:domain rdac:C10007 ;
    rdfs:isDefinedBy rdam: ;
    rdfs:subPropertyOf rdam:P30191,
        rdau:P60569 ;
    owl:sameAs rdam:generationOfDigitalResource ;
    skos:definition "Relates a manifestation to the relationship between an original carrier of a digital resource and the carrier of a reproduction made from the original (e.g., a derivative master)."@en ;
    skos:inScheme : ;
    skos:prefLabel "has generation of digital resource"@en .

rdam:P30193 a skos:Concept ;
    reg:name "generationOfMotionPictureFilm"@en ;
    reg:status <http://metadataregistry.org/uri/RegStatus/1001> ;
    rdfs:domain rdac:C10007 ;
    rdfs:isDefinedBy rdam: ;
    rdfs:subPropertyOf rdam:P30191,
        rdau:P60570 ;
    owl:sameAs rdam:generationOfMotionPictureFilm ;
    skos:definition "Relates a manifestation to the relationship between an original carrier of a motion picture film resource and the carrier of a reproduction made from the original (e.g., a reference print)."@en ;
    skos:inScheme : ;
    skos:prefLabel "has generation of motion picture film"@en .

rdam:P30194 a skos:Concept ;
    reg:name "generationOfVideotape"@en ;
    reg:status <http://metadataregistry.org/uri/RegStatus/1001> ;
    rdfs:domain rdac:C10007 ;
    rdfs:isDefinedBy rdam: ;
    rdfs:subPropertyOf rdam:P30191,
        rdau:P60571 ;
    owl:sameAs rdam:generationOfVideotape ;
    skos:definition "Relates a manifestation to the relationship between an original carrier of a videotape resource and the carrier of a reproduction made from the original (e.g., a show copy)."@en ;
    skos:inScheme : ;
    skos:prefLabel "has generation of videotape"@en .

rdam:P30195 a skos:Concept ;
    reg:name "generationOfMicroform"@en ;
    reg:status <http://metadataregistry.org/uri/RegStatus/1001> ;
    rdfs:domain rdac:C10007 ;
    rdfs:isDefinedBy rdam: ;
    rdfs:subPropertyOf rdam:P30191,
        rdau:P60572 ;
    owl:sameAs rdam:generationOfMicroform ;
    skos:definition "Relates a manifestation to the relationship between an original microform carrier and the carrier of a reproduction made from the original (e.g., a printing master)."@en ;
    skos:inScheme : ;
    skos:prefLabel "has generation of microform"@en .

rdam:P30199 a skos:Concept ;
    reg:name "fontSize"@en ;
    reg:status <http://metadataregistry.org/uri/RegStatus/1001> ;
    rdfs:domain rdac:C10007 ;
    rdfs:isDefinedBy rdam: ;
    rdfs:subPropertyOf rdau:P60582 ;
    owl:sameAs rdam:fontSize ;
    skos:definition "Relates a manifestation to the size of the type used to represent the characters and symbols in a resource."@en ;
    skos:inScheme : ;
    skos:prefLabel "has font size"@en .

rdam:P30200 a skos:Concept ;
    reg:name "projectionSpeed"@en ;
    reg:status <http://metadataregistry.org/uri/RegStatus/1001> ;
    rdfs:domain rdac:C10007 ;
    rdfs:isDefinedBy rdam: ;
    rdfs:subPropertyOf rdam:P30127,
        rdau:P60585 ;
    owl:sameAs rdam:projectionSpeed ;
    skos:definition "Relates a manifestation to the speed at which a projected carrier must be operated to produce the moving image intended."@en ;
    skos:inScheme : ;
    skos:prefLabel "has projection speed"@en .

rdam:P30201 a skos:Concept ;
    reg:name "playingSpeed"@en ;
    reg:status <http://metadataregistry.org/uri/RegStatus/1001> ;
    rdfs:domain rdac:C10007 ;
    rdfs:isDefinedBy rdam: ;
    rdfs:subPropertyOf rdam:P30125,
        rdau:P60586 ;
    owl:sameAs rdam:playingSpeed ;
    skos:definition "Relates a manifestation to the speed at which an audio carrier must be operated to produce the sound intended."@en ;
    skos:inScheme : ;
    skos:prefLabel "has playing speed"@en .

rdam:P30202 a skos:Concept ;
    reg:name "encodedBitrate"@en ;
    reg:status <http://metadataregistry.org/uri/RegStatus/1001> ;
    rdfs:domain rdac:C10007 ;
    rdfs:isDefinedBy rdam: ;
    rdfs:subPropertyOf rdam:P30124,
        rdau:P60587 ;
    owl:sameAs rdam:encodedBitrate ;
    skos:definition "Relates a manifestation to the speed at which streaming audio, video, etc., is designed to play."@en ;
    skos:inScheme : ;
    skos:prefLabel "has encoded bitrate"@en .

rdam:P30206 a skos:Concept ;
    reg:name "recordingMedium"@en ;
    reg:status <http://metadataregistry.org/uri/RegStatus/1001> ;
    rdfs:domain rdac:C10007 ;
    rdfs:isDefinedBy rdam: ;
    rdfs:subPropertyOf rdam:P30125,
        rdau:P60594 ;
    owl:sameAs rdam:recordingMedium ;
    skos:definition "Relates a manifestation to the type of medium used to record sound on an audio carrier (e.g., magnetic, optical)."@en ;
    skos:inScheme : ;
    skos:prefLabel "has recording medium"@en .

rdam:P30207 a skos:Concept ;
    reg:name "baseMaterialForMicrofilmMicrofichePhotographicFilmAndMotionPictureFilm"@en ;
    reg:status <http://metadataregistry.org/uri/RegStatus/1001> ;
    rdfs:domain rdac:C10007 ;
    rdfs:isDefinedBy rdam: ;
    rdfs:subPropertyOf rdam:P30208,
        rdau:P60595 ;
    owl:sameAs rdam:baseMaterialForMicrofilmMicrofichePhotographicFilmAndMotionPictureFilm ;
    skos:definition "Relates a manifestation to the underlying physical material of a microfilm, microfiche, photographic film, or motion picture film resource."@en ;
    skos:inScheme : ;
    skos:prefLabel "has base material for microfilm, microfiche, photographic film, and motion picture film"@en .

rdam:P30208 a skos:Concept ;
    reg:hasSubproperty rdam:P30207 ;
    reg:name "baseMaterial"@en ;
    reg:status <http://metadataregistry.org/uri/RegStatus/1001> ;
    rdfs:domain rdac:C10007 ;
    rdfs:isDefinedBy rdam: ;
    rdfs:subPropertyOf rdau:P60596 ;
    owl:sameAs rdam:baseMaterial ;
    skos:definition "Relates a manifestation to the underlying physical material of a resource."@en ;
    skos:inScheme : ;
    skos:prefLabel "has base material"@en .

rdam:P30210 a skos:Concept ;
    reg:hasSubproperty rdam:P30027 ;
    reg:name "accompanyingManifestationRelationship"@en ;
    reg:status <http://metadataregistry.org/uri/RegStatus/1001> ;
    rdfs:domain rdac:C10007 ;
    rdfs:isDefinedBy rdam: ;
    rdfs:range rdac:C10007 ;
    rdfs:subPropertyOf rdau:P60709 ;
    owl:sameAs rdam:accompanyingManifestationRelationship ;
    skos:definition "Relates a manifestation to a manifestation that accompanies or is accompanied by the manifestation."@en ;
    skos:inScheme : ;
    skos:prefLabel "has accompanying manifestation relationship with"@en .

rdam:P30214 a skos:Concept ;
    reg:name "noteOnCarrier"@en ;
    reg:status <http://metadataregistry.org/uri/RegStatus/1001> ;
    rdfs:domain rdac:C10007 ;
    rdfs:isDefinedBy rdam: ;
    rdfs:subPropertyOf rdau:P60470 ;
    owl:sameAs rdam:noteOnCarrier ;
    skos:inScheme : ;
    skos:prefLabel "has note on carrier"@en .

rdau:P60050 :vakioidutTermit <http://rdvocab.info/termList/RDAMediaType/1001> .

<http://rdvocab.info/termList/RDACarrierType/1008> skos:prefLabel "äänikela"@fi .

<http://rdvocab.info/termList/RDACarrierType/1011> skos:prefLabel "muistikortti"@fi .

<http://rdvocab.info/termList/RDACarrierType/1022> skos:prefLabel "mikrokortti"@fi .

<http://rdvocab.info/termList/RDACarrierType/1027> skos:prefLabel "mikrofilmiliuska"@fi .

<http://rdvocab.info/termList/RDACarrierType/1040> skos:prefLabel "dia"@fi .

<http://rdvocab.info/termList/RDACarrierType/1052> skos:prefLabel "videokasetti"@fi .

<http://rdvocab.info/termList/RDACarrierType/1056> skos:prefLabel "mikrofilmirulla"@fi .

<http://rdvocab.info/termList/RDAMediaType/1001> skos:prefLabel "audio"@fi ;
    skos:scopeNote "Viestin sisältää tallennettua ääntä, ja se on suunniteltu käytettäväksi soittolaitteella kuten levysoittimella, kasettisoittimella, CD-soittimella, MP3-soittimella. Käsittää sekä digitaalisesti koodattua että analogisesti tallennettua ääntä sisältävät viestimet."@fi .

<http://rdvocab.info/termList/fontSize/1001> skos:prefLabel "erittäin suuri teksti"@fi ;
    skos:scopeNote "Näkövammaisille tarkoitettu kirjasinkoko."@fi .

<http://rdvocab.info/termList/fontSize/1002> skos:prefLabel "isotekstinen"@fi .

<http://metatietosanasto.fi/019> a skos:Concept ;
    skos:broader <http://metatietosanasto.fi/018> ;
    skos:inScheme : ;
    skos:prefLabel "DAISY-lukulaite"@fi .

<http://metatietosanasto.fi/020> a skos:Concept ;
    skos:broader <http://metatietosanasto.fi/018> ;
    skos:inScheme : ;
    skos:prefLabel "e-kirjan lukulaite"@fi .

<http://metatietosanasto.fi/021> a skos:Concept ;
    skos:broader <http://metatietosanasto.fi/018> ;
    skos:inScheme : ;
    skos:prefLabel "mikrofilmin lukulaite"@fi .

<http://metatietosanasto.fi/030> a skos:Concept ;
    skos:broader <http://metatietosanasto.fi/029> ;
    skos:inScheme : ;
    skos:prefLabel "alanimeke"@fi .

<http://metatietosanasto.fi/031> a skos:Concept ;
    skos:broader <http://metatietosanasto.fi/029> ;
    skos:inScheme : ;
    skos:prefLabel "ylänimeke"@fi .

<http://metatietosanasto.fi/071> a skos:Concept ;
    skos:broader <http://rdvocab.info/termList/RDACarrierType/1045> ;
    skos:inScheme : ;
    skos:prefLabel "kuvakortti"@fi .

<http://metatietosanasto.fi/072> a skos:Concept ;
    skos:broader <http://rdvocab.info/termList/RDACarrierType/1045> ;
    skos:inScheme : ;
    skos:prefLabel "kysymyskortti"@fi .

<http://metatietosanasto.fi/073> a skos:Concept ;
    skos:broader <http://rdvocab.info/termList/RDACarrierType/1045> ;
    skos:inScheme : ;
    skos:prefLabel "postikortti"@fi .

<http://metatietosanasto.fi/074> a skos:Concept ;
    skos:broader <http://rdvocab.info/termList/RDACarrierType/1045> ;
    skos:inScheme : ;
    skos:prefLabel "toimintakortti"@fi ;
    skos:scopeNote "Kortti, johon on painettu sanoja, numeroita, tai/ja kuvia, ja jota käytetään tietyn toiminnan toteuttamisessa (engl. activity card)"@fi .

<http://metatietosanasto.fi/080> a skos:Concept ;
    skos:broader <http://rdvocab.info/termList/RDACarrierType/1013> ;
    skos:inScheme : ;
    skos:prefLabel "Blu-ray-levy"@fi ;
    skos:scopeNote "Korkeatarkkuuksinen optinen levy. Blu-ray on Philipsin ja Sonyn UDO- (Ultra Density Optical) ja Pioneerin DVDR Blue -tutkimusprojektien yhteistyössä syntynyt levyformaatti(Wikipedia, 27.9.2011)"@fi .

<http://metatietosanasto.fi/082> a skos:Concept ;
    skos:broader <http://metatietosanasto.fi/081> ;
    skos:inScheme : ;
    skos:prefLabel "CD-ROM-levy"@fi .

<http://metatietosanasto.fi/084> a skos:Concept ;
    skos:broader <http://metatietosanasto.fi/083> ;
    skos:inScheme : ;
    skos:prefLabel "DVD-ROM-levy"@fi .

<http://metatietosanasto.fi/085> a skos:Concept ;
    skos:broader <http://rdvocab.info/termList/RDACarrierType/1013> ;
    skos:inScheme : ;
    skos:prefLabel "CD-DVD-levy"@fi .

<http://metatietosanasto.fi/086> a skos:Concept ;
    skos:broader <http://rdvocab.info/termList/RDACarrierType/1060> ;
    skos:inScheme : ;
    skos:prefLabel "DVD-videolevy"@fi .

<http://metatietosanasto.fi/087> a skos:Concept ;
    skos:broader <http://rdvocab.info/termList/RDACarrierType/1060> ;
    skos:inScheme : ;
    skos:prefLabel "Blue-ray-videolevy"@fi .

<http://metatietosanasto.fi/088> a skos:Concept ;
    skos:broader <http://rdvocab.info/termList/RDACarrierType/1004> ;
    skos:inScheme : ;
    skos:prefLabel "Blue-ray-äänilevy"@fi .

<http://metatietosanasto.fi/089> a skos:Concept ;
    skos:broader <http://rdvocab.info/termList/RDACarrierType/1004> ;
    skos:inScheme : ;
    skos:prefLabel "CD-äänilevy"@fi .

<http://metatietosanasto.fi/090> a skos:Concept ;
    skos:broader <http://rdvocab.info/termList/RDACarrierType/1004> ;
    skos:inScheme : ;
    skos:prefLabel "DVD-äänilevy"@fi ;
    skos:scopeNote "Pääosin audiodataa sisältävä DVD-levy"@fi .

<http://metatietosanasto.fi/091> a skos:Concept ;
    skos:broader <http://rdvocab.info/termList/RDACarrierType/1004> ;
    skos:inScheme : ;
    skos:prefLabel "MD-äänilevy"@fi .

<http://metatietosanasto.fi/092> a skos:Concept ;
    skos:broader <http://rdvocab.info/termList/RDACarrierType/1004> ;
    skos:inScheme : ;
    skos:prefLabel "SACD-äänilevy"@fi .

<http://metatietosanasto.fi/097> a skos:Concept ;
    skos:broader <http://metatietosanasto.fi/096> ;
    skos:inScheme : ;
    skos:prefLabel "lautapeli"@fi .

<http://metatietosanasto.fi/098> a skos:Concept ;
    skos:broader <http://metatietosanasto.fi/096> ;
    skos:inScheme : ;
    skos:prefLabel "palapeli"@fi .

<http://metatietosanasto.fi/102> a skos:Concept ;
    skos:broader <http://rdvocab.info/termList/RDACarrierType/1018> ;
    skos:inScheme : ;
    skos:prefLabel "verkkojulkaisu"@fi .

<http://metatietosanasto.fi/103> a skos:Concept ;
    skos:broader <http://rdvocab.info/termList/RDACarrierType/1007> ;
    skos:inScheme : ;
    skos:prefLabel "C-kasetti"@fi .

<http://metatietosanasto.fi/104> a skos:Concept ;
    skos:broader <http://rdvocab.info/termList/RDACarrierType/1007> ;
    skos:inScheme : ;
    skos:prefLabel "DAT-kasetti"@fi .

<http://metatietosanasto.fi/136> a skos:Concept ;
    skos:broader <http://rdvocab.info/termList/fileType/1001> ;
    skos:inScheme : ;
    skos:prefLabel "CD audio"@fi .

<http://metatietosanasto.fi/137> a skos:Concept ;
    skos:broader <http://rdvocab.info/termList/fileType/1001> ;
    skos:inScheme : ;
    skos:prefLabel "DAISY"@fi .

<http://metatietosanasto.fi/138> a skos:Concept ;
    skos:broader <http://rdvocab.info/termList/fileType/1001> ;
    skos:inScheme : ;
    skos:prefLabel "DVD audio"@fi .

<http://metatietosanasto.fi/139> a skos:Concept ;
    skos:broader <http://rdvocab.info/termList/fileType/1001> ;
    skos:inScheme : ;
    skos:prefLabel "MP3"@fi .

<http://metatietosanasto.fi/140> a skos:Concept ;
    skos:broader <http://rdvocab.info/termList/fileType/1001> ;
    skos:inScheme : ;
    skos:prefLabel "SACD"@fi .

<http://metatietosanasto.fi/141> a skos:Concept ;
    skos:broader <http://rdvocab.info/termList/fileType/1001> ;
    skos:inScheme : ;
    skos:prefLabel "WAV"@fi ;
    skos:scopeNote "Waveform Audio File"@fi .

<http://metatietosanasto.fi/142> a skos:Concept ;
    skos:broader <http://rdvocab.info/termList/fileType/1002> ;
    skos:inScheme : ;
    skos:prefLabel "EPUB"@fi .

<http://metatietosanasto.fi/143> a skos:Concept ;
    skos:broader <http://rdvocab.info/termList/fileType/1002> ;
    skos:inScheme : ;
    skos:prefLabel "HTML"@fi .

<http://metatietosanasto.fi/144> a skos:Concept ;
    skos:broader <http://rdvocab.info/termList/fileType/1002> ;
    skos:inScheme : ;
    skos:prefLabel "MS Word"@fi .

<http://metatietosanasto.fi/145> a skos:Concept ;
    skos:broader <http://rdvocab.info/termList/fileType/1002> ;
    skos:inScheme : ;
    skos:prefLabel "PDF"@fi .

<http://metatietosanasto.fi/146> a skos:Concept ;
    skos:broader <http://rdvocab.info/termList/fileType/1002> ;
    skos:inScheme : ;
    skos:prefLabel "RTF"@fi .

<http://metatietosanasto.fi/147> a skos:Concept ;
    skos:broader <http://rdvocab.info/termList/fileType/1002> ;
    skos:inScheme : ;
    skos:prefLabel "WordPerfect"@fi .

<http://metatietosanasto.fi/148> a skos:Concept ;
    skos:broader <http://rdvocab.info/termList/fileType/1002> ;
    skos:inScheme : ;
    skos:prefLabel "XML"@fi .

<http://metatietosanasto.fi/149> a skos:Concept ;
    skos:broader <http://rdvocab.info/termList/fileType/1006> ;
    skos:inScheme : ;
    skos:prefLabel "Blu-ray"@fi .

<http://metatietosanasto.fi/150> a skos:Concept ;
    skos:broader <http://rdvocab.info/termList/fileType/1006> ;
    skos:inScheme : ;
    skos:prefLabel "DVD video"@fi .

<http://metatietosanasto.fi/151> a skos:Concept ;
    skos:broader <http://rdvocab.info/termList/fileType/1006> ;
    skos:inScheme : ;
    skos:prefLabel "MPEG-4"@fi .

<http://metatietosanasto.fi/152> a skos:Concept ;
    skos:broader <http://rdvocab.info/termList/fileType/1006> ;
    skos:inScheme : ;
    skos:prefLabel "Windows Media"@fi .

<http://metatietosanasto.fi/154> a skos:Concept ;
    skos:broader <http://rdvocab.info/termList/fileType/1006> ;
    skos:inScheme : ;
    skos:prefLabel "GIF"@fi .

<http://metatietosanasto.fi/155> a skos:Concept ;
    skos:broader <http://rdvocab.info/termList/fileType/1006> ;
    skos:inScheme : ;
    skos:prefLabel "JPEG"@fi .

<http://metatietosanasto.fi/156> a skos:Concept ;
    skos:broader <http://rdvocab.info/termList/fileType/1006> ;
    skos:inScheme : ;
    skos:prefLabel "JPEG2000"@fi .

<http://metatietosanasto.fi/157> a skos:Concept ;
    skos:inScheme : ;
    skos:prefLabel "näköispainos"@fi ;
    skos:scopeNote "Julkaisu, jonka pääteksti on tarkasti jäljennetty aikaisemmasta painoksesta (engl. facsimile edition)"@fi .

<http://metatietosanasto.fi/158> a skos:Concept ;
    skos:inScheme : ;
    skos:prefLabel "painos"@fi ;
    skos:scopeNote "Kaikki julkaisun peruskappaleesta painamalla tai muulla menetelmällä tuotetut kappaleet, jotka sama kustantaja, yhteisö tai henkilö on julkaissut. (Kuvailusäännöt) (engl. edition)"@fi .

<http://metatietosanasto.fi/159> a skos:Concept ;
    skos:inScheme : ;
    skos:prefLabel "uudistettu painos"@fi ;
    skos:scopeNote "Sisältö on tarkistettu ja uudistettu. Esim. tilastotietoja päivitetty tai kartan maan rajat muuttuneet ja painos siltä osin uudistettu. Onix-termi. (engl.:revised edition)"@fi .

<http://metatietosanasto.fi/160> a skos:Concept ;
    skos:inScheme : ;
    skos:prefLabel "uusi  painos"@fi ;
    skos:scopeNote "Saman sisältöinen kuin aikaisempi painos. Pieniä muutoksia saatettu tehdä, esim. kirjoitusvirheitä korjattu. Onix-termi. (engl.: new edition)"@fi .

rdam:P30007 a skos:Concept ;
    reg:name "copyrightDate"@en ;
    reg:status <http://metadataregistry.org/uri/RegStatus/1001> ;
    rdfs:domain rdac:C10007 ;
    rdfs:isDefinedBy rdam: ;
    rdfs:subPropertyOf rdau:P60069 ;
    owl:sameAs rdam:copyrightDate ;
    skos:definition "Relates a manifestation to a date associated with a claim of protection under copyright or a similar regime."@en ;
    skos:inScheme : ;
    skos:prefLabel "has copyright date"@en .

rdam:P30016 a skos:Concept ;
    reg:name "electronicReproduction"@en ;
    reg:status <http://metadataregistry.org/uri/RegStatus/1001> ;
    rdfs:domain rdac:C10007 ;
    rdfs:isDefinedBy rdam: ;
    rdfs:range rdac:C10007 ;
    rdfs:subPropertyOf rdam:P30039,
        rdau:P60083 ;
    owl:inverseOf rdam:P30136 ;
    owl:sameAs rdam:electronicReproduction ;
    skos:definition "Relates a manifestation to a digital manifestation resulting from the reproduction of an analog manifestation."@en ;
    skos:inScheme : ;
    skos:prefLabel "is electronic reproduction"@en .

rdam:P30019 a skos:Concept ;
    reg:name "facsimileContainedIn"@en ;
    reg:status <http://metadataregistry.org/uri/RegStatus/1001> ;
    rdfs:domain rdac:C10007 ;
    rdfs:isDefinedBy rdam: ;
    rdfs:range rdac:C10007 ;
    rdfs:subPropertyOf rdam:P30020,
        rdau:P60100 ;
    owl:inverseOf rdam:P30046 ;
    owl:sameAs rdam:facsimileContainedIn ;
    skos:definition "Relates a manifestation to a larger manifestation of which a part is a discrete component that exactly reproduces another manifestation embodying the same expression of a work."@en ;
    skos:inScheme : ;
    skos:prefLabel "is facsimile contained in"@en .

rdam:P30021 a skos:Concept ;
    reg:name "preservationFacsimile"@en ;
    reg:status <http://metadataregistry.org/uri/RegStatus/1001> ;
    rdfs:domain rdac:C10007 ;
    rdfs:isDefinedBy rdam: ;
    rdfs:range rdac:C10007 ;
    rdfs:subPropertyOf rdam:P30031,
        rdau:P60179 ;
    owl:inverseOf rdam:P30045 ;
    owl:sameAs rdam:preservationFacsimile ;
    skos:definition "Relates a manifestation to a manifestation consisting of an exact reproduction on preservation-quality media, such as acid-free permanent or archival paper."@en ;
    skos:inScheme : ;
    skos:prefLabel "is preservation facsimile"@en .

rdam:P30022 a skos:Concept ;
    reg:name "insert"@en ;
    reg:status <http://metadataregistry.org/uri/RegStatus/1001> ;
    rdfs:domain rdac:C10007 ;
    rdfs:isDefinedBy rdam: ;
    rdfs:range rdac:C10007 ;
    rdfs:subPropertyOf rdam:P30033,
        rdau:P60183 ;
    owl:inverseOf rdam:P30025 ;
    owl:sameAs rdam:insert ;
    skos:definition "Relates a manifestation to a manifestation consisting of separately issued material that is not an integral part of the larger manifestation into which it has been inserted."@en ;
    skos:inScheme : ;
    skos:prefLabel "is insert"@en .

rdam:P30025 a skos:Concept ;
    reg:name "insertedIn"@en ;
    reg:status <http://metadataregistry.org/uri/RegStatus/1001> ;
    rdfs:domain rdac:C10007 ;
    rdfs:isDefinedBy rdam: ;
    rdfs:range rdac:C10007 ;
    rdfs:subPropertyOf rdam:P30020,
        rdau:P60194 ;
    owl:inverseOf rdam:P30022 ;
    owl:sameAs rdam:insertedIn ;
    skos:definition "Relates a manifestation to a manifestation into which material has been inserted that is not an integral part of the publication."@en ;
    skos:inScheme : ;
    skos:prefLabel "is inserted in"@en .

rdam:P30026 a skos:Concept ;
    reg:name "alsoIssuedAs"@en ;
    reg:status <http://metadataregistry.org/uri/RegStatus/1001> ;
    rdfs:domain rdac:C10007 ;
    rdfs:isDefinedBy rdam: ;
    rdfs:range rdac:C10007 ;
    rdfs:subPropertyOf rdam:P30024,
        rdau:P60195 ;
    owl:inverseOf rdam:P30026 ;
    owl:sameAs rdam:alsoIssuedAs ;
    skos:definition "Relates a manifestation to a manifestation issued in a different format embodying the same expression of a work as the resource being described."@en ;
    skos:inScheme : ;
    skos:prefLabel "is also issued as"@en .

rdam:P30028 a skos:Concept ;
    reg:name "mirrorSite"@en ;
    reg:status <http://metadataregistry.org/uri/RegStatus/1001> ;
    rdfs:domain rdac:C10007 ;
    rdfs:isDefinedBy rdam: ;
    rdfs:range rdac:C10007 ;
    rdfs:subPropertyOf rdam:P30024,
        rdau:P60197 ;
    owl:inverseOf rdam:P30028 ;
    owl:sameAs rdam:mirrorSite ;
    skos:definition "Relates a manifestation to a manifestation of a website that is an exact copy, used to reduce network traffic or improve the availability of the original site."@en ;
    skos:inScheme : ;
    skos:prefLabel "is mirror site"@en .

rdam:P30029 a skos:Concept ;
    reg:name "digitalTransfer"@en ;
    reg:status <http://metadataregistry.org/uri/RegStatus/1001> ;
    rdfs:domain rdac:C10007 ;
    rdfs:isDefinedBy rdam: ;
    rdfs:range rdac:C10007 ;
    rdfs:subPropertyOf rdam:P30039,
        rdau:P60200 ;
    owl:inverseOf rdam:P30040 ;
    owl:sameAs rdam:digitalTransfer ;
    skos:definition "Relates a manifestation to a manifestation resulting from the transfer of a resource from one digital format to another."@en ;
    skos:inScheme : ;
    skos:prefLabel "is digital transfer"@en .

rdam:P30030 a skos:Concept ;
    reg:name "specialIssue"@en ;
    reg:status <http://metadataregistry.org/uri/RegStatus/1001> ;
    rdfs:domain rdac:C10007 ;
    rdfs:isDefinedBy rdam: ;
    rdfs:range rdac:C10007 ;
    rdfs:subPropertyOf rdam:P30033,
        rdau:P60207 ;
    owl:inverseOf rdam:P30101 ;
    owl:sameAs rdam:specialIssue ;
    skos:definition "Relates a manifestation to a manifestation that consists of a single issue or a supplementary section of a serial or newspaper devoted to a special subject."@en ;
    skos:inScheme : ;
    skos:prefLabel "is special issue"@en .

rdam:P30036 a skos:Concept ;
    reg:name "onDiscWithManifestation"@en ;
    reg:status <http://metadataregistry.org/uri/RegStatus/1001> ;
    rdfs:domain rdac:C10007 ;
    rdfs:isDefinedBy rdam: ;
    rdfs:range rdac:C10007 ;
    rdfs:subPropertyOf rdam:P30035,
        rdau:P60257 ;
    owl:inverseOf rdam:P30036 ;
    owl:sameAs rdam:onDiscWithManifestation ;
    skos:definition "Relates a manifestation to a manifestation that is issued on the same disc with the manifestation being described."@en ;
    skos:inScheme : ;
    skos:prefLabel "is on disc with (manifestation)"@en .

rdam:P30037 a skos:Concept ;
    reg:name "filmedWithManifestation"@en ;
    reg:status <http://metadataregistry.org/uri/RegStatus/1001> ;
    rdfs:domain rdac:C10007 ;
    rdfs:isDefinedBy rdam: ;
    rdfs:range rdac:C10007 ;
    rdfs:subPropertyOf rdam:P30035,
        rdau:P60258 ;
    owl:inverseOf rdam:P30037 ;
    owl:sameAs rdam:filmedWithManifestation ;
    skos:definition "Relates a manifestation to a manifestation that is issued on the same microform with the manifestation being described."@en ;
    skos:inScheme : ;
    skos:prefLabel "is filmed with (manifestation)"@en .

rdam:P30038 a skos:Concept ;
    reg:name "reprintedAs"@en ;
    reg:status <http://metadataregistry.org/uri/RegStatus/1001> ;
    rdfs:domain rdac:C10007 ;
    rdfs:isDefinedBy rdam: ;
    rdfs:range rdac:C10007 ;
    rdfs:subPropertyOf rdam:P30039,
        rdau:P60271 ;
    owl:inverseOf rdam:P30093 ;
    owl:sameAs rdam:reprintedAs ;
    skos:definition "Relates a manifestation to a manifestation that reissues the same expression of the work as the printed resource being described."@en ;
    skos:inScheme : ;
    skos:prefLabel "is reprinted as"@en .

rdam:P30040 a skos:Concept ;
    reg:name "digitalTransferManifestation"@en ;
    reg:status <http://metadataregistry.org/uri/RegStatus/1001> ;
    rdfs:domain rdac:C10007 ;
    rdfs:isDefinedBy rdam: ;
    rdfs:range rdac:C10007 ;
    rdfs:subPropertyOf rdam:P30043,
        rdau:P60287 ;
    owl:inverseOf rdam:P30029 ;
    owl:sameAs rdam:digitalTransferManifestation ;
    skos:definition "Relates a manifestation to a manifestation transferred from one digital format to another."@en ;
    skos:inScheme : ;
    skos:prefLabel "is digital transfer of (manifestation)"@en .

rdam:P30045 a skos:Concept ;
    reg:name "preservationFacsimileOfManifestation"@en ;
    reg:status <http://metadataregistry.org/uri/RegStatus/1001> ;
    rdfs:domain rdac:C10007 ;
    rdfs:isDefinedBy rdam: ;
    rdfs:range rdac:C10007 ;
    rdfs:subPropertyOf rdam:P30047,
        rdau:P60299 ;
    owl:inverseOf rdam:P30021 ;
    owl:sameAs rdam:preservationFacsimileOfManifestation ;
    skos:definition "Relates a manifestation to a manifestation used as the basis for an exact reproduction on preservation-quality media, such as acid-free permanent or archival paper."@en ;
    skos:inScheme : ;
    skos:prefLabel "is preservation facsimile of (manifestation)"@en .

rdam:P30046 a skos:Concept ;
    reg:name "facsimileContainerOf"@en ;
    reg:status <http://metadataregistry.org/uri/RegStatus/1001> ;
    rdfs:domain rdac:C10007 ;
    rdfs:isDefinedBy rdam: ;
    rdfs:range rdac:C10007 ;
    rdfs:subPropertyOf rdam:P30033,
        rdau:P60300 ;
    owl:inverseOf rdam:P30019 ;
    owl:sameAs rdam:containsFacsimileOf,
        rdam:facsimileContainerOf ;
    skos:definition "Relates a manifestation to a manifestation used as the basis for an exact reproduction that is a discrete component of a larger manifestation."@en ;
    skos:inScheme : ;
    skos:prefLabel "is facsimile container of"@en .

rdam:P30052 a skos:Concept ;
    reg:name "noteOnDistributionStatement"@en ;
    reg:status <http://metadataregistry.org/uri/RegStatus/1001> ;
    rdfs:domain rdac:C10007 ;
    rdfs:isDefinedBy rdam: ;
    rdfs:subPropertyOf rdam:P30137,
        rdau:P60125 ;
    owl:sameAs rdam:noteOnDistributionStatement ;
    skos:definition "Relates a manifestation to a note providing details on place of distribution, distributor, or date of distribution, or information on changes in the place of distribution, distributor, or distributor’s name."@en ;
    skos:inScheme : ;
    skos:prefLabel "has note on distribution statement"@en .

rdam:P30053 a skos:Concept ;
    reg:name "noteOnManufactureStatement"@en ;
    reg:status <http://metadataregistry.org/uri/RegStatus/1001> ;
    rdfs:domain rdac:C10007 ;
    rdfs:isDefinedBy rdam: ;
    rdfs:subPropertyOf rdam:P30137,
        rdau:P60126 ;
    owl:sameAs rdam:noteOnManufactureStatement ;
    skos:definition "Relates a manifestation to a note providing details on place of manufacture, manufacturer, or date of manufacture, or information on changes in the place of manufacture, manufacturer, or manufacturer’s name."@en ;
    skos:inScheme : ;
    skos:prefLabel "has note on manufacture statement"@en .

rdam:P30055 a skos:Concept ;
    reg:name "noteOnPublicationStatement"@en ;
    reg:status <http://metadataregistry.org/uri/RegStatus/1001> ;
    rdfs:domain rdac:C10007 ;
    rdfs:isDefinedBy rdam: ;
    rdfs:subPropertyOf rdam:P30137,
        rdau:P60128 ;
    owl:sameAs rdam:noteOnPublicationStatement ;
    skos:definition "Relates a manifestation to a note providing details on place of publication, publisher, or date of publication, information on changes in the place of publication, publisher, or publisher’s name, or on suspension of publication."@en ;
    skos:inScheme : ;
    skos:prefLabel "has note on publication statement"@en .

rdam:P30059 a skos:Concept ;
    reg:name "noteOnCopyrightDate"@en ;
    reg:status <http://metadataregistry.org/uri/RegStatus/1001> ;
    rdfs:domain rdac:C10007 ;
    rdfs:isDefinedBy rdam: ;
    rdfs:subPropertyOf rdam:P30137,
        rdau:P60132 ;
    owl:sameAs rdam:noteOnCopyrightDate ;
    skos:definition "Relates a manifestation to a note providing information on copyright dates not recorded as part of the copyright date element."@en ;
    skos:inScheme : ;
    skos:prefLabel "has note on copyright date"@en .

rdam:P30063 a skos:Concept ;
    reg:name "noteOnTitle"@en ;
    reg:status <http://metadataregistry.org/uri/RegStatus/1001> ;
    rdfs:domain rdac:C10007 ;
    rdfs:isDefinedBy rdam: ;
    rdfs:subPropertyOf rdam:P30137,
        rdau:P60136 ;
    owl:sameAs rdam:noteOnTitle ;
    skos:definition "Relates a manifestation to a note providing information on the source from which a title was taken, the date the title was viewed, variations in titles, inaccuracies, deletions, etc., or other information relating to a title."@en ;
    skos:inScheme : ;
    skos:prefLabel "has note on title"@en .

rdam:P30064 a skos:Concept ;
    reg:name "noteOnEditionStatement"@en ;
    reg:status <http://metadataregistry.org/uri/RegStatus/1001> ;
    rdfs:domain rdac:C10007 ;
    rdfs:isDefinedBy rdam: ;
    rdfs:subPropertyOf rdam:P30137,
        rdau:P60137 ;
    owl:sameAs rdam:noteOnEditionStatement ;
    skos:definition "Relates a manifestation to a note providing information on the source of an edition statement, on edition statements relating to issues, parts, etc., on changes in edition statements, or other information relating to an edition statement."@en ;
    skos:inScheme : ;
    skos:prefLabel "has note on edition statement"@en .

rdam:P30080 a skos:Concept ;
    reg:hasSubproperty rdam:P30068 ;
    reg:name "distributor"@en ;
    reg:status <http://metadataregistry.org/uri/RegStatus/1001> ;
    rdfs:domain rdac:C10007 ;
    rdfs:isDefinedBy rdam: ;
    rdfs:range rdac:C10002 ;
    rdfs:subPropertyOf rdau:P60438 ;
    owl:inverseOf rdaa:P50199 ;
    owl:sameAs rdam:distributor ;
    skos:definition "Relates a manifestation to a person, family, or corporate body responsible for distributing a resource."@en ;
    skos:inScheme : ;
    skos:prefLabel "has distributor"@en .

rdam:P30083 a skos:Concept ;
    reg:hasSubproperty rdam:P30067 ;
    reg:name "publisher"@en ;
    reg:status <http://metadataregistry.org/uri/RegStatus/1001> ;
    rdfs:domain rdac:C10007 ;
    rdfs:isDefinedBy rdam: ;
    rdfs:range rdac:C10002 ;
    rdfs:subPropertyOf rdau:P60444 ;
    owl:inverseOf rdaa:P50203 ;
    owl:sameAs rdam:publisher ;
    skos:definition "Relates a manifestation to a person, family, or corporate body responsible for publishing, releasing, or issuing a resource."@en ;
    skos:inScheme : ;
    skos:prefLabel "has publisher"@en .

rdam:P30093 a skos:Concept ;
    reg:name "reprintOfManifestation"@en ;
    reg:status <http://metadataregistry.org/uri/RegStatus/1001> ;
    rdfs:domain rdac:C10007 ;
    rdfs:isDefinedBy rdam: ;
    rdfs:range rdac:C10007 ;
    rdfs:subPropertyOf rdam:P30043,
        rdau:P60168 ;
    owl:inverseOf rdam:P30038 ;
    owl:sameAs rdam:reprintOfManifestation ;
    skos:definition "Relates a manifestation to a printed manifestation that is used as the basis for a reissue with the same content as the resource being described."@en ;
    skos:inScheme : ;
    skos:prefLabel "is reprint of (manifestation)"@en .

rdam:P30096 a skos:Concept ;
    reg:name "encodingFormat"@en ;
    reg:status <http://metadataregistry.org/uri/RegStatus/1001> ;
    rdfs:domain rdac:C10007 ;
    rdfs:isDefinedBy rdam: ;
    rdfs:subPropertyOf rdam:P30124,
        rdau:P60314 ;
    owl:sameAs rdam:encodingFormat ;
    skos:definition "Relates a manifestation to a schema, standard, etc., used to encode the digital content of a resource."@en ;
    skos:inScheme : ;
    skos:prefLabel "has encoding format"@en .

rdam:P30101 a skos:Concept ;
    reg:name "specialIssueOf"@en ;
    reg:status <http://metadataregistry.org/uri/RegStatus/1001> ;
    rdfs:domain rdac:C10007 ;
    rdfs:isDefinedBy rdam: ;
    rdfs:range rdac:C10007 ;
    rdfs:subPropertyOf rdam:P30020,
        rdau:P60317 ;
    owl:inverseOf rdam:P30030 ;
    owl:sameAs rdam:specialIssueOf ;
    skos:definition "Relates a manifestation to a serial or newspaper containing a single issue or a supplementary section devoted to a special subject, with or without serial numbering, such as an anniversary number of a periodical or newspaper."@en ;
    skos:inScheme : ;
    skos:prefLabel "is special issue of"@en .

rdam:P30117 a skos:Concept ;
    reg:hasSubproperty rdam:P30105,
        rdam:P30116 ;
    reg:name "statementOfResponsibility"@en ;
    reg:status <http://metadataregistry.org/uri/RegStatus/1001> ;
    rdfs:domain rdac:C10007 ;
    rdfs:isDefinedBy rdam: ;
    rdfs:subPropertyOf rdau:P60339 ;
    owl:sameAs rdam:statementOfResponsibility ;
    skos:definition "Relates a manifestation to a statement relating to the identification and/or function of any persons, families, or corporate bodies responsible for the creation of, or contributing to the realization of, the intellectual or artistic content of a resource."@en ;
    skos:inScheme : ;
    skos:prefLabel "has statement of responsibility"@en .

rdam:P30126 a skos:Concept ;
    reg:hasSubproperty rdam:P30104,
        rdam:P30123 ;
    reg:name "videoCharacteristic"@en ;
    reg:status <http://metadataregistry.org/uri/RegStatus/1001> ;
    rdfs:domain rdac:C10007 ;
    rdfs:isDefinedBy rdam: ;
    rdfs:subPropertyOf rdau:P60352 ;
    owl:sameAs rdam:videoCharacteristic ;
    skos:definition "Relates a manifestation to a technical specification relating to the encoding of video images in a resource."@en ;
    skos:inScheme : ;
    skos:prefLabel "has video characteristic"@en .

rdam:P30127 a skos:Concept ;
    reg:hasSubproperty rdam:P30163,
        rdam:P30200 ;
    reg:name "projectionCharacteristicOfMotionPictureFilm"@en ;
    reg:status <http://metadataregistry.org/uri/RegStatus/1001> ;
    rdfs:domain rdac:C10007 ;
    rdfs:isDefinedBy rdam: ;
    rdfs:subPropertyOf rdau:P60353 ;
    owl:sameAs rdam:projectionCharacteristicOfMotionPictureFilm ;
    skos:definition "Relates a manifestation to a technical specification relating to the projection of a motion picture film."@en ;
    skos:inScheme : ;
    skos:prefLabel "has projection characteristic of motion picture film"@en .

rdam:P30128 a skos:Concept ;
    reg:name "variantTitle"@en ;
    reg:status <http://metadataregistry.org/uri/RegStatus/1001> ;
    rdfs:domain rdac:C10007 ;
    rdfs:isDefinedBy rdam: ;
    rdfs:subPropertyOf rdam:P30134,
        rdau:P60355 ;
    owl:sameAs rdam:variantTitle ;
    skos:definition "Relates a manifestation to a title associated with a resource that differs from a title recorded as the title proper, a parallel title proper, other title information, parallel other title information, earlier title proper, later title proper, key title, or abbreviated title."@en ;
    skos:inScheme : ;
    skos:prefLabel "has variant title"@en .

rdam:P30136 a skos:Concept ;
    reg:name "electronicReproductionOfManifestation"@en ;
    reg:status <http://metadataregistry.org/uri/RegStatus/1001> ;
    rdfs:domain rdac:C10007 ;
    rdfs:isDefinedBy rdam: ;
    rdfs:range rdac:C10007 ;
    rdfs:subPropertyOf rdam:P30043,
        rdau:P60469 ;
    owl:inverseOf rdam:P30016 ;
    owl:sameAs rdam:electronicReproductionOfManifestation ;
    skos:definition "Relates a manifestation to an analog manifestation used as the basis for an electronic reproduction."@en ;
    skos:inScheme : ;
    skos:prefLabel "is electronic reproduction of (manifestation)"@en .

rdam:P30142 a skos:Concept ;
    reg:name "otherTitleInformation"@en ;
    reg:status <http://metadataregistry.org/uri/RegStatus/1001> ;
    rdfs:domain rdac:C10007 ;
    rdfs:isDefinedBy rdam: ;
    rdfs:subPropertyOf rdam:P30134,
        rdau:P60493 ;
    owl:sameAs rdam:otherTitleInformation ;
    skos:definition "Relates a manifestation to information that appears in conjunction with, and is subordinate to, the title proper of a resource."@en ;
    skos:inScheme : ;
    skos:prefLabel "has other title information"@en .

rdam:P30156 a skos:Concept ;
    reg:name "titleProper"@en ;
    reg:status <http://metadataregistry.org/uri/RegStatus/1001> ;
    rdfs:domain rdac:C10007 ;
    rdfs:isDefinedBy rdam: ;
    rdfs:subPropertyOf rdam:P30134,
        rdau:P60515 ;
    owl:sameAs rdam:titleProper ;
    skos:definition "Relates a manifestation to the chief name of a resource (i.e., the title normally used when citing the resource)."@en ;
    skos:inScheme : ;
    skos:prefLabel "has title proper"@en .

rdam:P30169 a skos:Concept ;
    reg:hasSubproperty rdam:P30170,
        rdam:P30171 ;
    reg:name "dimensions"@en ;
    reg:status <http://metadataregistry.org/uri/RegStatus/1001> ;
    rdfs:domain rdac:C10007 ;
    rdfs:isDefinedBy rdam: ;
    rdfs:subPropertyOf rdau:P60539 ;
    owl:sameAs rdam:dimensions ;
    skos:definition "Relates a manifestation to the measurements of the carrier or carriers and/or the container of a resource."@en ;
    skos:inScheme : ;
    skos:prefLabel "has dimensions"@en .

rdam:P30187 a skos:Concept ;
    reg:hasSubproperty rdam:P30188,
        rdam:P30189 ;
    reg:name "productionMethod"@en ;
    reg:status <http://metadataregistry.org/uri/RegStatus/1001> ;
    rdfs:domain rdac:C10007 ;
    rdfs:isDefinedBy rdam: ;
    rdfs:subPropertyOf rdau:P60560 ;
    owl:sameAs rdam:productionMethod ;
    skos:definition "Relates a manifestation to the process used to produce a resource."@en ;
    skos:inScheme : ;
    skos:prefLabel "has production method"@en .

rdam:P30203 a skos:Concept ;
    reg:name "parallelTitleProper"@en ;
    reg:status <http://metadataregistry.org/uri/RegStatus/1001> ;
    rdfs:domain rdac:C10007 ;
    rdfs:isDefinedBy rdam: ;
    rdfs:subPropertyOf rdam:P30134,
        rdau:P60589 ;
    owl:sameAs rdam:parallelTitleProper ;
    skos:definition "Relates a manifestation to the title proper in another language and/or script."@en ;
    skos:inScheme : ;
    skos:prefLabel "has parallel title proper"@en .

rdam:P30209 a skos:Concept ;
    reg:name "keyTitle"@en ;
    reg:status <http://metadataregistry.org/uri/RegStatus/1001> ;
    rdfs:domain rdac:C10007 ;
    rdfs:isDefinedBy rdam: ;
    rdfs:subPropertyOf rdam:P30134,
        rdau:P60597 ;
    owl:sameAs rdam:keyTitle ;
    skos:definition "Relates a manifestation to the unique name assigned to a resource by an issn registration agency."@en ;
    skos:inScheme : ;
    skos:prefLabel "has key title"@en .

rdam:P30211 a skos:Concept ;
    reg:hasSubproperty rdam:P30023 ;
    reg:name "descriptiveManifestationRelationship"@en ;
    reg:status <http://metadataregistry.org/uri/RegStatus/1001> ;
    rdfs:domain rdac:C10007 ;
    rdfs:isDefinedBy rdam: ;
    rdfs:range rdac:C10007 ;
    rdfs:subPropertyOf rdam:P30048,
        rdau:P60711 ;
    owl:sameAs rdam:descriptiveManifestationRelationship ;
    skos:definition "Relates a manifestation to a work that is a description of the manifestation."@en ;
    skos:inScheme : ;
    skos:prefLabel "has descriptive manifestation relationship with"@en .

rdam:P30213 a skos:Concept ;
    reg:hasSubproperty rdam:P30020 ;
    reg:name "wholePartManifestationRelationship"@en ;
    reg:status <http://metadataregistry.org/uri/RegStatus/1001> ;
    rdfs:domain rdac:C10007 ;
    rdfs:isDefinedBy rdam: ;
    rdfs:range rdac:C10007 ;
    rdfs:subPropertyOf rdam:P30048,
        rdau:P60714 ;
    owl:sameAs rdam:wholePartManifestationRelationship ;
    skos:definition "Relates a manifestation to a manifestation that is contained in or contains the manifestation."@en ;
    skos:inScheme : ;
    skos:prefLabel "has whole-part manifestation relationship with"@en .

<http://rdvocab.info/termList/RDACarrierType/1018> skos:narrower <http://metatietosanasto.fi/102> ;
    skos:prefLabel "verkkoaineisto"@fi .

<http://rdvocab.info/termList/fileType/1004> skos:narrower <http://metatietosanasto.fi/153> ;
    skos:prefLabel "kuvatiedostomuoto"@fi .

<http://metatietosanasto.fi/029> a skos:Concept ;
    skos:inScheme : ;
    skos:narrower <http://metatietosanasto.fi/030>,
        <http://metatietosanasto.fi/031> ;
    skos:prefLabel "muu nimeketieto"@fi ;
    skos:scopeNote "Sana, ilmaisu tai merkkiryhmä, joka esiintyy julkaisun päänimekkeen yhteydessä ja sille alisteisena. Muu nimeketieto määrittelee, selittää tai täydentää nimekettä, johon se kuuluu."@fi .

<http://metatietosanasto.fi/081> a skos:Concept ;
    skos:broader <http://rdvocab.info/termList/RDACarrierType/1013> ;
    skos:inScheme : ;
    skos:narrower <http://metatietosanasto.fi/082> ;
    skos:prefLabel "CD-levy"@fi ;
    skos:scopeNote "(CD compact disc) tiedontallennukseen käytettävä optisesti luettava levy. CD-levylle tietoa (ääntä, kuvaa ja tekstiä) voidaan tallentaa yhdelle puolelle yhteen kerrokseen. CD-levytyyppeihin, joiden käyttötavat poikkeavat toisistaan, voidaan viitata kuhunkin eri termillä. CD-äänilevyä ja CD-ROM-levyä (CD-tietolevyä) voidaan ainoastaan toistaa, CD-R-levylle voidaan tallentaa yhden kerran ja CD-RW-levylle useita kertoja. (Tietotekniikan termitalkoot, 15.1.2013)"@fi .

<http://metatietosanasto.fi/083> a skos:Concept ;
    skos:broader <http://rdvocab.info/termList/RDACarrierType/1013> ;
    skos:inScheme : ;
    skos:narrower <http://metatietosanasto.fi/084> ;
    skos:prefLabel "DVD-levy"@fi .

<http://metatietosanasto.fi/096> a skos:Concept ;
    skos:inScheme : ;
    skos:narrower <http://metatietosanasto.fi/097>,
        <http://metatietosanasto.fi/098> ;
    skos:prefLabel "peli"@fi .

<http://metatietosanasto.fi/153> a skos:Concept ;
    skos:broader <http://rdvocab.info/termList/fileType/1004>,
        <http://rdvocab.info/termList/fileType/1006> ;
    skos:inScheme : ;
    skos:prefLabel "TIFF"@fi .

rdam:P30004 a skos:Concept ;
    reg:hasSubproperty rdam:P30065,
        rdam:P30066 ;
    reg:name "identifierForTheManifestation"@en ;
    reg:status <http://metadataregistry.org/uri/RegStatus/1001> ;
    rdfs:domain rdac:C10007 ;
    rdfs:isDefinedBy rdam: ;
    rdfs:subPropertyOf rdau:P60052 ;
    owl:sameAs rdam:identifierForTheManifestation ;
    skos:definition "Relates a manifestation to a character string associated with a manifestation that serves to differentiate that manifestation from other manifestations."@en ;
    skos:inScheme : ;
    skos:prefLabel "has identifier for the manifestation"@en .

rdam:P30027 a skos:Concept ;
    reg:hasSubproperty rdam:P30035 ;
    reg:name "accompaniedByManifestation"@en ;
    reg:status <http://metadataregistry.org/uri/RegStatus/1001> ;
    rdfs:domain rdac:C10007 ;
    rdfs:isDefinedBy rdam: ;
    rdfs:range rdac:C10007 ;
    rdfs:subPropertyOf rdam:P30210,
        rdau:P60196 ;
    owl:inverseOf rdam:P30027 ;
    owl:sameAs rdam:accompaniedByManifestation ;
    skos:definition "Relates a manifestation to a manifestation issued with another manifestation, without any relationship to its content."@en ;
    skos:inScheme : ;
    skos:prefLabel "is accompanied by (manifestation)"@en .

rdam:P30031 a skos:Concept ;
    reg:hasSubproperty rdam:P30021 ;
    reg:name "facsimile"@en ;
    reg:status <http://metadataregistry.org/uri/RegStatus/1001> ;
    rdfs:domain rdac:C10007 ;
    rdfs:isDefinedBy rdam: ;
    rdfs:range rdac:C10007 ;
    rdfs:subPropertyOf rdam:P30039,
        rdau:P60217 ;
    owl:inverseOf rdam:P30047 ;
    owl:sameAs rdam:facsimile ;
    skos:definition "Relates a manifestation to a manifestation that exactly reproduces another manifestation embodying the same expression of a work."@en ;
    skos:inScheme : ;
    skos:prefLabel "is facsimile"@en .

rdam:P30047 a skos:Concept ;
    reg:hasSubproperty rdam:P30045 ;
    reg:name "facsimileOfManifestation"@en ;
    reg:status <http://metadataregistry.org/uri/RegStatus/1001> ;
    rdfs:domain rdac:C10007 ;
    rdfs:isDefinedBy rdam: ;
    rdfs:range rdac:C10007 ;
    rdfs:subPropertyOf rdam:P30043,
        rdau:P60301 ;
    owl:inverseOf rdam:P30031 ;
    owl:sameAs rdam:facsimileOfManifestation ;
    skos:definition "Relates a manifestation to a manifestation used as the basis for an exact reproduction."@en ;
    skos:inScheme : ;
    skos:prefLabel "is facsimile of (manifestation)"@en .

rdam:P30212 a skos:Concept ;
    reg:hasSubproperty rdam:P30024 ;
    reg:name "equivalentManifestationRelationship"@en ;
    reg:status <http://metadataregistry.org/uri/RegStatus/1001> ;
    rdfs:domain rdac:C10007 ;
    rdfs:isDefinedBy rdam: ;
    rdfs:range rdac:C10007 ;
    rdfs:subPropertyOf rdam:P30048,
        rdau:P60712 ;
    owl:inverseOf rdam:P30212 ;
    owl:sameAs rdam:equivalentManifestationRelationship ;
    skos:definition "Relates a manifestation to a manifestation that is equivalent to the manifestation."@en ;
    skos:inScheme : ;
    skos:prefLabel "has equivalent manifestation relationship with"@en .

<http://rdvocab.info/termList/RDACarrierType/1007> skos:narrower <http://metatietosanasto.fi/103>,
        <http://metatietosanasto.fi/104> ;
    skos:prefLabel "äänikasetti"@fi .

<http://rdvocab.info/termList/RDACarrierType/1060> skos:narrower <http://metatietosanasto.fi/086>,
        <http://metatietosanasto.fi/087> ;
    skos:prefLabel "videolevy"@fi .

<http://metatietosanasto.fi/018> a skos:Concept ;
    skos:inScheme : ;
    skos:narrower <http://metatietosanasto.fi/019>,
        <http://metatietosanasto.fi/020>,
        <http://metatietosanasto.fi/021> ;
    skos:prefLabel "Lukulaite"@fi ;
    skos:scopeNote "Lukulaite = lukemislaite. Mikrofilmin lukulaite. Sähkökirjan lukulaite (Kielitoimiston sanakirja)"@fi .

rdam:P30033 a skos:Concept ;
    reg:hasSubproperty rdam:P30022,
        rdam:P30030,
        rdam:P30046 ;
    reg:name "containerOfManifestation"@en ;
    reg:status <http://metadataregistry.org/uri/RegStatus/1001> ;
    rdfs:domain rdac:C10007 ;
    rdfs:isDefinedBy rdam: ;
    rdfs:range rdac:C10007 ;
    rdfs:subPropertyOf rdau:P60249 ;
    owl:inverseOf rdam:P30020 ;
    owl:sameAs rdam:containerOfManifestation,
        rdam:containsManifestation ;
    skos:definition "Relates a manifestation to a manifestation that is a discrete component of a larger manifestation."@en ;
    skos:inScheme : ;
    skos:prefLabel "is container of (manifestation)"@en .

rdam:P30035 a skos:Concept ;
    reg:hasSubproperty rdam:P30036,
        rdam:P30037 ;
    reg:name "issuedWith"@en ;
    reg:status <http://metadataregistry.org/uri/RegStatus/1001> ;
    rdfs:domain rdac:C10007 ;
    rdfs:isDefinedBy rdam: ;
    rdfs:range rdac:C10007 ;
    rdfs:subPropertyOf rdam:P30027,
        rdau:P60256 ;
    owl:inverseOf rdam:P30035 ;
    owl:sameAs rdam:issuedWith ;
    skos:definition "Relates a manifestation to a manifestation that is issued on the same carrier as the manifestation being described."@en ;
    skos:inScheme : ;
    skos:prefLabel "is issued with"@en .

rdam:P30048 a skos:Concept ;
    reg:hasSubproperty rdam:P30211,
        rdam:P30212,
        rdam:P30213 ;
    reg:name "relatedManifestation"@en ;
    reg:status <http://metadataregistry.org/uri/RegStatus/1001> ;
    rdfs:domain rdac:C10007 ;
    rdfs:isDefinedBy rdam: ;
    rdfs:range rdac:C10007 ;
    rdfs:subPropertyOf rdau:P60313 ;
    owl:inverseOf rdam:P30048 ;
    owl:sameAs rdam:relatedManifestation ;
    skos:definition "Relates a manifestation to a manifestation, represented by an identifier or a description, that is related to the manifestation being described (e.g., a manifestation in a different format)."@en ;
    skos:inScheme : ;
    skos:prefLabel "has related manifestation"@en .

rdam:P30020 a skos:Concept ;
    reg:hasSubproperty rdam:P30019,
        rdam:P30025,
        rdam:P30101 ;
    reg:name "containedInManifestation"@en ;
    reg:status <http://metadataregistry.org/uri/RegStatus/1001> ;
    rdfs:domain rdac:C10007 ;
    rdfs:isDefinedBy rdam: ;
    rdfs:range rdac:C10007 ;
    rdfs:subPropertyOf rdam:P30213,
        rdau:P60101 ;
    owl:inverseOf rdam:P30033 ;
    owl:sameAs rdam:containedInManifestation ;
    skos:definition "Relates a manifestation to a larger manifestation of which the manifestation is a discrete component."@en ;
    skos:inScheme : ;
    skos:prefLabel "is contained in (manifestation)"@en .

rdam:P30182 a skos:Concept ;
    reg:hasSubproperty rdam:P30177,
        rdam:P30178,
        rdam:P30179,
        rdam:P30180,
        rdam:P30181 ;
    reg:name "extent"@en ;
    reg:status <http://metadataregistry.org/uri/RegStatus/1001> ;
    rdfs:domain rdac:C10007 ;
    rdfs:isDefinedBy rdam: ;
    rdfs:subPropertyOf rdau:P60550 ;
    owl:sameAs rdam:extent ;
    skos:definition "Relates a manifestation to the number and type of units and/or subunits making up a resource."@en ;
    skos:inScheme : ;
    skos:prefLabel "has extent"@en .

rdam:P30191 a skos:Concept ;
    reg:hasSubproperty rdam:P30190,
        rdam:P30192,
        rdam:P30193,
        rdam:P30194,
        rdam:P30195 ;
    reg:name "generation"@en ;
    reg:status <http://metadataregistry.org/uri/RegStatus/1001> ;
    rdfs:domain rdac:C10007 ;
    rdfs:isDefinedBy rdam: ;
    rdfs:subPropertyOf rdau:P60568 ;
    owl:sameAs rdam:generation ;
    skos:definition "Relates a manifestation to the relationship between an original carrier and the carrier of a reproduction made from the original (e.g., a first generation camera master, a second generation printing master)."@en ;
    skos:inScheme : ;
    skos:prefLabel "has generation"@en .

<http://rdvocab.info/termList/RDACarrierType/1013> skos:narrower <http://metatietosanasto.fi/080>,
        <http://metatietosanasto.fi/081>,
        <http://metatietosanasto.fi/083>,
        <http://metatietosanasto.fi/085> ;
    skos:prefLabel "tietolevy"@fi .

<http://rdvocab.info/termList/RDACarrierType/1045> skos:narrower <http://metatietosanasto.fi/071>,
        <http://metatietosanasto.fi/072>,
        <http://metatietosanasto.fi/073>,
        <http://metatietosanasto.fi/074> ;
    skos:prefLabel "kortti"@fi ;
    skos:scopeNote "Kortti = Tavallisesti pienehkö, suorakaiteen muotoinen, jhk määrätarkoitukseen käytettävä (us. kuvallinen t. kirjoitusta sisältävä) kappale jäykkää paperia t. ohutta pahvia.(Kielitoimiston sanakirja)"@fi .

rdam:P30023 a skos:Concept ;
    reg:hasSubproperty rdam:P30032,
        rdam:P30034,
        rdam:P30041,
        rdam:P30042,
        rdam:P30044 ;
    reg:name "descriptionOfManifestation"@en ;
    reg:status <http://metadataregistry.org/uri/RegStatus/1001> ;
    rdfs:domain rdac:C10007 ;
    rdfs:isDefinedBy rdam: ;
    rdfs:range rdac:C10007 ;
    rdfs:subPropertyOf rdam:P30211,
        rdau:P60190 ;
    owl:sameAs rdam:descriptionOfManifestation ;
    skos:definition "Relates a manifestation to a manifestation described by a describing work."@en ;
    skos:inScheme : ;
    skos:prefLabel "is description of (manifestation)"@en .

rdam:P30024 a skos:Concept ;
    reg:hasSubproperty rdam:P30026,
        rdam:P30028,
        rdam:P30039,
        rdam:P30043 ;
    reg:name "equivalentManifestation"@en ;
    reg:status <http://metadataregistry.org/uri/RegStatus/1001> ;
    rdfs:domain rdac:C10007 ;
    rdfs:isDefinedBy rdam: ;
    rdfs:range rdac:C10007 ;
    rdfs:subPropertyOf rdam:P30212,
        rdau:P60191 ;
    owl:inverseOf rdam:P30024 ;
    owl:sameAs rdam:equivalentManifestation ;
    skos:definition "Relates a manifestation to a manifestation embodying the same expression of a work."@en ;
    skos:inScheme : ;
    skos:prefLabel "is equivalent (manifestation)"@en .

rdam:P30039 a skos:Concept ;
    reg:hasSubproperty rdam:P30016,
        rdam:P30029,
        rdam:P30031,
        rdam:P30038 ;
    reg:name "reproducedAs"@en ;
    reg:status <http://metadataregistry.org/uri/RegStatus/1001> ;
    rdfs:domain rdac:C10007 ;
    rdfs:isDefinedBy rdam: ;
    rdfs:range rdac:C10007 ;
    rdfs:subPropertyOf rdam:P30024,
        rdau:P60272 ;
    owl:inverseOf rdam:P30043 ;
    owl:sameAs rdam:reproducedAs ;
    skos:definition "Relates a manifestation to a manifestation that reproduces another manifestation embodying the same expression of a work."@en ;
    skos:inScheme : ;
    skos:prefLabel "is reproduced as"@en .

rdam:P30043 a skos:Concept ;
    reg:hasSubproperty rdam:P30040,
        rdam:P30047,
        rdam:P30093,
        rdam:P30136 ;
    reg:name "reproductionOfManifestation"@en ;
    reg:status <http://metadataregistry.org/uri/RegStatus/1001> ;
    rdfs:domain rdac:C10007 ;
    rdfs:isDefinedBy rdam: ;
    rdfs:range rdac:C10007 ;
    rdfs:subPropertyOf rdam:P30024,
        rdau:P60297 ;
    owl:inverseOf rdam:P30039 ;
    owl:sameAs rdam:reproductionOfManifestation ;
    skos:definition "Relates a manifestation to a manifestation used as the basis for a reproduction."@en ;
    skos:inScheme : ;
    skos:prefLabel "is reproduction of (manifestation)"@en .

<http://rdvocab.info/termList/RDACarrierType/1004> skos:narrower <http://metatietosanasto.fi/088>,
        <http://metatietosanasto.fi/089>,
        <http://metatietosanasto.fi/090>,
        <http://metatietosanasto.fi/091>,
        <http://metatietosanasto.fi/092> ;
    skos:prefLabel "äänilevy"@fi .

rdam:P30124 a skos:Concept ;
    reg:hasSubproperty rdam:P30006,
        rdam:P30018,
        rdam:P30096,
        rdam:P30102,
        rdam:P30159,
        rdam:P30183,
        rdam:P30202 ;
    reg:name "digitalFileCharacteristic"@en ;
    reg:status <http://metadataregistry.org/uri/RegStatus/1001> ;
    rdfs:domain rdac:C10007 ;
    rdfs:isDefinedBy rdam: ;
    rdfs:subPropertyOf rdau:P60350 ;
    owl:sameAs rdam:digitalFileCharacteristic ;
    skos:definition "Relates a manifestation to a technical specification relating to the digital encoding of text, image, audio, video, and other types of data in a resource."@en ;
    skos:inScheme : ;
    skos:prefLabel "has digital file characteristic"@en .

<http://rdvocab.info/termList/fileType/1001> skos:narrower <http://metatietosanasto.fi/136>,
        <http://metatietosanasto.fi/137>,
        <http://metatietosanasto.fi/138>,
        <http://metatietosanasto.fi/139>,
        <http://metatietosanasto.fi/140>,
        <http://metatietosanasto.fi/141> ;
    skos:prefLabel "äänitiedostomuoto"@fi .

rdam:P30125 a skos:Concept ;
    reg:hasSubproperty rdam:P30138,
        rdam:P30161,
        rdam:P30164,
        rdam:P30172,
        rdam:P30184,
        rdam:P30185,
        rdam:P30201,
        rdam:P30206 ;
    reg:name "soundCharacteristic"@en ;
    reg:status <http://metadataregistry.org/uri/RegStatus/1001> ;
    rdfs:domain rdac:C10007 ;
    rdfs:isDefinedBy rdam: ;
    rdfs:subPropertyOf rdau:P60351 ;
    owl:sameAs rdam:soundCharacteristic ;
    skos:definition "Relates a manifestation to a technical specification relating to the encoding of sound in a resource."@en ;
    skos:inScheme : ;
    skos:prefLabel "has sound characteristic"@en .

rdam:P30165 a skos:Concept ;
    reg:hasSubproperty rdam:P30097,
        rdam:P30098,
        rdam:P30099,
        rdam:P30100,
        rdam:P30147,
        rdam:P30148,
        rdam:P30149,
        rdam:P30150 ;
    reg:name "numberingOfSerials"@en ;
    reg:status <http://metadataregistry.org/uri/RegStatus/1001> ;
    rdfs:domain rdac:C10007 ;
    rdfs:isDefinedBy rdam: ;
    rdfs:subPropertyOf rdau:P60533 ;
    owl:sameAs rdam:numberingOfSerials ;
    skos:definition "Relates a manifestation to the identification of each of the issues or parts of a serial. numbering of serials may include a numeral, a letter, any other character, or the combination of these with or without an accompanying caption (volume, number, etc.) and/or a chronological designation."@en ;
    skos:inScheme : ;
    skos:prefLabel "has numbering of serials"@en .

<http://rdvocab.info/termList/fileType/1002> skos:narrower <http://metatietosanasto.fi/142>,
        <http://metatietosanasto.fi/143>,
        <http://metatietosanasto.fi/144>,
        <http://metatietosanasto.fi/145>,
        <http://metatietosanasto.fi/146>,
        <http://metatietosanasto.fi/147>,
        <http://metatietosanasto.fi/148> ;
    skos:prefLabel "tekstitiedostomuoto"@fi .

rdam:P30134 a skos:Concept ;
    reg:hasSubproperty rdam:P30128,
        rdam:P30129,
        rdam:P30130,
        rdam:P30131,
        rdam:P30142,
        rdam:P30151,
        rdam:P30156,
        rdam:P30203,
        rdam:P30209 ;
    reg:name "title"@en ;
    reg:status <http://metadataregistry.org/uri/RegStatus/1001> ;
    rdfs:domain rdac:C10007 ;
    rdfs:isDefinedBy rdam: ;
    rdfs:subPropertyOf rdau:P60369 ;
    owl:sameAs rdam:title ;
    skos:definition "Relates a manifestation to a word, character, or group of words and/or characters that names a resource or a work contained in it."@en ;
    skos:inScheme : ;
    skos:prefLabel "has title"@en .

<http://rdvocab.info/termList/fileType/1006> skos:narrower <http://metatietosanasto.fi/149>,
        <http://metatietosanasto.fi/150>,
        <http://metatietosanasto.fi/151>,
        <http://metatietosanasto.fi/152>,
        <http://metatietosanasto.fi/153>,
        <http://metatietosanasto.fi/154>,
        <http://metatietosanasto.fi/155>,
        <http://metatietosanasto.fi/156> ;
    skos:prefLabel "videotiedostomuoto"@fi .

rdam:P30082 a skos:Concept ;
    reg:hasSubproperty rdam:P30069,
        rdam:P30070,
        rdam:P30071,
        rdam:P30072,
        rdam:P30073,
        rdam:P30074,
        rdam:P30075,
        rdam:P30076,
        rdam:P30077,
        rdam:P30078 ;
    reg:name "manufacturer"@en ;
    reg:status <http://metadataregistry.org/uri/RegStatus/1001> ;
    rdfs:domain rdac:C10007 ;
    rdfs:isDefinedBy rdam: ;
    rdfs:range rdac:C10002 ;
    rdfs:subPropertyOf rdau:P60443 ;
    owl:inverseOf rdaa:P50202 ;
    owl:sameAs rdam:manufacturer ;
    skos:definition "Relates a manifestation to a person, family, or corporate body responsible for printing, duplicating, casting, etc., a resource in a published form."@en ;
    skos:inScheme : ;
    skos:prefLabel "has manufacturer"@en .

rdam:P30137 a skos:Concept ;
    reg:hasSubproperty rdam:P30050,
        rdam:P30051,
        rdam:P30052,
        rdam:P30053,
        rdam:P30054,
        rdam:P30055,
        rdam:P30056,
        rdam:P30057,
        rdam:P30058,
        rdam:P30059,
        rdam:P30062,
        rdam:P30063,
        rdam:P30064 ;
    reg:name "noteOnManifestation"@en ;
    reg:status <http://metadataregistry.org/uri/RegStatus/1001> ;
    rdfs:domain rdac:C10007 ;
    rdfs:isDefinedBy rdam: ;
    owl:sameAs rdam:noteOnManifestation,
        rdam:noteOnManifestationOrItem ;
    skos:definition "Relates a manifestation to an annotation providing additional information about manifestation attributes."@en ;
    skos:inScheme : ;
    skos:prefLabel "has note on manifestation"@en .

mts:C10007 a isothes:ConceptGroup,
        skos:Collection ;
    rdfs:seeAlso rdac:C10007 ;
    skos:definition "Teoksen ekspression saama ilmiasu."@fi ;
    skos:prefLabel "Manifestaatio"@fi .

<http://metadataregistry.org/uri/RegStatus/1001> a skos:Concept ;
    skos:inScheme : ;
    skos:prefLabel "Published"@en .

rdam: dc:title "RDA Manifestation properties"@en ;
    skos:note "Properties derived from RDA elements and relationship designators with the domain of RDA Manifestation."@en .

: a skos:ConceptScheme ;
    owl:versionInfo "Created with TopBraid Composer"^^xsd:string .

